<?xml version="1.0" encoding="utf-8"?>
<rdf:RDF xmlns:dcmit="http://purl.org/dc/dcmitype/"
   xmlns:dct="http://purl.org/dc/terms/"
   xmlns:foaf="http://xmlns.com/foaf/0.1/"
   xmlns:ont="http://purl.org/net/ns/ontology-annot#"
   xmlns:owl="http://www.w3.org/2002/07/owl#"
   xmlns:rdf="http://www.w3.org/1999/02/22-rdf-syntax-ns#"
   xmlns:rdfs="http://www.w3.org/2000/01/rdf-schema#"
   xmlns:skos="http://www.w3.org/2004/02/skos/core#"
   xmlns:vann="http://purl.org/vocab/vann/"
   xmlns:voaf="http://purl.org/vocommons/voaf#"
   xmlns:vs="http://www.w3.org/2003/06/sw-vocab-status/ns#"
   xmlns:xsd="http://www.w3.org/2001/XMLSchema#"
   xmlns="http://www.w3.org/ns/odrl/2/">
  <owl:Ontology rdf:about="http://www.w3.org/ns/odrl/2/">
    <dct:contributor>W3C Permissions &amp; Obligations Expression Working Group</dct:contributor>
    <dct:creator>James Birminham</dct:creator>
    <dct:creator>Michael Steidl</dct:creator>
    <dct:creator>Mo McRoberts</dct:creator>
    <dct:creator>Renato Iannella</dct:creator>
    <dct:creator>Stuart Myles</dct:creator>
    <dct:description xml:lang="en">The ODRL Vocabulary and Expression defines a set of concepts and terms (the vocabulary) and encoding mechanism (the expression) for permissions and obligations statements describing digital content usage based on the ODRL Information Model</dct:description>
    <dct:issued rdf:datatype="http://www.w3.org/2001/XMLSchema#date">2016-07-05</dct:issued>
    <dct:license rdf:resource="https://www.w3.org/Consortium/Legal/2002/ipr-notice-20021231#Copyright/"/>
    <vann:example rdf:resource="http://www.w3.org/ns/odrl/2/Asset"/>
    <vann:preferredNamespacePrefix>odrl</vann:preferredNamespacePrefix>
    <vann:preferredNamespaceUri rdf:resource="http://w3.org/ns/odrl/2/"/>
    <rdf:type rdf:resource="http://purl.org/vocommons/voaf#Vocabulary"/>
    <rdfs:comment xml:lang="en">This is the RDF ontology for ODRL Version 2.2 (working draft).</rdfs:comment>
    <rdfs:label xml:lang="en">ODRL Version 2.2</rdfs:label>
    <owl:versionInfo>2.2</owl:versionInfo>
  </owl:Ontology>
  <skos:Collection rdf:about="http://www.w3.org/ns/odrl/2/#actionConcept">
    <skos:member rdf:resource="http://www.w3.org/ns/odrl/2/Action"/>
    <skos:member rdf:resource="http://www.w3.org/ns/odrl/2/action"/>
    <skos:prefLabel xml:lang="en">Action Concepts</skos:prefLabel>
  </skos:Collection>
  <skos:Collection rdf:about="http://www.w3.org/ns/odrl/2/#actionValues">
    <skos:member rdf:resource="http://www.w3.org/ns/odrl/2/policyUsage"/>
    <skos:prefLabel xml:lang="en">Values for Actions</skos:prefLabel>
  </skos:Collection>
  <skos:Collection rdf:about="http://www.w3.org/ns/odrl/2/#actions">
    <skos:member rdf:resource="http://www.w3.org/ns/odrl/2/aggregate"/>
    <skos:member rdf:resource="http://www.w3.org/ns/odrl/2/annotate"/>
    <skos:member rdf:resource="http://www.w3.org/ns/odrl/2/anonymize"/>
    <skos:member rdf:resource="http://www.w3.org/ns/odrl/2/archive"/>
    <skos:member rdf:resource="http://www.w3.org/ns/odrl/2/concurrentUse"/>
    <skos:member rdf:resource="http://www.w3.org/ns/odrl/2/derive"/>
    <skos:member rdf:resource="http://www.w3.org/ns/odrl/2/digitize"/>
    <skos:member rdf:resource="http://www.w3.org/ns/odrl/2/display"/>
    <skos:member rdf:resource="http://www.w3.org/ns/odrl/2/distribute"/>
    <skos:member rdf:resource="http://www.w3.org/ns/odrl/2/execute"/>
    <skos:member rdf:resource="http://www.w3.org/ns/odrl/2/extract"/>
    <skos:member rdf:resource="http://www.w3.org/ns/odrl/2/give"/>
    <skos:member rdf:resource="http://www.w3.org/ns/odrl/2/grantUse"/>
    <skos:member rdf:resource="http://www.w3.org/ns/odrl/2/index"/>
    <skos:member rdf:resource="http://www.w3.org/ns/odrl/2/install"/>
    <skos:member rdf:resource="http://www.w3.org/ns/odrl/2/modify"/>
    <skos:member rdf:resource="http://www.w3.org/ns/odrl/2/move"/>
    <skos:member rdf:resource="http://www.w3.org/ns/odrl/2/pay"/>
    <skos:member rdf:resource="http://www.w3.org/ns/odrl/2/play"/>
    <skos:member rdf:resource="http://www.w3.org/ns/odrl/2/present"/>
    <skos:member rdf:resource="http://www.w3.org/ns/odrl/2/print"/>
    <skos:member rdf:resource="http://www.w3.org/ns/odrl/2/read"/>
    <skos:member rdf:resource="http://www.w3.org/ns/odrl/2/reproduce"/>
    <skos:member rdf:resource="http://www.w3.org/ns/odrl/2/sell"/>
    <skos:member rdf:resource="http://www.w3.org/ns/odrl/2/textToSpeech"/>
    <skos:member rdf:resource="http://www.w3.org/ns/odrl/2/transfer"/>
    <skos:member rdf:resource="http://www.w3.org/ns/odrl/2/transform"/>
    <skos:member rdf:resource="http://www.w3.org/ns/odrl/2/translate"/>
    <skos:member rdf:resource="http://www.w3.org/ns/odrl/2/use"/>
    <skos:prefLabel xml:lang="en">Actions for Permissions and Prohibitions</skos:prefLabel>
  </skos:Collection>
  <skos:Collection rdf:about="http://www.w3.org/ns/odrl/2/#assetConcepts">
    <skos:member rdf:resource="http://www.w3.org/ns/odrl/2/Asset"/>
    <skos:member rdf:resource="http://www.w3.org/ns/odrl/2/relation"/>
    <skos:prefLabel xml:lang="en">Asset Concepts</skos:prefLabel>
  </skos:Collection>
  <skos:Collection rdf:about="http://www.w3.org/ns/odrl/2/#assetRelations">
    <skos:member rdf:resource="http://www.w3.org/ns/odrl/2/output"/>
    <skos:member rdf:resource="http://www.w3.org/ns/odrl/2/target"/>
    <skos:prefLabel xml:lang="en">Asset Relations</skos:prefLabel>
  </skos:Collection>
  <skos:Collection rdf:about="http://www.w3.org/ns/odrl/2/#constraintActions">
    <skos:member rdf:resource="http://www.w3.org/ns/odrl/2/absolutePosition"/>
    <skos:member rdf:resource="http://www.w3.org/ns/odrl/2/absoluteSize"/>
    <skos:member rdf:resource="http://www.w3.org/ns/odrl/2/count"/>
    <skos:member rdf:resource="http://www.w3.org/ns/odrl/2/dateTime"/>
    <skos:member rdf:resource="http://www.w3.org/ns/odrl/2/deliveryChannel"/>
    <skos:member rdf:resource="http://www.w3.org/ns/odrl/2/elapsedTime"/>
    <skos:member rdf:resource="http://www.w3.org/ns/odrl/2/event"/>
    <skos:member rdf:resource="http://www.w3.org/ns/odrl/2/fileFormat"/>
    <skos:member rdf:resource="http://www.w3.org/ns/odrl/2/industry"/>
    <skos:member rdf:resource="http://www.w3.org/ns/odrl/2/language"/>
    <skos:member rdf:resource="http://www.w3.org/ns/odrl/2/media"/>
    <skos:member rdf:resource="http://www.w3.org/ns/odrl/2/meteredTime"/>
    <skos:member rdf:resource="http://www.w3.org/ns/odrl/2/payAmount"/>
    <skos:member rdf:resource="http://www.w3.org/ns/odrl/2/percentage"/>
    <skos:member rdf:resource="http://www.w3.org/ns/odrl/2/product"/>
    <skos:member rdf:resource="http://www.w3.org/ns/odrl/2/purpose"/>
    <skos:member rdf:resource="http://www.w3.org/ns/odrl/2/recipient"/>
    <skos:member rdf:resource="http://www.w3.org/ns/odrl/2/relativePosition"/>
    <skos:member rdf:resource="http://www.w3.org/ns/odrl/2/relativeSize"/>
    <skos:member rdf:resource="http://www.w3.org/ns/odrl/2/resolution"/>
    <skos:member rdf:resource="http://www.w3.org/ns/odrl/2/spatial"/>
    <skos:member rdf:resource="http://www.w3.org/ns/odrl/2/systemDevice"/>
    <skos:member rdf:resource="http://www.w3.org/ns/odrl/2/timeInterval"/>
    <skos:member rdf:resource="http://www.w3.org/ns/odrl/2/version"/>
    <skos:member rdf:resource="http://www.w3.org/ns/odrl/2/virtualLocation"/>
    <skos:prefLabel xml:lang="en">Actions for Constraints</skos:prefLabel>
  </skos:Collection>
  <skos:Collection rdf:about="http://www.w3.org/ns/odrl/2/#constraintOperators">
    <skos:member rdf:resource="http://www.w3.org/ns/odrl/2/eq"/>
    <skos:member rdf:resource="http://www.w3.org/ns/odrl/2/gt"/>
    <skos:member rdf:resource="http://www.w3.org/ns/odrl/2/gteq"/>
    <skos:member rdf:resource="http://www.w3.org/ns/odrl/2/hasPart"/>
    <skos:member rdf:resource="http://www.w3.org/ns/odrl/2/isA"/>
    <skos:member rdf:resource="http://www.w3.org/ns/odrl/2/isAllof"/>
    <skos:member rdf:resource="http://www.w3.org/ns/odrl/2/isAnyof"/>
    <skos:member rdf:resource="http://www.w3.org/ns/odrl/2/isNoneOf"/>
    <skos:member rdf:resource="http://www.w3.org/ns/odrl/2/isPartOf"/>
    <skos:member rdf:resource="http://www.w3.org/ns/odrl/2/lt"/>
    <skos:member rdf:resource="http://www.w3.org/ns/odrl/2/lteq"/>
    <skos:member rdf:resource="http://www.w3.org/ns/odrl/2/neq"/>
    <skos:prefLabel xml:lang="en">Constraint Operators</skos:prefLabel>
  </skos:Collection>
  <skos:Collection rdf:about="http://www.w3.org/ns/odrl/2/#constraints">
    <skos:member rdf:resource="http://www.w3.org/ns/odrl/2/Constraint"/>
    <skos:member rdf:resource="http://www.w3.org/ns/odrl/2/Operator"/>
    <skos:member rdf:resource="http://www.w3.org/ns/odrl/2/constraint"/>
    <skos:member rdf:resource="http://www.w3.org/ns/odrl/2/dataType"/>
    <skos:member rdf:resource="http://www.w3.org/ns/odrl/2/operator"/>
    <skos:member rdf:resource="http://www.w3.org/ns/odrl/2/rightOperand"/>
    <skos:member rdf:resource="http://www.w3.org/ns/odrl/2/status"/>
    <skos:member rdf:resource="http://www.w3.org/ns/odrl/2/unit"/>
    <skos:prefLabel xml:lang="en">Constraint Concepts</skos:prefLabel>
  </skos:Collection>
  <skos:Collection rdf:about="http://www.w3.org/ns/odrl/2/#deprecatedTerms">
    <skos:member rdf:resource="http://www.w3.org/ns/odrl/2/adHocShare"/>
    <skos:member rdf:resource="http://www.w3.org/ns/odrl/2/append"/>
    <skos:member rdf:resource="http://www.w3.org/ns/odrl/2/appendTo"/>
    <skos:member rdf:resource="http://www.w3.org/ns/odrl/2/attachPolicy"/>
    <skos:member rdf:resource="http://www.w3.org/ns/odrl/2/attachSource"/>
    <skos:member rdf:resource="http://www.w3.org/ns/odrl/2/commercialize"/>
    <skos:member rdf:resource="http://www.w3.org/ns/odrl/2/copy"/>
    <skos:member rdf:resource="http://www.w3.org/ns/odrl/2/device"/>
    <skos:member rdf:resource="http://www.w3.org/ns/odrl/2/export"/>
    <skos:member rdf:resource="http://www.w3.org/ns/odrl/2/extractChar"/>
    <skos:member rdf:resource="http://www.w3.org/ns/odrl/2/extractPage"/>
    <skos:member rdf:resource="http://www.w3.org/ns/odrl/2/extractWord"/>
    <skos:member rdf:resource="http://www.w3.org/ns/odrl/2/lease"/>
    <skos:member rdf:resource="http://www.w3.org/ns/odrl/2/lend"/>
    <skos:member rdf:resource="http://www.w3.org/ns/odrl/2/license"/>
    <skos:member rdf:resource="http://www.w3.org/ns/odrl/2/preview"/>
    <skos:member rdf:resource="http://www.w3.org/ns/odrl/2/proximity"/>
    <skos:member rdf:resource="http://www.w3.org/ns/odrl/2/secondaryUse"/>
    <skos:member rdf:resource="http://www.w3.org/ns/odrl/2/share"/>
    <skos:member rdf:resource="http://www.w3.org/ns/odrl/2/shareAlike"/>
    <skos:member rdf:resource="http://www.w3.org/ns/odrl/2/system"/>
    <skos:member rdf:resource="http://www.w3.org/ns/odrl/2/timedCount"/>
    <skos:member rdf:resource="http://www.w3.org/ns/odrl/2/write"/>
    <skos:member rdf:resource="http://www.w3.org/ns/odrl/2/writeTo"/>
    <skos:prefLabel xml:lang="en">Deprecated Terms</skos:prefLabel>
  </skos:Collection>
  <skos:Collection rdf:about="http://www.w3.org/ns/odrl/2/#duties">
    <skos:member rdf:resource="http://www.w3.org/ns/odrl/2/Duty"/>
    <skos:member rdf:resource="http://www.w3.org/ns/odrl/2/duty"/>
    <skos:prefLabel xml:lang="en">Duty Concepts</skos:prefLabel>
  </skos:Collection>
  <skos:Collection rdf:about="http://www.w3.org/ns/odrl/2/#dutyActions">
    <skos:member rdf:resource="http://www.w3.org/ns/odrl/2/acceptTracking"/>
    <skos:member rdf:resource="http://www.w3.org/ns/odrl/2/attribute"/>
    <skos:member rdf:resource="http://www.w3.org/ns/odrl/2/compensate"/>
    <skos:member rdf:resource="http://www.w3.org/ns/odrl/2/delete"/>
    <skos:member rdf:resource="http://www.w3.org/ns/odrl/2/ensureExclusivity"/>
    <skos:member rdf:resource="http://www.w3.org/ns/odrl/2/include"/>
    <skos:member rdf:resource="http://www.w3.org/ns/odrl/2/inform"/>
    <skos:member rdf:resource="http://www.w3.org/ns/odrl/2/nextPolicy"/>
    <skos:member rdf:resource="http://www.w3.org/ns/odrl/2/obtainConsent"/>
    <skos:member rdf:resource="http://www.w3.org/ns/odrl/2/reviewPolicy"/>
    <skos:member rdf:resource="http://www.w3.org/ns/odrl/2/uninstall"/>
    <skos:member rdf:resource="http://www.w3.org/ns/odrl/2/watermark"/>
    <skos:prefLabel xml:lang="en">Actions for Duties</skos:prefLabel>
  </skos:Collection>
  <skos:Collection rdf:about="http://www.w3.org/ns/odrl/2/#partyConcepts">
    <skos:member rdf:resource="http://www.w3.org/ns/odrl/2/Party"/>
    <skos:member rdf:resource="http://www.w3.org/ns/odrl/2/function"/>
    <skos:prefLabel xml:lang="en">Party Concepts</skos:prefLabel>
  </skos:Collection>
  <skos:Collection rdf:about="http://www.w3.org/ns/odrl/2/#partyRoles">
    <skos:member rdf:resource="http://www.w3.org/ns/odrl/2/assignee"/>
    <skos:member rdf:resource="http://www.w3.org/ns/odrl/2/assigner"/>
    <skos:member rdf:resource="http://www.w3.org/ns/odrl/2/attributedParty"/>
    <skos:member rdf:resource="http://www.w3.org/ns/odrl/2/compensatedParty"/>
    <skos:member rdf:resource="http://www.w3.org/ns/odrl/2/consentingParty"/>
    <skos:member rdf:resource="http://www.w3.org/ns/odrl/2/informedParty"/>
    <skos:member rdf:resource="http://www.w3.org/ns/odrl/2/payeeParty"/>
    <skos:member rdf:resource="http://www.w3.org/ns/odrl/2/trackingParty"/>
    <skos:prefLabel xml:lang="en">Party Roles</skos:prefLabel>
  </skos:Collection>
  <skos:Collection rdf:about="http://www.w3.org/ns/odrl/2/#partyScopes">
    <skos:member rdf:resource="http://www.w3.org/ns/odrl/2/All"/>
    <skos:member rdf:resource="http://www.w3.org/ns/odrl/2/All2ndConnections"/>
    <skos:member rdf:resource="http://www.w3.org/ns/odrl/2/AllConnections"/>
    <skos:member rdf:resource="http://www.w3.org/ns/odrl/2/AllGroups"/>
    <skos:member rdf:resource="http://www.w3.org/ns/odrl/2/Group"/>
    <skos:member rdf:resource="http://www.w3.org/ns/odrl/2/Individual"/>
    <skos:prefLabel xml:lang="en">Party Scopes</skos:prefLabel>
  </skos:Collection>
  <skos:Collection rdf:about="http://www.w3.org/ns/odrl/2/#permissions">
    <skos:member rdf:resource="http://www.w3.org/ns/odrl/2/Permission"/>
    <skos:member rdf:resource="http://www.w3.org/ns/odrl/2/permission"/>
    <skos:prefLabel xml:lang="en">Permission Concepts</skos:prefLabel>
  </skos:Collection>
  <skos:Collection rdf:about="http://www.w3.org/ns/odrl/2/#policyConcepts">
    <skos:member rdf:resource="http://www.w3.org/ns/odrl/2/ConflictTerm"/>
    <skos:member rdf:resource="http://www.w3.org/ns/odrl/2/Policy"/>
    <skos:member rdf:resource="http://www.w3.org/ns/odrl/2/Rule"/>
    <skos:member rdf:resource="http://www.w3.org/ns/odrl/2/UndefinedTerm"/>
    <skos:member rdf:resource="http://www.w3.org/ns/odrl/2/conflict"/>
    <skos:member rdf:resource="http://www.w3.org/ns/odrl/2/ignore"/>
    <skos:member rdf:resource="http://www.w3.org/ns/odrl/2/inheritAllowed"/>
    <skos:member rdf:resource="http://www.w3.org/ns/odrl/2/inheritFrom"/>
    <skos:member rdf:resource="http://www.w3.org/ns/odrl/2/invalid"/>
    <skos:member rdf:resource="http://www.w3.org/ns/odrl/2/perm"/>
    <skos:member rdf:resource="http://www.w3.org/ns/odrl/2/profile"/>
    <skos:member rdf:resource="http://www.w3.org/ns/odrl/2/prohibit"/>
    <skos:member rdf:resource="http://www.w3.org/ns/odrl/2/support"/>
    <skos:member rdf:resource="http://www.w3.org/ns/odrl/2/undefined"/>
    <skos:prefLabel xml:lang="en">Policy Concepts</skos:prefLabel>
  </skos:Collection>
  <skos:Collection rdf:about="http://www.w3.org/ns/odrl/2/#policyTypes">
    <skos:member rdf:resource="http://www.w3.org/ns/odrl/2/Agreement"/>
    <skos:member rdf:resource="http://www.w3.org/ns/odrl/2/Offer"/>
    <skos:member rdf:resource="http://www.w3.org/ns/odrl/2/Privacy"/>
    <skos:member rdf:resource="http://www.w3.org/ns/odrl/2/Request"/>
    <skos:member rdf:resource="http://www.w3.org/ns/odrl/2/Set"/>
    <skos:member rdf:resource="http://www.w3.org/ns/odrl/2/Ticket"/>
    <skos:prefLabel xml:lang="en">Policy Types</skos:prefLabel>
  </skos:Collection>
  <skos:Collection rdf:about="http://www.w3.org/ns/odrl/2/#prohibitions">
    <skos:member rdf:resource="http://www.w3.org/ns/odrl/2/Prohibition"/>
    <skos:member rdf:resource="http://www.w3.org/ns/odrl/2/prohibition"/>
    <skos:prefLabel xml:lang="en">Prohibition Concepts</skos:prefLabel>
  </skos:Collection>
  <rdfs:Class rdf:about="http://www.w3.org/ns/odrl/2/Action">
    <rdf:type rdf:resource="http://www.w3.org/2002/07/owl#Class"/>
    <rdfs:comment xml:lang="en">Actions may be allowed by Permissions, disalloed by Prohibitions, or made mandatory by Duties.</rdfs:comment>
    <rdfs:isDefinedBy rdf:resource="http://www.w3.org/ns/odrl/2/"/>
    <rdfs:label xml:lang="en">Action</rdfs:label>
    <rdfs:subClassOf rdf:resource="http://www.w3.org/2004/02/skos/core#Concept"/>
    <skos:definition xml:lang="en">Instances of Action are operations that can be performed</skos:definition>
  </rdfs:Class>
  <rdfs:Class rdf:about="http://www.w3.org/ns/odrl/2/Agreement">
    <rdf:type rdf:resource="http://www.w3.org/2002/07/owl#Class"/>
    <rdfs:comment xml:lang="en">Must contain at least the Party entity with Assigner role and a Party with Assignee role. The latter being granted the terms of the Agreement from the former.</rdfs:comment>
    <rdfs:isDefinedBy rdf:resource="http://www.w3.org/ns/odrl/2/"/>
    <rdfs:label xml:lang="en">Agreement</rdfs:label>
    <rdfs:subClassOf rdf:resource="http://www.w3.org/ns/odrl/2/Policy"/>
    <owl:disjointWith rdf:resource="http://www.w3.org/ns/odrl/2/Offer"/>
    <owl:disjointWith rdf:resource="http://www.w3.org/ns/odrl/2/Privacy"/>
    <owl:disjointWith rdf:resource="http://www.w3.org/ns/odrl/2/Request"/>
    <owl:disjointWith rdf:resource="http://www.w3.org/ns/odrl/2/Set"/>
    <owl:disjointWith rdf:resource="http://www.w3.org/ns/odrl/2/Ticket"/>
    <skos:definition xml:lang="en">Policy expressions that are formal contracts (or licenses) stipulating all the terms of usage and all the parties involved.</skos:definition>
  </rdfs:Class>
  <rdfs:Class rdf:about="http://www.w3.org/ns/odrl/2/All">
    <rdf:type rdf:resource="http://www.w3.org/2002/07/owl#Class"/>
    <rdfs:comment xml:lang="en">For example, may be used to indicate all the users of a specific social network the party is a member of. Note that “group” scope is also assumed.</rdfs:comment>
    <rdfs:isDefinedBy rdf:resource="http://www.w3.org/ns/odrl/2/"/>
    <rdfs:label xml:lang="en">All</rdfs:label>
    <rdfs:subClassOf rdf:resource="http://www.w3.org/ns/odrl/2/Party"/>
    <skos:definition xml:lang="en">Specifies that the scope of the relationship is all of the collective individuals within a context.</skos:definition>
  </rdfs:Class>
  <rdfs:Class rdf:about="http://www.w3.org/ns/odrl/2/All2ndConnections">
    <rdf:type rdf:resource="http://www.w3.org/2002/07/owl#Class"/>
    <rdfs:comment xml:lang="en">For example, may be used to indicate all “friends of friends” of the Party. Note that “group” scope is also assumed.</rdfs:comment>
    <rdfs:isDefinedBy rdf:resource="http://www.w3.org/ns/odrl/2/"/>
    <rdfs:label xml:lang="en">All second-level connections</rdfs:label>
    <rdfs:subClassOf rdf:resource="http://www.w3.org/ns/odrl/2/Party"/>
    <skos:definition xml:lang="en">Specifies that the scope of the relationship is all of the second-level connections to the Party.</skos:definition>
  </rdfs:Class>
  <rdfs:Class rdf:about="http://www.w3.org/ns/odrl/2/AllConnections">
    <rdf:type rdf:resource="http://www.w3.org/2002/07/owl#Class"/>
    <rdfs:comment xml:lang="en">For example, may be used to indicate all “friends” of the Party. Note that “group” scope is also assumed.</rdfs:comment>
    <rdfs:isDefinedBy rdf:resource="http://www.w3.org/ns/odrl/2/"/>
    <rdfs:label xml:lang="en">All connections</rdfs:label>
    <rdfs:subClassOf rdf:resource="http://www.w3.org/ns/odrl/2/Party"/>
    <skos:definition xml:lang="en">Specifies that the scope of the relationship is all of the first-level connections of the Party.</skos:definition>
  </rdfs:Class>
  <rdfs:Class rdf:about="http://www.w3.org/ns/odrl/2/AllGroups">
    <rdf:type rdf:resource="http://www.w3.org/2002/07/owl#Class"/>
    <rdfs:comment xml:lang="en">For example, may be used to indicate all groups that the Party is a member of. Note that “group” scope is also assumed.</rdfs:comment>
    <rdfs:isDefinedBy rdf:resource="http://www.w3.org/ns/odrl/2/"/>
    <rdfs:label xml:lang="en">All groups</rdfs:label>
    <rdfs:subClassOf rdf:resource="http://www.w3.org/ns/odrl/2/Party"/>
    <skos:definition xml:lang="en">Specifies that the scope of the relationship is all of the group connections of the Party.</skos:definition>
  </rdfs:Class>
  <rdfs:Class rdf:about="http://www.w3.org/ns/odrl/2/Asset">
    <rdf:type rdf:resource="http://www.w3.org/2002/07/owl#Class"/>
    <rdfs:comment xml:lang="en">The Asset entity can be any form of identifiable resource, such as data/information, content/media, applications, or services. Furthermore, it can be used to represent other Asset entities that are needed to undertake the Policy expression, such as with the Duty entity. To describe more details about the Asset, it is recommened to use Dublin Core [[dcterms]] elements or other content metadata.</rdfs:comment>
    <rdfs:isDefinedBy rdf:resource="http://www.w3.org/ns/odrl/2/"/>
    <rdfs:label xml:lang="en">Asset</rdfs:label>
    <owl:equivalentClass rdf:resource="http://www.w3.org/2002/07/owl#Thing"/>
    <skos:definition xml:lang="en">The Asset entity is the subject of an ODRL policy expression that permissions and prohibitions are applied to.</skos:definition>
  </rdfs:Class>
  <rdfs:Class rdf:about="http://www.w3.org/ns/odrl/2/ConflictTerm">
    <rdf:type rdf:resource="http://www.w3.org/2002/07/owl#Class"/>
    <rdfs:comment xml:lang="en">Instances of ConflictTerm describe policies for resolving conflicts.</rdfs:comment>
    <rdfs:isDefinedBy rdf:resource="http://www.w3.org/ns/odrl/2/"/>
    <rdfs:label xml:lang="en">Conflict term</rdfs:label>
    <skos:definition xml:lang="en">Is used to resolve conflicts arising from the merging of policies, specifically when there are conflicting Actions in the Permissions and Prohibitions</skos:definition>
  </rdfs:Class>
  <rdfs:Class rdf:about="http://www.w3.org/ns/odrl/2/Constraint">
    <rdf:type rdf:resource="http://www.w3.org/2002/07/owl#Class"/>
    <rdfs:comment xml:lang="en">Parent class of all Constraints.</rdfs:comment>
    <rdfs:isDefinedBy rdf:resource="http://www.w3.org/ns/odrl/2/"/>
    <rdfs:label xml:lang="en">Constraint</rdfs:label>
    <rdfs:subClassOf rdf:resource="http://www.w3.org/2002/07/owl#Thing"/>
    <skos:definition xml:lang="en">The Constraint entity indicates limits and restrictions to the Permission, the Prohibition and the Duty entity</skos:definition>
  </rdfs:Class>
  <rdfs:Class rdf:about="http://www.w3.org/ns/odrl/2/Duty">
    <rdf:type rdf:resource="http://www.w3.org/2002/07/owl#Class"/>
    <rdfs:comment xml:lang="en">While implying different semantics, the Duty entity is similar to Permission in that it is an Action that must be undertaken.</rdfs:comment>
    <rdfs:isDefinedBy rdf:resource="http://www.w3.org/ns/odrl/2/"/>
    <rdfs:label xml:lang="en">Duty</rdfs:label>
    <rdfs:subClassOf rdf:resource="http://www.w3.org/ns/odrl/2/Rule"/>
    <owl:disjointWith rdf:resource="http://www.w3.org/ns/odrl/2/Permission"/>
    <owl:disjointWith rdf:resource="http://www.w3.org/ns/odrl/2/Prohibition"/>
    <skos:definition xml:lang="en">A Duty is a rule which indicates a requirement that must be fulfilled in return for being entitled to the referring Permission entity.</skos:definition>
  </rdfs:Class>
  <rdfs:Class rdf:about="http://www.w3.org/ns/odrl/2/Group">
    <rdf:type rdf:resource="http://www.w3.org/2002/07/owl#Class"/>
    <rdfs:comment xml:lang="en">Must be supported.</rdfs:comment>
    <rdfs:isDefinedBy rdf:resource="http://www.w3.org/ns/odrl/2/"/>
    <rdfs:label xml:lang="en">Group</rdfs:label>
    <rdfs:subClassOf rdf:resource="http://www.w3.org/ns/odrl/2/Party"/>
    <skos:definition xml:lang="en">Specifies that the scope of the relationship is the defined group with multiple individual members.</skos:definition>
  </rdfs:Class>
  <rdfs:Class rdf:about="http://www.w3.org/ns/odrl/2/Individual">
    <rdf:type rdf:resource="http://www.w3.org/2002/07/owl#Class"/>
    <rdfs:comment xml:lang="en">Must be supported.</rdfs:comment>
    <rdfs:isDefinedBy rdf:resource="http://www.w3.org/ns/odrl/2/"/>
    <rdfs:label xml:lang="en">Individual</rdfs:label>
    <rdfs:subClassOf rdf:resource="http://www.w3.org/ns/odrl/2/Party"/>
    <skos:definition xml:lang="en">Specifies that the scope of the relationship is the single Party individual.</skos:definition>
  </rdfs:Class>
  <dcmit:Text rdf:about="http://www.w3.org/ns/odrl/2/ODRL22.html">
    <dct:format rdf:resource="http://purl.org/NET/mediatypes/text/html"/>
    <dct:isVersionOf rdf:resource="http://www.w3.org/ns/odrl/2/"/>
    <rdfs:label xml:lang="en">ODRL 2.2 (HTML)</rdfs:label>
    <foaf:primaryTopic rdf:resource="http://www.w3.org/ns/odrl/2/"/>
  </dcmit:Text>
  <dcmit:Text rdf:about="http://www.w3.org/ns/odrl/2/ODRL22.json">
    <dct:format rdf:resource="http://purl.org/NET/mediatypes/application/json"/>
    <dct:isVersionOf rdf:resource="http://www.w3.org/ns/odrl/2/"/>
    <rdfs:label xml:lang="en">ODRL 2.2 (JSON Schema Definition)</rdfs:label>
    <foaf:primaryTopic rdf:resource="http://www.w3.org/ns/odrl/2/"/>
  </dcmit:Text>
  <dcmit:Text rdf:about="http://www.w3.org/ns/odrl/2/ODRL22.rdf">
    <dct:format rdf:resource="http://purl.org/NET/mediatypes/application/rdf+xml"/>
    <dct:isVersionOf rdf:resource="http://www.w3.org/ns/odrl/2/"/>
    <rdfs:label xml:lang="en">ODRL 2.2 (RDF/XML)</rdfs:label>
    <foaf:primaryTopic rdf:resource="http://www.w3.org/ns/odrl/2/"/>
  </dcmit:Text>
  <dcmit:Text rdf:about="http://www.w3.org/ns/odrl/2/ODRL22.ttl">
    <dct:format rdf:resource="http://purl.org/NET/mediatypes/text/turtle"/>
    <dct:isVersionOf rdf:resource="http://www.w3.org/ns/odrl/2/"/>
    <rdfs:label xml:lang="en">ODRL 2.2 (Turtle)</rdfs:label>
    <foaf:primaryTopic rdf:resource="http://www.w3.org/ns/odrl/2/"/>
  </dcmit:Text>
  <dcmit:Text rdf:about="http://www.w3.org/ns/odrl/2/ODRL22.xsd">
    <dct:format rdf:resource="http://purl.org/NET/mediatypes/application/xml"/>
    <dct:isVersionOf rdf:resource="http://www.w3.org/ns/odrl/2/"/>
    <rdfs:label xml:lang="en">ODRL 2.2 (XML Schema Definition)</rdfs:label>
    <foaf:primaryTopic rdf:resource="http://www.w3.org/ns/odrl/2/"/>
  </dcmit:Text>
  <rdfs:Class rdf:about="http://www.w3.org/ns/odrl/2/Offer">
    <rdf:type rdf:resource="http://www.w3.org/2002/07/owl#Class"/>
    <rdfs:comment xml:lang="en">Must contain a Party entity with Assigner role. The Offer may contain a Party entity with Assignee role, but does not grant any privileges to that Party.</rdfs:comment>
    <rdfs:isDefinedBy rdf:resource="http://www.w3.org/ns/odrl/2/"/>
    <rdfs:label xml:lang="en">Offer</rdfs:label>
    <rdfs:subClassOf rdf:resource="http://www.w3.org/ns/odrl/2/Policy"/>
    <owl:disjointWith rdf:resource="http://www.w3.org/ns/odrl/2/Agreement"/>
    <owl:disjointWith rdf:resource="http://www.w3.org/ns/odrl/2/Privacy"/>
    <owl:disjointWith rdf:resource="http://www.w3.org/ns/odrl/2/Request"/>
    <owl:disjointWith rdf:resource="http://www.w3.org/ns/odrl/2/Set"/>
    <owl:disjointWith rdf:resource="http://www.w3.org/ns/odrl/2/Ticket"/>
    <skos:definition xml:lang="en">Policy expression that proposes terms of usage from an Asset owner.</skos:definition>
  </rdfs:Class>
  <rdfs:Class rdf:about="http://www.w3.org/ns/odrl/2/Operator">
    <rdf:type rdf:resource="http://www.w3.org/2002/07/owl#Class"/>
    <rdfs:comment xml:lang="en">Instances of the Operator class represent boolean operators</rdfs:comment>
    <rdfs:isDefinedBy rdf:resource="http://www.w3.org/ns/odrl/2/"/>
    <rdfs:label xml:lang="en">Operator</rdfs:label>
    <rdfs:subClassOf rdf:resource="http://www.w3.org/2002/07/owl#Thing"/>
    <skos:definition xml:lang="en">Operators for constraint expressions.</skos:definition>
  </rdfs:Class>
  <rdfs:Class rdf:about="http://www.w3.org/ns/odrl/2/Party">
    <rdf:type rdf:resource="http://www.w3.org/2002/07/owl#Class"/>
    <rdfs:comment xml:lang="en">The Party entity can be any form of identifiable entity, such as a person, group of people, organisation, or agent. An agent is a person or thing that takes an active role or produces a specified effect. To describe more details about the Party, it is recommened to use vCard [[vcard-rdf]] or [[foaf]] metadata.</rdfs:comment>
    <rdfs:isDefinedBy rdf:resource="http://www.w3.org/ns/odrl/2/"/>
    <rdfs:label xml:lang="en">Party</rdfs:label>
    <skos:definition xml:lang="en">The Party entity is the object of an ODRL policy that performs (or not performs) actions or has a role in a Duty.</skos:definition>
  </rdfs:Class>
  <rdfs:Class rdf:about="http://www.w3.org/ns/odrl/2/Permission">
    <rdf:type rdf:resource="http://www.w3.org/2002/07/owl#Class"/>
    <rdfs:comment xml:lang="en">In other words, what the assigner (supplier) has granted to the assignee (consumer).</rdfs:comment>
    <rdfs:isDefinedBy rdf:resource="http://www.w3.org/ns/odrl/2/"/>
    <rdfs:label xml:lang="en">Permission</rdfs:label>
    <rdfs:subClassOf rdf:resource="http://www.w3.org/ns/odrl/2/Rule"/>
    <owl:disjointWith rdf:resource="http://www.w3.org/ns/odrl/2/Duty"/>
    <owl:disjointWith rdf:resource="http://www.w3.org/ns/odrl/2/Prohibition"/>
    <skos:definition xml:lang="en">A Permission is a rule which indicates the actions the assignee is permitted to perform on the associated asset.</skos:definition>
  </rdfs:Class>
  <rdfs:Class rdf:about="http://www.w3.org/ns/odrl/2/Policy">
    <rdf:type rdf:resource="http://www.w3.org/2002/07/owl#Class"/>
    <rdfs:comment xml:lang="en">A top level entity for describing policies.</rdfs:comment>
    <rdfs:isDefinedBy rdf:resource="http://www.w3.org/ns/odrl/2/"/>
    <rdfs:label xml:lang="en">Policy</rdfs:label>
    <rdfs:subClassOf rdf:resource="http://www.w3.org/ns/odrl/2/Asset"/>
    <skos:definition xml:lang="en">An entity to capture the statements of the policy</skos:definition>
  </rdfs:Class>
  <rdfs:Class rdf:about="http://www.w3.org/ns/odrl/2/Privacy">
    <rdf:type rdf:resource="http://www.w3.org/2002/07/owl#Class"/>
    <rdfs:comment xml:lang="en">Must contain at least the Party entity with Assigner role and a Party with Assignee role. Must also contain a Duty on the assignee related to obligations towards managing the assigner’s Asset containing personal information. The Assignee is being granted the terms of the Privacy policy from the Assigner.</rdfs:comment>
    <rdfs:isDefinedBy rdf:resource="http://www.w3.org/ns/odrl/2/"/>
    <rdfs:label xml:lang="en">Privacy</rdfs:label>
    <rdfs:subClassOf rdf:resource="http://www.w3.org/ns/odrl/2/Policy"/>
    <owl:disjointWith rdf:resource="http://www.w3.org/ns/odrl/2/Agreement"/>
    <owl:disjointWith rdf:resource="http://www.w3.org/ns/odrl/2/Offer"/>
    <owl:disjointWith rdf:resource="http://www.w3.org/ns/odrl/2/Request"/>
    <owl:disjointWith rdf:resource="http://www.w3.org/ns/odrl/2/Set"/>
    <owl:disjointWith rdf:resource="http://www.w3.org/ns/odrl/2/Ticket"/>
    <skos:definition xml:lang="en">Policy expression that stipulates the terms of usage over personal information.</skos:definition>
  </rdfs:Class>
  <rdfs:Class rdf:about="http://www.w3.org/ns/odrl/2/Prohibition">
    <rdf:type rdf:resource="http://www.w3.org/2002/07/owl#Class"/>
    <rdfs:comment xml:lang="en">Prohibitions are issued by the supplier of the Asset – the Party with the Role assigner.</rdfs:comment>
    <rdfs:isDefinedBy rdf:resource="http://www.w3.org/ns/odrl/2/"/>
    <rdfs:label xml:lang="en">Prohibition</rdfs:label>
    <rdfs:subClassOf rdf:resource="http://www.w3.org/ns/odrl/2/Rule"/>
    <owl:disjointWith rdf:resource="http://www.w3.org/ns/odrl/2/Duty"/>
    <owl:disjointWith rdf:resource="http://www.w3.org/ns/odrl/2/Permission"/>
    <skos:definition xml:lang="en">A Prohibition is a rule which indicates the Actions that the assignee is prohibited to perform on the related Asset.</skos:definition>
  </rdfs:Class>
  <rdfs:Class rdf:about="http://www.w3.org/ns/odrl/2/Request">
    <rdf:type rdf:resource="http://www.w3.org/2002/07/owl#Class"/>
    <rdfs:comment xml:lang="en">Must contain a Party entity with Assignee role. The Request may also contain the Party entity with Assigner role if this is known. No privileges are granted to any Party.</rdfs:comment>
    <rdfs:isDefinedBy rdf:resource="http://www.w3.org/ns/odrl/2/"/>
    <rdfs:label xml:lang="en">Request</rdfs:label>
    <rdfs:subClassOf rdf:resource="http://www.w3.org/ns/odrl/2/Policy"/>
    <owl:disjointWith rdf:resource="http://www.w3.org/ns/odrl/2/Agreement"/>
    <owl:disjointWith rdf:resource="http://www.w3.org/ns/odrl/2/Offer"/>
    <owl:disjointWith rdf:resource="http://www.w3.org/ns/odrl/2/Privacy"/>
    <owl:disjointWith rdf:resource="http://www.w3.org/ns/odrl/2/Set"/>
    <owl:disjointWith rdf:resource="http://www.w3.org/ns/odrl/2/Ticket"/>
    <skos:definition xml:lang="en">Policy expression that proposes terms of usage to an Asset owner.</skos:definition>
  </rdfs:Class>
  <rdfs:Class rdf:about="http://www.w3.org/ns/odrl/2/Rule">
    <rdf:type rdf:resource="http://www.w3.org/2002/07/owl#Class"/>
    <rdfs:comment xml:lang="en">Rule is an abstract concept.</rdfs:comment>
    <rdfs:isDefinedBy rdf:resource="http://www.w3.org/ns/odrl/2/"/>
    <rdfs:label xml:lang="en">Rule</rdfs:label>
    <skos:definition xml:lang="en">A common ancestor to Permissions, Prohibitions and Duties</skos:definition>
  </rdfs:Class>
  <rdfs:Class rdf:about="http://www.w3.org/ns/odrl/2/Set">
    <rdf:type rdf:resource="http://www.w3.org/2002/07/owl#Class"/>
    <rdfs:comment xml:lang="en">The Set is aimed at scenarios where there is an open criteria for the semantics of the policy expressions and typically refined by other systems/profiles that process the information at a later time. No privileges are granted to any Party.</rdfs:comment>
    <rdfs:isDefinedBy rdf:resource="http://www.w3.org/ns/odrl/2/"/>
    <rdfs:label xml:lang="en">Set</rdfs:label>
    <rdfs:subClassOf rdf:resource="http://www.w3.org/ns/odrl/2/Policy"/>
    <owl:disjointWith rdf:resource="http://www.w3.org/ns/odrl/2/Agreement"/>
    <owl:disjointWith rdf:resource="http://www.w3.org/ns/odrl/2/Offer"/>
    <owl:disjointWith rdf:resource="http://www.w3.org/ns/odrl/2/Privacy"/>
    <owl:disjointWith rdf:resource="http://www.w3.org/ns/odrl/2/Request"/>
    <owl:disjointWith rdf:resource="http://www.w3.org/ns/odrl/2/Ticket"/>
    <skos:definition xml:lang="en">Policy expression that consists of entities from the complete model.</skos:definition>
  </rdfs:Class>
  <rdfs:Class rdf:about="http://www.w3.org/ns/odrl/2/Ticket">
    <rdf:type rdf:resource="http://www.w3.org/2002/07/owl#Class"/>
    <rdfs:comment xml:lang="en">May contain the Party entity with Assigner role and the Party entity with Assignee role. A Ticket (or Voucher) may be anonymous or personalised, where the holder of that Ticket may remain unknown or has to be identified. The holder, or if known, the Assignee, is being granted the terms of the Ticket from the Assigner (in known).</rdfs:comment>
    <rdfs:isDefinedBy rdf:resource="http://www.w3.org/ns/odrl/2/"/>
    <rdfs:label xml:lang="en">Ticket</rdfs:label>
    <rdfs:subClassOf rdf:resource="http://www.w3.org/ns/odrl/2/Policy"/>
    <owl:disjointWith rdf:resource="http://www.w3.org/ns/odrl/2/Agreement"/>
    <owl:disjointWith rdf:resource="http://www.w3.org/ns/odrl/2/Offer"/>
    <owl:disjointWith rdf:resource="http://www.w3.org/ns/odrl/2/Privacy"/>
    <owl:disjointWith rdf:resource="http://www.w3.org/ns/odrl/2/Request"/>
    <owl:disjointWith rdf:resource="http://www.w3.org/ns/odrl/2/Set"/>
    <skos:definition xml:lang="en">Policy expression that stipulates the terms of usage and is redeemable by any Party who currently holds the Ticket in their possession.</skos:definition>
  </rdfs:Class>
  <rdfs:Class rdf:about="http://www.w3.org/ns/odrl/2/UndefinedTerm">
    <rdf:type rdf:resource="http://www.w3.org/2002/07/owl#Class"/>
    <rdfs:comment xml:lang="en">Instances of UndefinedTerm describe policies for processing unsupported actions.</rdfs:comment>
    <rdfs:isDefinedBy rdf:resource="http://www.w3.org/ns/odrl/2/"/>
    <rdfs:label xml:lang="en">Undefined values</rdfs:label>
    <skos:definition xml:lang="en">Is used to indicate how to support Actions that are not part of any profile in the policy expression system</skos:definition>
  </rdfs:Class>
  <rdf:Property rdf:about="http://www.w3.org/ns/odrl/2/absolutePosition">
    <rdf:type rdf:resource="http://www.w3.org/2002/07/owl#DatatypeProperty"/>
    <rdfs:comment xml:lang="en">For example, JPEG image must be positioned at 100×100 pixel location. This may be used to express [[plus]] semantics.</rdfs:comment>
    <rdfs:isDefinedBy rdf:resource="http://www.w3.org/ns/odrl/2/"/>
    <rdfs:label xml:lang="en">absolute position</rdfs:label>
    <rdfs:subPropertyOf rdf:resource="http://www.w3.org/ns/odrl/2/rightOperand"/>
    <skos:definition xml:lang="en">A point defined with absolute coordinates.</skos:definition>
  </rdf:Property>
  <rdf:Property rdf:about="http://www.w3.org/ns/odrl/2/absoluteSize">
    <rdf:type rdf:resource="http://www.w3.org/2002/07/owl#DatatypeProperty"/>
    <rdfs:comment xml:lang="en">For example, JPEG image must be reproduced onto an area no larger than A0. This may be used to express [[plus]] semantics.</rdfs:comment>
    <rdfs:isDefinedBy rdf:resource="http://www.w3.org/ns/odrl/2/"/>
    <rdfs:label xml:lang="en">absolute size</rdfs:label>
    <rdfs:range rdf:resource="http://www.w3.org/2001/XMLSchema#decimal"/>
    <rdfs:subPropertyOf rdf:resource="http://www.w3.org/ns/odrl/2/rightOperand"/>
    <skos:definition xml:lang="en">The absolute dimension that the Asset may be resized.</skos:definition>
  </rdf:Property>
  <Action rdf:about="http://www.w3.org/ns/odrl/2/acceptTracking">
    <rdf:type rdf:resource="http://www.w3.org/2004/02/skos/core#Concept"/>
    <rdfs:comment xml:lang="en">The collected information may be tracked by the Assigner, or may link to a Party with the role function “trackingParty”.</rdfs:comment>
    <rdfs:isDefinedBy rdf:resource="http://www.w3.org/ns/odrl/2/"/>
    <rdfs:label xml:lang="en">Accept tracking</rdfs:label>
    <skos:definition xml:lang="en">The Assigner requires that the Assignees accepts that the use of the Asset may be tracked.</skos:definition>
  </Action>
  <rdf:Property rdf:about="http://www.w3.org/ns/odrl/2/action">
    <rdf:type rdf:resource="http://www.w3.org/2002/07/owl#ObjectProperty"/>
    <rdfs:comment xml:lang="en">A permission must include exactly one action.</rdfs:comment>
    <rdfs:domain rdf:resource="http://www.w3.org/ns/odrl/2/Rule"/>
    <rdfs:isDefinedBy rdf:resource="http://www.w3.org/ns/odrl/2/"/>
    <rdfs:label xml:lang="en">action</rdfs:label>
    <rdfs:range rdf:resource="http://www.w3.org/ns/odrl/2/Action"/>
    <skos:definition xml:lang="en">The operation relating to the asset for which the Rule is being subjected.</skos:definition>
  </rdf:Property>
  <skos:ConceptScheme rdf:about="http://www.w3.org/ns/odrl/2/actions">
    <rdfs:isDefinedBy rdf:resource="http://www.w3.org/ns/odrl/2/"/>
    <rdfs:label xml:lang="en">ODRL Actions vocabulary</rdfs:label>
    <skos:hasTopConcept rdf:resource="http://www.w3.org/ns/odrl/2/acceptTracking"/>
    <skos:hasTopConcept rdf:resource="http://www.w3.org/ns/odrl/2/adHocShare"/>
    <skos:hasTopConcept rdf:resource="http://www.w3.org/ns/odrl/2/aggregate"/>
    <skos:hasTopConcept rdf:resource="http://www.w3.org/ns/odrl/2/annotate"/>
    <skos:hasTopConcept rdf:resource="http://www.w3.org/ns/odrl/2/anonymize"/>
    <skos:hasTopConcept rdf:resource="http://www.w3.org/ns/odrl/2/append"/>
    <skos:hasTopConcept rdf:resource="http://www.w3.org/ns/odrl/2/appendTo"/>
    <skos:hasTopConcept rdf:resource="http://www.w3.org/ns/odrl/2/archive"/>
    <skos:hasTopConcept rdf:resource="http://www.w3.org/ns/odrl/2/attachPolicy"/>
    <skos:hasTopConcept rdf:resource="http://www.w3.org/ns/odrl/2/attachSource"/>
    <skos:hasTopConcept rdf:resource="http://www.w3.org/ns/odrl/2/attribute"/>
    <skos:hasTopConcept rdf:resource="http://www.w3.org/ns/odrl/2/commercialize"/>
    <skos:hasTopConcept rdf:resource="http://www.w3.org/ns/odrl/2/compensate"/>
    <skos:hasTopConcept rdf:resource="http://www.w3.org/ns/odrl/2/concurrentUse"/>
    <skos:hasTopConcept rdf:resource="http://www.w3.org/ns/odrl/2/copy"/>
    <skos:hasTopConcept rdf:resource="http://www.w3.org/ns/odrl/2/delete"/>
    <skos:hasTopConcept rdf:resource="http://www.w3.org/ns/odrl/2/derive"/>
    <skos:hasTopConcept rdf:resource="http://www.w3.org/ns/odrl/2/digitize"/>
    <skos:hasTopConcept rdf:resource="http://www.w3.org/ns/odrl/2/display"/>
    <skos:hasTopConcept rdf:resource="http://www.w3.org/ns/odrl/2/distribute"/>
    <skos:hasTopConcept rdf:resource="http://www.w3.org/ns/odrl/2/ensureExclusivity"/>
    <skos:hasTopConcept rdf:resource="http://www.w3.org/ns/odrl/2/execute"/>
    <skos:hasTopConcept rdf:resource="http://www.w3.org/ns/odrl/2/export"/>
    <skos:hasTopConcept rdf:resource="http://www.w3.org/ns/odrl/2/extract"/>
    <skos:hasTopConcept rdf:resource="http://www.w3.org/ns/odrl/2/give"/>
    <skos:hasTopConcept rdf:resource="http://www.w3.org/ns/odrl/2/grantUse"/>
    <skos:hasTopConcept rdf:resource="http://www.w3.org/ns/odrl/2/include"/>
    <skos:hasTopConcept rdf:resource="http://www.w3.org/ns/odrl/2/index"/>
    <skos:hasTopConcept rdf:resource="http://www.w3.org/ns/odrl/2/inform"/>
    <skos:hasTopConcept rdf:resource="http://www.w3.org/ns/odrl/2/install"/>
    <skos:hasTopConcept rdf:resource="http://www.w3.org/ns/odrl/2/lease"/>
    <skos:hasTopConcept rdf:resource="http://www.w3.org/ns/odrl/2/lend"/>
    <skos:hasTopConcept rdf:resource="http://www.w3.org/ns/odrl/2/license"/>
    <skos:hasTopConcept rdf:resource="http://www.w3.org/ns/odrl/2/modify"/>
    <skos:hasTopConcept rdf:resource="http://www.w3.org/ns/odrl/2/move"/>
    <skos:hasTopConcept rdf:resource="http://www.w3.org/ns/odrl/2/nextPolicy"/>
    <skos:hasTopConcept rdf:resource="http://www.w3.org/ns/odrl/2/obtainConsent"/>
    <skos:hasTopConcept rdf:resource="http://www.w3.org/ns/odrl/2/pay"/>
    <skos:hasTopConcept rdf:resource="http://www.w3.org/ns/odrl/2/play"/>
    <skos:hasTopConcept rdf:resource="http://www.w3.org/ns/odrl/2/present"/>
    <skos:hasTopConcept rdf:resource="http://www.w3.org/ns/odrl/2/preview"/>
    <skos:hasTopConcept rdf:resource="http://www.w3.org/ns/odrl/2/print"/>
    <skos:hasTopConcept rdf:resource="http://www.w3.org/ns/odrl/2/read"/>
    <skos:hasTopConcept rdf:resource="http://www.w3.org/ns/odrl/2/reproduce"/>
    <skos:hasTopConcept rdf:resource="http://www.w3.org/ns/odrl/2/reviewPolicy"/>
    <skos:hasTopConcept rdf:resource="http://www.w3.org/ns/odrl/2/secondaryUse"/>
    <skos:hasTopConcept rdf:resource="http://www.w3.org/ns/odrl/2/sell"/>
    <skos:hasTopConcept rdf:resource="http://www.w3.org/ns/odrl/2/share"/>
    <skos:hasTopConcept rdf:resource="http://www.w3.org/ns/odrl/2/shareAlike"/>
    <skos:hasTopConcept rdf:resource="http://www.w3.org/ns/odrl/2/textToSpeech"/>
    <skos:hasTopConcept rdf:resource="http://www.w3.org/ns/odrl/2/transfer"/>
    <skos:hasTopConcept rdf:resource="http://www.w3.org/ns/odrl/2/transform"/>
    <skos:hasTopConcept rdf:resource="http://www.w3.org/ns/odrl/2/translate"/>
    <skos:hasTopConcept rdf:resource="http://www.w3.org/ns/odrl/2/uninstall"/>
    <skos:hasTopConcept rdf:resource="http://www.w3.org/ns/odrl/2/use"/>
    <skos:hasTopConcept rdf:resource="http://www.w3.org/ns/odrl/2/watermark"/>
    <skos:hasTopConcept rdf:resource="http://www.w3.org/ns/odrl/2/write"/>
    <skos:hasTopConcept rdf:resource="http://www.w3.org/ns/odrl/2/writeTo"/>
  </skos:ConceptScheme>
  <Action rdf:about="http://www.w3.org/ns/odrl/2/adHocShare">
    <ont:deprecatedBy rdf:resource="http://www.openmobilealliance.com/oma-dd/adhoc-share"/>
    <rdf:type rdf:resource="http://www.w3.org/2004/02/skos/core#Concept"/>
    <rdfs:isDefinedBy rdf:resource="http://www.w3.org/ns/odrl/2/"/>
    <rdfs:label xml:lang="en">Ad-hoc sharing</rdfs:label>
    <skos:definition xml:lang="en">The act of sharing the asset to parties in close proximity to the owner.</skos:definition>
  </Action>
  <Action rdf:about="http://www.w3.org/ns/odrl/2/aggregate">
    <rdf:type rdf:resource="http://www.w3.org/2004/02/skos/core#Concept"/>
    <rdfs:isDefinedBy rdf:resource="http://www.w3.org/ns/odrl/2/"/>
    <rdfs:label xml:lang="en">Aggregate</rdfs:label>
    <skos:broaderTransitive rdf:resource="http://www.w3.org/ns/odrl/2/use"/>
    <skos:definition xml:lang="en">The Assigner permits/prohibits the Assignees to use the Asset or parts of it as part of a composite collection.</skos:definition>
  </Action>
  <Action rdf:about="http://www.w3.org/ns/odrl/2/annotate">
    <rdf:type rdf:resource="http://www.w3.org/2004/02/skos/core#Concept"/>
    <rdfs:isDefinedBy rdf:resource="http://www.w3.org/ns/odrl/2/"/>
    <rdfs:label xml:lang="en">Annotate</rdfs:label>
    <skos:broaderTransitive rdf:resource="http://www.w3.org/ns/odrl/2/use"/>
    <skos:definition xml:lang="en">The Assigner permits/prohibits the Assignees to add explanatory notations/commentaries to the Asset without modifying the Asset in any other way.</skos:definition>
  </Action>
  <Action rdf:about="http://www.w3.org/ns/odrl/2/anonymize">
    <rdf:type rdf:resource="http://www.w3.org/2004/02/skos/core#Concept"/>
    <rdfs:comment xml:lang="en">For example, to remove identifying particulars for statistical or for other comparable purposes, or to use the asset without stating the author/source.</rdfs:comment>
    <rdfs:isDefinedBy rdf:resource="http://www.w3.org/ns/odrl/2/"/>
    <rdfs:label xml:lang="en">Anonymize</rdfs:label>
    <skos:broaderTransitive rdf:resource="http://www.w3.org/ns/odrl/2/use"/>
    <skos:definition xml:lang="en">The Assigner permits/prohibits the Assignees to anonymize all or parts of the Asset.</skos:definition>
  </Action>
  <Action rdf:about="http://www.w3.org/ns/odrl/2/append">
    <ont:deprecatedBy rdf:resource="http://www.w3.org/ns/odrl/2/modify"/>
    <rdf:type rdf:resource="http://www.w3.org/2004/02/skos/core#Concept"/>
    <rdfs:isDefinedBy rdf:resource="http://www.w3.org/ns/odrl/2/"/>
    <rdfs:label xml:lang="en">Append</rdfs:label>
    <skos:definition xml:lang="en">The act of adding to the end of an asset.</skos:definition>
  </Action>
  <Action rdf:about="http://www.w3.org/ns/odrl/2/appendTo">
    <ont:deprecatedBy rdf:resource="http://www.w3.org/ns/odrl/2/modify"/>
    <rdf:type rdf:resource="http://www.w3.org/2004/02/skos/core#Concept"/>
    <rdfs:isDefinedBy rdf:resource="http://www.w3.org/ns/odrl/2/"/>
    <rdfs:label xml:lang="en">Append to</rdfs:label>
    <skos:broaderTransitive rdf:resource="http://www.w3.org/ns/odrl/2/writeTo"/>
    <skos:definition xml:lang="en">The act of appending data to the Asset without modifying the Asset in any other way</skos:definition>
  </Action>
  <Action rdf:about="http://www.w3.org/ns/odrl/2/archive">
    <rdf:type rdf:resource="http://www.w3.org/2004/02/skos/core#Concept"/>
    <rdfs:comment xml:lang="en">Constraints may be used for temporal conditions.</rdfs:comment>
    <rdfs:isDefinedBy rdf:resource="http://www.w3.org/ns/odrl/2/"/>
    <rdfs:label xml:lang="en">Archive</rdfs:label>
    <skos:broaderTransitive rdf:resource="http://www.w3.org/ns/odrl/2/use"/>
    <skos:definition xml:lang="en">The Assigner permits/prohibits the Assignees to store the Asset (in a non-transient form).</skos:definition>
  </Action>
  <rdf:Property rdf:about="http://www.w3.org/ns/odrl/2/assignee">
    <rdf:type rdf:resource="http://www.w3.org/2002/07/owl#ObjectProperty"/>
    <rdfs:comment xml:lang="en">Must be supported.</rdfs:comment>
    <rdfs:isDefinedBy rdf:resource="http://www.w3.org/ns/odrl/2/"/>
    <rdfs:label xml:lang="en">assignee</rdfs:label>
    <rdfs:range rdf:resource="http://www.w3.org/ns/odrl/2/Party"/>
    <rdfs:subPropertyOf rdf:resource="http://www.w3.org/ns/odrl/2/function"/>
    <skos:definition xml:lang="en">The Party is the recipient of the policy statement.</skos:definition>
  </rdf:Property>
  <rdf:Property rdf:about="http://www.w3.org/ns/odrl/2/assigner">
    <rdf:type rdf:resource="http://www.w3.org/2002/07/owl#ObjectProperty"/>
    <rdfs:comment xml:lang="en">Must be supported.</rdfs:comment>
    <rdfs:isDefinedBy rdf:resource="http://www.w3.org/ns/odrl/2/"/>
    <rdfs:label xml:lang="en">assigner</rdfs:label>
    <rdfs:range rdf:resource="http://www.w3.org/ns/odrl/2/Party"/>
    <rdfs:subPropertyOf rdf:resource="http://www.w3.org/ns/odrl/2/function"/>
    <skos:definition xml:lang="en">The Party is the issuer of the policy statement.</skos:definition>
  </rdf:Property>
  <Action rdf:about="http://www.w3.org/ns/odrl/2/attachPolicy">
    <ont:deprecatedBy rdf:resource="http://creativecommons.org/ns#Notice"/>
    <rdf:type rdf:resource="http://www.w3.org/2004/02/skos/core#Concept"/>
    <rdfs:isDefinedBy rdf:resource="http://www.w3.org/ns/odrl/2/"/>
    <rdfs:label xml:lang="en">Attach policy</rdfs:label>
    <skos:definition xml:lang="en">The act of keeping the policy notice with the asset.</skos:definition>
  </Action>
  <Action rdf:about="http://www.w3.org/ns/odrl/2/attachSource">
    <ont:deprecatedBy rdf:resource="http://creativecommons.org/ns#SourceCode"/>
    <rdf:type rdf:resource="http://www.w3.org/2004/02/skos/core#Concept"/>
    <rdfs:isDefinedBy rdf:resource="http://www.w3.org/ns/odrl/2/"/>
    <rdfs:label xml:lang="en">Attach source</rdfs:label>
    <skos:definition xml:lang="en">The act of attaching the source of the asset and its derivatives.</skos:definition>
  </Action>
  <Action rdf:about="http://www.w3.org/ns/odrl/2/attribute">
    <rdf:type rdf:resource="http://www.w3.org/2004/02/skos/core#Concept"/>
    <rdfs:comment xml:lang="en">May link to an Asset with the attribution information. May link to a Party with the role function “attributedParty”.</rdfs:comment>
    <rdfs:isDefinedBy rdf:resource="http://www.w3.org/ns/odrl/2/"/>
    <rdfs:label xml:lang="en">Attribute</rdfs:label>
    <skos:definition xml:lang="en">The Assigner requires that the Assignees attributes the Asset to the Assigner or an attributed Party.</skos:definition>
  </Action>
  <rdf:Property rdf:about="http://www.w3.org/ns/odrl/2/attributedParty">
    <rdf:type rdf:resource="http://www.w3.org/2002/07/owl#ObjectProperty"/>
    <rdfs:comment xml:lang="en">Maybe specified as part of the attribute action.</rdfs:comment>
    <rdfs:isDefinedBy rdf:resource="http://www.w3.org/ns/odrl/2/"/>
    <rdfs:label xml:lang="en">attributed party</rdfs:label>
    <rdfs:subPropertyOf rdf:resource="http://www.w3.org/ns/odrl/2/function"/>
    <skos:definition xml:lang="en">The Party to be attributed.</skos:definition>
  </rdf:Property>
  <Action rdf:about="http://www.w3.org/ns/odrl/2/commercialize">
    <ont:deprecatedBy rdf:resource="http://creativecommons.org/ns#CommercialUse"/>
    <rdf:type rdf:resource="http://www.w3.org/2004/02/skos/core#Concept"/>
    <rdfs:isDefinedBy rdf:resource="http://www.w3.org/ns/odrl/2/"/>
    <rdfs:label xml:lang="en">Commercialize</rdfs:label>
    <skos:definition xml:lang="en">The act of using the asset in a business environment.</skos:definition>
  </Action>
  <Action rdf:about="http://www.w3.org/ns/odrl/2/compensate">
    <rdf:type rdf:resource="http://www.w3.org/2004/02/skos/core#Concept"/>
    <rdfs:comment xml:lang="en">The compensation may use different types of things with a value: (i) the thing is expressed by the value (term) of the Constraint name; (b) the value is expressed by operator, rightOperand, dataType and unit</rdfs:comment>
    <rdfs:isDefinedBy rdf:resource="http://www.w3.org/ns/odrl/2/"/>
    <rdfs:label xml:lang="en">Compensate</rdfs:label>
    <skos:definition xml:lang="en">The Assigner requires that the Assignees compensates the Assigner (or other specified compensation Party) by some amount of value, if defined, for use of the Asset.</skos:definition>
  </Action>
  <rdf:Property rdf:about="http://www.w3.org/ns/odrl/2/compensatedParty">
    <rdf:type rdf:resource="http://www.w3.org/2002/07/owl#ObjectProperty"/>
    <rdfs:comment xml:lang="en">Maybe specified as part of the compensate duty action.</rdfs:comment>
    <rdfs:isDefinedBy rdf:resource="http://www.w3.org/ns/odrl/2/"/>
    <rdfs:label xml:lang="en">payee party</rdfs:label>
    <rdfs:subPropertyOf rdf:resource="http://www.w3.org/ns/odrl/2/function"/>
    <skos:definition xml:lang="en">The Party is the recipient of the compensation.</skos:definition>
  </rdf:Property>
  <Action rdf:about="http://www.w3.org/ns/odrl/2/concurrentUse">
    <rdf:type rdf:resource="http://www.w3.org/2004/02/skos/core#Concept"/>
    <rdfs:isDefinedBy rdf:resource="http://www.w3.org/ns/odrl/2/"/>
    <rdfs:label xml:lang="en">Concurrent use</rdfs:label>
    <skos:broaderTransitive rdf:resource="http://www.w3.org/ns/odrl/2/use"/>
    <skos:definition xml:lang="en">The Assigner permits/prohibits the Assignees to create multiple copies of the Asset that are being concurrently used.</skos:definition>
  </Action>
  <rdf:Property rdf:about="http://www.w3.org/ns/odrl/2/conflict">
    <rdf:type rdf:resource="http://www.w3.org/2002/07/owl#ObjectProperty"/>
    <rdfs:comment xml:lang="en">If no mechanism is specified, the default is invalid.</rdfs:comment>
    <rdfs:domain rdf:resource="http://www.w3.org/ns/odrl/2/Policy"/>
    <rdfs:isDefinedBy rdf:resource="http://www.w3.org/ns/odrl/2/"/>
    <rdfs:label xml:lang="en">conflict</rdfs:label>
    <rdfs:range rdf:resource="http://www.w3.org/ns/odrl/2/ConflictTerm"/>
    <skos:definition xml:lang="en">Relates a conflict-resolution mechansim to a Policy.</skos:definition>
  </rdf:Property>
  <rdf:Property rdf:about="http://www.w3.org/ns/odrl/2/consentingParty">
    <rdf:type rdf:resource="http://www.w3.org/2002/07/owl#ObjectProperty"/>
    <rdfs:comment xml:lang="en">Maybe specified as part of the obtainConsent action.</rdfs:comment>
    <rdfs:isDefinedBy rdf:resource="http://www.w3.org/ns/odrl/2/"/>
    <rdfs:label xml:lang="en">consenting party</rdfs:label>
    <rdfs:subPropertyOf rdf:resource="http://www.w3.org/ns/odrl/2/function"/>
    <skos:definition xml:lang="en">The Party to obtain consent from.</skos:definition>
  </rdf:Property>
  <rdf:Property rdf:about="http://www.w3.org/ns/odrl/2/constraint">
    <rdf:type rdf:resource="http://www.w3.org/2002/07/owl#ObjectProperty"/>
    <rdfs:comment xml:lang="en">One or more constraints which affect the validity of the Rule; e.g. if the Action play is only permitted for a certain period of time.</rdfs:comment>
    <rdfs:domain rdf:resource="http://www.w3.org/ns/odrl/2/Rule"/>
    <rdfs:isDefinedBy rdf:resource="http://www.w3.org/ns/odrl/2/"/>
    <rdfs:label xml:lang="en">constraint</rdfs:label>
    <rdfs:range rdf:resource="http://www.w3.org/ns/odrl/2/Constraint"/>
    <skos:definition xml:lang="en">The constraint relating to the Rule</skos:definition>
  </rdf:Property>
  <Action rdf:about="http://www.w3.org/ns/odrl/2/copy">
    <ont:deprecatedBy rdf:resource="http://www.w3.org/ns/odrl/2/reproduce"/>
    <rdf:type rdf:resource="http://www.w3.org/2004/02/skos/core#Concept"/>
    <rdfs:isDefinedBy rdf:resource="http://www.w3.org/ns/odrl/2/"/>
    <rdfs:label xml:lang="en">Copy</rdfs:label>
    <owl:sameAs rdf:resource="http://www.w3.org/ns/odrl/2/reproduce"/>
    <skos:definition xml:lang="en">The act of making an exact reproduction of the asset.</skos:definition>
  </Action>
  <rdf:Property rdf:about="http://www.w3.org/ns/odrl/2/count">
    <rdf:type rdf:resource="http://www.w3.org/2002/07/owl#DatatypeProperty"/>
    <rdfs:comment xml:lang="en">Should be a positive integer</rdfs:comment>
    <rdfs:isDefinedBy rdf:resource="http://www.w3.org/ns/odrl/2/"/>
    <rdfs:label xml:lang="en">count</rdfs:label>
    <rdfs:range rdf:resource="http://www.w3.org/2001/XMLSchema#nonNegativeInteger"/>
    <rdfs:subPropertyOf rdf:resource="http://www.w3.org/ns/odrl/2/rightOperand"/>
    <skos:definition xml:lang="en">The numeric count indicating the number of times the corresponding entity may be exercised</skos:definition>
  </rdf:Property>
  <rdf:Property rdf:about="http://www.w3.org/ns/odrl/2/dataType">
    <rdfs:domain rdf:resource="http://www.w3.org/ns/odrl/2/Constraint"/>
    <rdfs:isDefinedBy rdf:resource="http://www.w3.org/ns/odrl/2/"/>
    <rdfs:label xml:lang="en">unit</rdfs:label>
    <rdfs:range rdf:resource="http://www.w3.org/2000/01/rdf-schema#Resource"/>
    <skos:definition xml:lang="en">The datatype used for the constraint value.</skos:definition>
  </rdf:Property>
  <rdf:Property rdf:about="http://www.w3.org/ns/odrl/2/dateTime">
    <rdf:type rdf:resource="http://www.w3.org/2002/07/owl#DatatypeProperty"/>
    <rdfs:comment xml:lang="en">Value must conform to [iso8601] as represented in [xmlschema11-2]. The use of Timezone information is strongly recommended.</rdfs:comment>
    <rdfs:isDefinedBy rdf:resource="http://www.w3.org/ns/odrl/2/"/>
    <rdfs:label xml:lang="en">date/time</rdfs:label>
    <rdfs:range>
      <owl:Class>
        <owl:unionOf>
          <rdf:Description>
            <rdf:first rdf:resource="http://www.w3.org/2001/XMLSchema#date"/>
            <rdf:rest>
              <rdf:Description>
                <rdf:first rdf:resource="http://www.w3.org/2001/XMLSchema#dateTime"/>
                <rdf:rest rdf:resource="http://www.w3.org/1999/02/22-rdf-syntax-ns#nil"/>
              </rdf:Description>
            </rdf:rest>
          </rdf:Description>
        </owl:unionOf>
      </owl:Class>
    </rdfs:range>
    <rdfs:subPropertyOf rdf:resource="http://www.w3.org/ns/odrl/2/rightOperand"/>
    <skos:definition xml:lang="en">The date (and optional time and timezone) representing a point in time or period.</skos:definition>
  </rdf:Property>
  <Action rdf:about="http://www.w3.org/ns/odrl/2/delete">
    <rdf:type rdf:resource="http://www.w3.org/2004/02/skos/core#Concept"/>
    <rdfs:comment xml:lang="en">Use a constraint to define under which conditions the Asset should be deleted.</rdfs:comment>
    <rdfs:isDefinedBy rdf:resource="http://www.w3.org/ns/odrl/2/"/>
    <rdfs:label xml:lang="en">Delete</rdfs:label>
    <skos:definition xml:lang="en">The Assigner requires that the Assignees permanently removes all copies of the Asset.</skos:definition>
  </Action>
  <rdf:Property rdf:about="http://www.w3.org/ns/odrl/2/deliveryChannel">
    <rdf:type rdf:resource="http://www.w3.org/2002/07/owl#ObjectProperty"/>
    <rdfs:comment xml:lang="en">For example, the asset may be distributed only on mobile networks.</rdfs:comment>
    <rdfs:isDefinedBy rdf:resource="http://www.w3.org/ns/odrl/2/"/>
    <rdfs:label xml:lang="en">delivery channel</rdfs:label>
    <rdfs:subPropertyOf rdf:resource="http://www.w3.org/ns/odrl/2/rightOperand"/>
    <skos:definition xml:lang="en">The delivery channel used for storing or communicating the asset.</skos:definition>
  </rdf:Property>
  <Action rdf:about="http://www.w3.org/ns/odrl/2/derive">
    <rdf:type rdf:resource="http://www.w3.org/2004/02/skos/core#Concept"/>
    <rdfs:comment xml:lang="en">A new asset is created and may have significant overlaps with the original Asset. (Note that the notion of whether or not the change is significant enough to qualify as a new asset is subjective). To the derived Asset a next policy may be applied.</rdfs:comment>
    <rdfs:isDefinedBy rdf:resource="http://www.w3.org/ns/odrl/2/"/>
    <rdfs:label xml:lang="en">Derive</rdfs:label>
    <skos:broaderTransitive rdf:resource="http://www.w3.org/ns/odrl/2/use"/>
    <skos:definition xml:lang="en">The Assigner permits/prohibits the Assignees to create a new derivative Asset from this Asset and to edit or modify the derivative.</skos:definition>
  </Action>
  <rdf:Property rdf:about="http://www.w3.org/ns/odrl/2/device">
    <ont:deprecatedBy rdf:resource="http://www.w3.org/ns/odrl/2/systemDevice"/>
    <rdf:type rdf:resource="http://www.w3.org/2002/07/owl#ObjectProperty"/>
    <rdfs:isDefinedBy rdf:resource="http://www.w3.org/ns/odrl/2/"/>
    <rdfs:label xml:lang="en">device</rdfs:label>
    <rdfs:subPropertyOf rdf:resource="http://www.w3.org/ns/odrl/2/rightOperand"/>
    <owl:equivalentProperty rdf:resource="http://www.w3.org/ns/odrl/2/system"/>
    <skos:definition xml:lang="en">An identifiable computing system.</skos:definition>
  </rdf:Property>
  <Action rdf:about="http://www.w3.org/ns/odrl/2/digitize">
    <rdf:type rdf:resource="http://www.w3.org/2004/02/skos/core#Concept"/>
    <rdfs:isDefinedBy rdf:resource="http://www.w3.org/ns/odrl/2/"/>
    <rdfs:label xml:lang="en">Digitize</rdfs:label>
    <skos:broaderTransitive rdf:resource="http://www.w3.org/ns/odrl/2/use"/>
    <skos:definition xml:lang="en">The Assigner permits/prohibits the Assignees to produce a digital copy of (or otherwise digitize) the Asset from its analogue form.</skos:definition>
  </Action>
  <Action rdf:about="http://www.w3.org/ns/odrl/2/display">
    <rdf:type rdf:resource="http://www.w3.org/2004/02/skos/core#Concept"/>
    <rdfs:comment xml:lang="en">For example, displaying an image on a screen.</rdfs:comment>
    <rdfs:isDefinedBy rdf:resource="http://www.w3.org/ns/odrl/2/"/>
    <rdfs:label xml:lang="en">Display</rdfs:label>
    <skos:broaderTransitive rdf:resource="http://www.w3.org/ns/odrl/2/present"/>
    <skos:definition xml:lang="en">The Assigner permits/prohibits the Assignees to display the visual media Asset to an audience or the public.</skos:definition>
  </Action>
  <Action rdf:about="http://www.w3.org/ns/odrl/2/distribute">
    <rdf:type rdf:resource="http://www.w3.org/2004/02/skos/core#Concept"/>
    <rdfs:isDefinedBy rdf:resource="http://www.w3.org/ns/odrl/2/"/>
    <rdfs:label xml:lang="en">Distribute</rdfs:label>
    <skos:broaderTransitive rdf:resource="http://www.w3.org/ns/odrl/2/use"/>
    <skos:definition xml:lang="en">The Assigner permits/prohibits the Assignees to distribute the Asset.</skos:definition>
  </Action>
  <rdf:Property rdf:about="http://www.w3.org/ns/odrl/2/duty">
    <rdf:type rdf:resource="http://www.w3.org/2002/07/owl#ObjectProperty"/>
    <rdfs:comment xml:lang="en">A Duty indicates requirements which must be fulfilled in order to receive the permission.</rdfs:comment>
    <rdfs:domain rdf:resource="http://www.w3.org/ns/odrl/2/Permission"/>
    <rdfs:isDefinedBy rdf:resource="http://www.w3.org/ns/odrl/2/"/>
    <rdfs:label xml:lang="en">duty</rdfs:label>
    <rdfs:range>
      <owl:Class>
        <owl:unionOf>
          <rdf:Description>
            <rdf:first rdf:resource="http://www.w3.org/ns/odrl/2/Duty"/>
            <rdf:rest>
              <rdf:Description>
                <rdf:first rdf:resource="http://www.w3.org/ns/odrl/2/Action"/>
                <rdf:rest rdf:resource="http://www.w3.org/1999/02/22-rdf-syntax-ns#nil"/>
              </rdf:Description>
            </rdf:rest>
          </rdf:Description>
        </owl:unionOf>
      </owl:Class>
    </rdfs:range>
    <skos:definition xml:lang="en">The duty relating to the Permission</skos:definition>
  </rdf:Property>
  <rdf:Property rdf:about="http://www.w3.org/ns/odrl/2/elapsedTime">
    <rdf:type rdf:resource="http://www.w3.org/2002/07/owl#DatatypeProperty"/>
    <rdfs:comment xml:lang="en">The start of the period is when the action is first exercised. Value must conform to [iso8601] as represented in [xmlschema11-2].</rdfs:comment>
    <rdfs:isDefinedBy rdf:resource="http://www.w3.org/ns/odrl/2/"/>
    <rdfs:label xml:lang="en">elapsed time</rdfs:label>
    <rdfs:range rdf:resource="http://www.w3.org/2001/XMLSchema#duration"/>
    <rdfs:subPropertyOf rdf:resource="http://www.w3.org/ns/odrl/2/rightOperand"/>
    <skos:definition xml:lang="en">A period of time in which the policy action can be exercised.</skos:definition>
  </rdf:Property>
  <Action rdf:about="http://www.w3.org/ns/odrl/2/ensureExclusivity">
    <rdf:type rdf:resource="http://www.w3.org/2004/02/skos/core#Concept"/>
    <rdfs:isDefinedBy rdf:resource="http://www.w3.org/ns/odrl/2/"/>
    <rdfs:label xml:lang="en">Ensure exclusivity</rdfs:label>
    <skos:definition xml:lang="en">The Assignee requires that the Assigners ensure that the permission on the Asset is exclusive to the Assignee.</skos:definition>
  </Action>
  <Operator rdf:about="http://www.w3.org/ns/odrl/2/eq">
    <rdf:type rdf:resource="http://www.w3.org/2002/07/owl#NamedIndividual"/>
    <rdfs:isDefinedBy rdf:resource="http://www.w3.org/ns/odrl/2/"/>
    <rdfs:label xml:lang="en">Equal to</rdfs:label>
    <skos:definition xml:lang="en">Indicating that a given value equals the right operand of the Constraint.</skos:definition>
  </Operator>
  <rdf:Property rdf:about="http://www.w3.org/ns/odrl/2/event">
    <rdf:type rdf:resource="http://www.w3.org/2002/07/owl#ObjectProperty"/>
    <rdfs:comment xml:lang="en">For example, asset may be used at the “FIFA World Cup” only. To express events related to undertaking Duties, specific event values may be defined (eg see policyUsage).</rdfs:comment>
    <rdfs:isDefinedBy rdf:resource="http://www.w3.org/ns/odrl/2/"/>
    <rdfs:label xml:lang="en">event</rdfs:label>
    <rdfs:subPropertyOf rdf:resource="http://www.w3.org/ns/odrl/2/rightOperand"/>
    <skos:definition xml:lang="en">Specification of a defined event applicable to the asset usage.</skos:definition>
  </rdf:Property>
  <Action rdf:about="http://www.w3.org/ns/odrl/2/execute">
    <rdf:type rdf:resource="http://www.w3.org/2004/02/skos/core#Concept"/>
    <rdfs:comment xml:lang="en">For example, machine executable code or Java such as a game or application.</rdfs:comment>
    <rdfs:isDefinedBy rdf:resource="http://www.w3.org/ns/odrl/2/"/>
    <rdfs:label xml:lang="en">Execute</rdfs:label>
    <skos:broaderTransitive rdf:resource="http://www.w3.org/ns/odrl/2/use"/>
    <skos:definition xml:lang="en">The Assigner permits/prohibits the Assignees to run the computer program Asset.</skos:definition>
  </Action>
  <Action rdf:about="http://www.w3.org/ns/odrl/2/export">
    <ont:deprecatedBy rdf:resource="http://www.w3.org/ns/odrl/2/transform"/>
    <rdf:type rdf:resource="http://www.w3.org/2004/02/skos/core#Concept"/>
    <rdfs:isDefinedBy rdf:resource="http://www.w3.org/ns/odrl/2/"/>
    <rdfs:label xml:lang="en">Export</rdfs:label>
    <skos:definition xml:lang="en">The act of transforming the asset into a new form.</skos:definition>
  </Action>
  <Action rdf:about="http://www.w3.org/ns/odrl/2/extract">
    <rdf:type rdf:resource="http://www.w3.org/2004/02/skos/core#Concept"/>
    <rdfs:comment xml:lang="en">A new asset is created and may have very little in common with the original Asset. (Note that the notion of whether or not the change is significant enough to qualify as a new asset is subjective). To the extracted Asset a next policy may be applied.</rdfs:comment>
    <rdfs:isDefinedBy rdf:resource="http://www.w3.org/ns/odrl/2/"/>
    <rdfs:label xml:lang="en">Extract</rdfs:label>
    <skos:broaderTransitive rdf:resource="http://www.w3.org/ns/odrl/2/reproduce"/>
    <skos:definition xml:lang="en">The Assigner permits/prohibits the Assignees to extract parts of the Asset and to use it as a new Asset.</skos:definition>
  </Action>
  <Action rdf:about="http://www.w3.org/ns/odrl/2/extractChar">
    <ont:deprecatedBy rdf:resource="http://www.editeur.org/onix-pl/extract-char"/>
    <rdf:type rdf:resource="http://www.w3.org/2004/02/skos/core#Concept"/>
    <rdfs:isDefinedBy rdf:resource="http://www.w3.org/ns/odrl/2/"/>
    <rdfs:label xml:lang="en">Extract character</rdfs:label>
    <skos:broader rdf:resource="http://www.w3.org/ns/odrl/2/extract"/>
    <skos:definition xml:lang="en">The act of extracting (replicating) unchanged characters from the asset.</skos:definition>
  </Action>
  <Action rdf:about="http://www.w3.org/ns/odrl/2/extractPage">
    <ont:deprecatedBy rdf:resource="http://www.editeur.org/onix-pl/extract-word"/>
    <rdf:type rdf:resource="http://www.w3.org/2004/02/skos/core#Concept"/>
    <rdfs:isDefinedBy rdf:resource="http://www.w3.org/ns/odrl/2/"/>
    <rdfs:label xml:lang="en">Extract page</rdfs:label>
    <skos:broader rdf:resource="http://www.w3.org/ns/odrl/2/extract"/>
    <skos:definition xml:lang="en">The act of extracting (replicating) unchanged pages from the asset.</skos:definition>
  </Action>
  <Action rdf:about="http://www.w3.org/ns/odrl/2/extractWord">
    <ont:deprecatedBy rdf:resource="http://www.editeur.org/onix-pl/extract-page"/>
    <rdf:type rdf:resource="http://www.w3.org/2004/02/skos/core#Concept"/>
    <rdfs:isDefinedBy rdf:resource="http://www.w3.org/ns/odrl/2/"/>
    <rdfs:label xml:lang="en">Extract word</rdfs:label>
    <skos:broader rdf:resource="http://www.w3.org/ns/odrl/2/extract"/>
    <skos:definition xml:lang="en">The act of extracting (replicating) unchanged words from the asset.</skos:definition>
  </Action>
  <rdf:Property rdf:about="http://www.w3.org/ns/odrl/2/fileFormat">
    <rdf:type rdf:resource="http://www.w3.org/2002/07/owl#ObjectProperty"/>
    <rdfs:comment xml:lang="en">For example only JPEG image may be distributed. This may be used to express [[plus]] semantics.</rdfs:comment>
    <rdfs:isDefinedBy rdf:resource="http://www.w3.org/ns/odrl/2/"/>
    <rdfs:label xml:lang="en">file format</rdfs:label>
    <rdfs:subPropertyOf rdf:resource="http://www.w3.org/ns/odrl/2/rightOperand"/>
    <skos:definition xml:lang="en">The file format applicable to the Asset.</skos:definition>
  </rdf:Property>
  <rdf:Property rdf:about="http://www.w3.org/ns/odrl/2/function">
    <rdf:type rdf:resource="http://www.w3.org/2002/07/owl#ObjectProperty"/>
    <rdfs:domain rdf:resource="http://www.w3.org/ns/odrl/2/Rule"/>
    <rdfs:isDefinedBy rdf:resource="http://www.w3.org/ns/odrl/2/"/>
    <rdfs:label xml:lang="en">function</rdfs:label>
    <rdfs:range rdf:resource="http://www.w3.org/ns/odrl/2/Party"/>
    <skos:definition xml:lang="en">Function is an abstract property whose sub-properties define the roles which may be fulfilled by a party in relation to a Rule</skos:definition>
  </rdf:Property>
  <Action rdf:about="http://www.w3.org/ns/odrl/2/give">
    <rdf:type rdf:resource="http://www.w3.org/2004/02/skos/core#Concept"/>
    <rdfs:isDefinedBy rdf:resource="http://www.w3.org/ns/odrl/2/"/>
    <rdfs:label xml:lang="en">Give</rdfs:label>
    <skos:broaderTransitive rdf:resource="http://www.w3.org/ns/odrl/2/transfer"/>
    <skos:definition xml:lang="en">The Assigner permits/prohibits the Assignees to transfer the ownership of the Asset to a third party without compensation and while deleting the original asset.</skos:definition>
  </Action>
  <Action rdf:about="http://www.w3.org/ns/odrl/2/grantUse">
    <rdf:type rdf:resource="http://www.w3.org/2004/02/skos/core#Concept"/>
    <rdfs:comment xml:lang="en">This action enables the Assignee to create policies for the use of the Asset for third parties. nextPolicy is recommended to be agreed with the third party. Use of temporal constraints is recommended.</rdfs:comment>
    <rdfs:isDefinedBy rdf:resource="http://www.w3.org/ns/odrl/2/"/>
    <rdfs:label xml:lang="en">Grant use</rdfs:label>
    <skos:broaderTransitive rdf:resource="http://www.w3.org/ns/odrl/2/use"/>
    <skos:definition xml:lang="en">The Assigner permits/prohibits the Assignee to grant the use the Asset to third parties.</skos:definition>
  </Action>
  <Operator rdf:about="http://www.w3.org/ns/odrl/2/gt">
    <rdf:type rdf:resource="http://www.w3.org/2002/07/owl#NamedIndividual"/>
    <rdfs:isDefinedBy rdf:resource="http://www.w3.org/ns/odrl/2/"/>
    <rdfs:label xml:lang="en">Greater than</rdfs:label>
    <skos:definition xml:lang="en">Indicating that a given value is greater than the right operand of the Constraint</skos:definition>
  </Operator>
  <Operator rdf:about="http://www.w3.org/ns/odrl/2/gteq">
    <rdf:type rdf:resource="http://www.w3.org/2002/07/owl#NamedIndividual"/>
    <rdfs:isDefinedBy rdf:resource="http://www.w3.org/ns/odrl/2/"/>
    <rdfs:label xml:lang="en">Greater than or equal to</rdfs:label>
    <skos:definition xml:lang="en">Indicating that a given value is greater than or equal to the right operand of the Constraint</skos:definition>
  </Operator>
  <Operator rdf:about="http://www.w3.org/ns/odrl/2/hasPart">
    <rdf:type rdf:resource="http://www.w3.org/2002/07/owl#NamedIndividual"/>
    <rdfs:isDefinedBy rdf:resource="http://www.w3.org/ns/odrl/2/"/>
    <rdfs:label xml:lang="en">Has part</rdfs:label>
    <skos:definition xml:lang="en">Indicating that a given value contains the right operand of the Constraint</skos:definition>
  </Operator>
  <UndefinedTerm rdf:about="http://www.w3.org/ns/odrl/2/ignore">
    <rdf:type rdf:resource="http://www.w3.org/2002/07/owl#NamedIndividual"/>
    <rdfs:comment xml:lang="en">Used to support actions not known to the policy system.</rdfs:comment>
    <rdfs:isDefinedBy rdf:resource="http://www.w3.org/ns/odrl/2/"/>
    <rdfs:label xml:lang="en">Ignore</rdfs:label>
    <skos:definition xml:lang="en">The Action is to be ignored and not part of the policy – and the policy remains valid.</skos:definition>
  </UndefinedTerm>
  <Action rdf:about="http://www.w3.org/ns/odrl/2/include">
    <rdf:type rdf:resource="http://www.w3.org/2004/02/skos/core#Concept"/>
    <rdfs:comment xml:lang="en">For example: bio picture must be included in the attribution. Use of the Asset relation attribute is required.</rdfs:comment>
    <rdfs:isDefinedBy rdf:resource="http://www.w3.org/ns/odrl/2/"/>
    <rdfs:label xml:lang="en">Include</rdfs:label>
    <skos:definition xml:lang="en">The Assigner requires that the Assignees include other related assets in the Asset.</skos:definition>
  </Action>
  <Action rdf:about="http://www.w3.org/ns/odrl/2/index">
    <rdf:type rdf:resource="http://www.w3.org/2004/02/skos/core#Concept"/>
    <rdfs:comment xml:lang="en">For example, to include a link to the Asset in a search engine database.</rdfs:comment>
    <rdfs:isDefinedBy rdf:resource="http://www.w3.org/ns/odrl/2/"/>
    <rdfs:label xml:lang="en">Index</rdfs:label>
    <skos:broaderTransitive rdf:resource="http://www.w3.org/ns/odrl/2/use"/>
    <skos:definition xml:lang="en">The Assigner permits/prohibits the Assignees to record the Asset in an index.</skos:definition>
  </Action>
  <rdf:Property rdf:about="http://www.w3.org/ns/odrl/2/industry">
    <rdf:type rdf:resource="http://www.w3.org/2002/07/owl#DatatypeProperty"/>
    <rdfs:comment xml:lang="en">For example, publishing, financial.</rdfs:comment>
    <rdfs:isDefinedBy rdf:resource="http://www.w3.org/ns/odrl/2/"/>
    <rdfs:label xml:lang="en">industry</rdfs:label>
    <rdfs:subPropertyOf rdf:resource="http://www.w3.org/ns/odrl/2/rightOperand"/>
    <skos:definition xml:lang="en">The defined industry sector applicable to the asset usage.</skos:definition>
  </rdf:Property>
  <Action rdf:about="http://www.w3.org/ns/odrl/2/inform">
    <rdf:type rdf:resource="http://www.w3.org/2004/02/skos/core#Concept"/>
    <rdfs:comment xml:lang="en">May link to a Party with the role function “informedParty”.</rdfs:comment>
    <rdfs:isDefinedBy rdf:resource="http://www.w3.org/ns/odrl/2/"/>
    <rdfs:label xml:lang="en">Inform</rdfs:label>
    <skos:definition xml:lang="en">The Assigner requires that the Assignees inform the Assigner or an informed Party that an action has been performed on or in relation to the Asset.</skos:definition>
  </Action>
  <rdf:Property rdf:about="http://www.w3.org/ns/odrl/2/informedParty">
    <rdf:type rdf:resource="http://www.w3.org/2002/07/owl#ObjectProperty"/>
    <rdfs:comment xml:lang="en">Maybe specified as part of the inform action.</rdfs:comment>
    <rdfs:isDefinedBy rdf:resource="http://www.w3.org/ns/odrl/2/"/>
    <rdfs:label xml:lang="en">informed party</rdfs:label>
    <rdfs:subPropertyOf rdf:resource="http://www.w3.org/ns/odrl/2/function"/>
    <skos:definition xml:lang="en">The Party to be informed of all uses.</skos:definition>
  </rdf:Property>
  <rdf:Property rdf:about="http://www.w3.org/ns/odrl/2/inheritAllowed">
    <rdf:type rdf:resource="http://www.w3.org/2002/07/owl#DatatypeProperty"/>
    <rdfs:comment xml:lang="en">A boolean value.</rdfs:comment>
    <rdfs:domain rdf:resource="http://www.w3.org/ns/odrl/2/Policy"/>
    <rdfs:isDefinedBy rdf:resource="http://www.w3.org/ns/odrl/2/"/>
    <rdfs:label xml:lang="en">inheritance allowed</rdfs:label>
    <rdfs:range rdf:resource="http://www.w3.org/2001/XMLSchema#boolean"/>
    <skos:definition xml:lang="en">Indicates if the Policy entity can be inherited.</skos:definition>
  </rdf:Property>
  <rdf:Property rdf:about="http://www.w3.org/ns/odrl/2/inheritFrom">
    <rdf:type rdf:resource="http://www.w3.org/2002/07/owl#ObjectProperty"/>
    <rdfs:comment xml:lang="en">The child policy will inherit from the parent policy</rdfs:comment>
    <rdfs:domain rdf:resource="http://www.w3.org/ns/odrl/2/Policy"/>
    <rdfs:isDefinedBy rdf:resource="http://www.w3.org/ns/odrl/2/"/>
    <rdfs:label xml:lang="en">inherits from</rdfs:label>
    <rdfs:range rdf:resource="http://www.w3.org/ns/odrl/2/Policy"/>
    <skos:definition xml:lang="en">Relates a (child) policy to another (parent) policy from which terms are inherited</skos:definition>
  </rdf:Property>
  <Action rdf:about="http://www.w3.org/ns/odrl/2/install">
    <rdf:type rdf:resource="http://www.w3.org/2004/02/skos/core#Concept"/>
    <rdfs:isDefinedBy rdf:resource="http://www.w3.org/ns/odrl/2/"/>
    <rdfs:label xml:lang="en">Install</rdfs:label>
    <skos:broaderTransitive rdf:resource="http://www.w3.org/ns/odrl/2/use"/>
    <skos:definition xml:lang="en">The Assigner permits/prohibits the Assignees to load the computer program Asset onto a storage device which allows operating or running the Asset.</skos:definition>
  </Action>
  <ConflictTerm rdf:about="http://www.w3.org/ns/odrl/2/invalid">
    <rdf:type rdf:resource="http://www.w3.org/2002/07/owl#NamedIndividual"/>
    <rdf:type rdf:resource="http://www.w3.org/ns/odrl/2/UndefinedTerm"/>
    <rdfs:comment xml:lang="en">Used to support actions not known to the policy system.</rdfs:comment>
    <rdfs:isDefinedBy rdf:resource="http://www.w3.org/ns/odrl/2/"/>
    <rdfs:label xml:lang="en">Invalid</rdfs:label>
    <skos:definition xml:lang="en">the Action is unknown – and the policy is invalid.</skos:definition>
  </ConflictTerm>
  <Operator rdf:about="http://www.w3.org/ns/odrl/2/isA">
    <rdf:type rdf:resource="http://www.w3.org/2002/07/owl#NamedIndividual"/>
    <rdfs:isDefinedBy rdf:resource="http://www.w3.org/ns/odrl/2/"/>
    <rdfs:label xml:lang="en">Is a</rdfs:label>
    <skos:definition xml:lang="en">Indicating that a given value is an instance of the right operand of the Constraint</skos:definition>
  </Operator>
  <Operator rdf:about="http://www.w3.org/ns/odrl/2/isAllOf">
    <rdf:type rdf:resource="http://www.w3.org/2002/07/owl#NamedIndividual"/>
    <rdfs:isDefinedBy rdf:resource="http://www.w3.org/ns/odrl/2/"/>
    <rdfs:label xml:lang="en">Is all of</rdfs:label>
    <skos:definition xml:lang="en">Indicating that a given value is all of the right operand of the Constraint</skos:definition>
  </Operator>
  <Operator rdf:about="http://www.w3.org/ns/odrl/2/isAnyOf">
    <rdf:type rdf:resource="http://www.w3.org/2002/07/owl#NamedIndividual"/>
    <rdfs:isDefinedBy rdf:resource="http://www.w3.org/ns/odrl/2/"/>
    <rdfs:label xml:lang="en">Is any of</rdfs:label>
    <skos:definition xml:lang="en">Indicating that a given value is any of the right operand of the Constraint</skos:definition>
  </Operator>
  <Operator rdf:about="http://www.w3.org/ns/odrl/2/isNoneOf">
    <rdf:type rdf:resource="http://www.w3.org/2002/07/owl#NamedIndividual"/>
    <rdfs:isDefinedBy rdf:resource="http://www.w3.org/ns/odrl/2/"/>
    <rdfs:label xml:lang="en">Is none of</rdfs:label>
    <skos:definition xml:lang="en">Indicating that a given value is none of the right operand of the Constraint</skos:definition>
  </Operator>
  <Operator rdf:about="http://www.w3.org/ns/odrl/2/isPartOf">
    <rdf:type rdf:resource="http://www.w3.org/2002/07/owl#NamedIndividual"/>
    <rdfs:isDefinedBy rdf:resource="http://www.w3.org/ns/odrl/2/"/>
    <rdfs:label xml:lang="en">Is part of</rdfs:label>
    <skos:definition xml:lang="en">Indicating that a given value is contained by the right operand of the Constraint</skos:definition>
  </Operator>
  <rdf:Property rdf:about="http://www.w3.org/ns/odrl/2/language">
    <rdf:type rdf:resource="http://www.w3.org/2002/07/owl#DatatypeProperty"/>
    <rdfs:comment xml:lang="en">For example, JPEG image may only be reproduced with Spanish text. May be used to express [[plus] semantics. Must use [bcp47] codes for language values.</rdfs:comment>
    <rdfs:isDefinedBy rdf:resource="http://www.w3.org/ns/odrl/2/"/>
    <rdfs:label xml:lang="en">language</rdfs:label>
    <rdfs:subPropertyOf rdf:resource="http://www.w3.org/ns/odrl/2/rightOperand"/>
    <skos:definition xml:lang="en">The natural language applicable to the asset usage</skos:definition>
  </rdf:Property>
  <Action rdf:about="http://www.w3.org/ns/odrl/2/lease">
    <ont:deprecatedBy rdf:resource="http://www.w3.org/1999/02/22-rdf-syntax-ns#nil"/>
    <rdf:type rdf:resource="http://www.w3.org/2004/02/skos/core#Concept"/>
    <rdfs:isDefinedBy rdf:resource="http://www.w3.org/ns/odrl/2/"/>
    <rdfs:label xml:lang="en">Lease</rdfs:label>
    <skos:definition xml:lang="en">The act of making available the asset to a third-party for a fixed period of time with exchange of value.</skos:definition>
  </Action>
  <Action rdf:about="http://www.w3.org/ns/odrl/2/lend">
    <ont:deprecatedBy rdf:resource="http://www.w3.org/1999/02/22-rdf-syntax-ns#nil"/>
    <rdf:type rdf:resource="http://www.w3.org/2004/02/skos/core#Concept"/>
    <rdfs:isDefinedBy rdf:resource="http://www.w3.org/ns/odrl/2/"/>
    <rdfs:label xml:lang="en">Lend</rdfs:label>
    <skos:definition xml:lang="en">The act of making available the asset to a third-party for a fixed period of time without exchange of value.</skos:definition>
  </Action>
  <Action rdf:about="http://www.w3.org/ns/odrl/2/license">
    <ont:deprecatedBy rdf:resource="http://www.w3.org/ns/odrl/2/grantUse"/>
    <rdf:type rdf:resource="http://www.w3.org/2004/02/skos/core#Concept"/>
    <rdfs:isDefinedBy rdf:resource="http://www.w3.org/ns/odrl/2/"/>
    <rdfs:label xml:lang="en">License</rdfs:label>
    <skos:definition xml:lang="en">The act of granting the right to use the asset to a third-party.</skos:definition>
  </Action>
  <Operator rdf:about="http://www.w3.org/ns/odrl/2/lt">
    <rdf:type rdf:resource="http://www.w3.org/2002/07/owl#NamedIndividual"/>
    <rdfs:isDefinedBy rdf:resource="http://www.w3.org/ns/odrl/2/"/>
    <rdfs:label xml:lang="en">Less than</rdfs:label>
    <skos:definition xml:lang="en">Indicating that a given value is less than the right operand of the Constraint</skos:definition>
  </Operator>
  <Operator rdf:about="http://www.w3.org/ns/odrl/2/lteq">
    <rdf:type rdf:resource="http://www.w3.org/2002/07/owl#NamedIndividual"/>
    <rdfs:isDefinedBy rdf:resource="http://www.w3.org/ns/odrl/2/"/>
    <rdfs:label xml:lang="en">Less than or equal to</rdfs:label>
    <skos:definition xml:lang="en">Indicating that a given value is less than or equal to the right operand of the Constraint</skos:definition>
  </Operator>
  <rdf:Property rdf:about="http://www.w3.org/ns/odrl/2/media">
    <rdfs:comment xml:lang="en">For example, electronic, print, advertising, marketing. This may be used to express [[plus]] semantics.</rdfs:comment>
    <rdfs:isDefinedBy rdf:resource="http://www.w3.org/ns/odrl/2/"/>
    <rdfs:label xml:lang="en">media</rdfs:label>
    <rdfs:subPropertyOf rdf:resource="http://www.w3.org/ns/odrl/2/rightOperand"/>
    <skos:definition xml:lang="en">The media type in which the asset may be used.</skos:definition>
  </rdf:Property>
  <rdf:Property rdf:about="http://www.w3.org/ns/odrl/2/meteredTime">
    <rdf:type rdf:resource="http://www.w3.org/2002/07/owl#DatatypeProperty"/>
    <rdfs:comment xml:lang="en">For example “P30H” indicates a 30 hour period. Value must conform to [iso8601] as represented in [xmlschema11-2].</rdfs:comment>
    <rdfs:isDefinedBy rdf:resource="http://www.w3.org/ns/odrl/2/"/>
    <rdfs:label xml:lang="en">metered time</rdfs:label>
    <rdfs:range rdf:resource="http://www.w3.org/2001/XMLSchema#duration"/>
    <rdfs:subPropertyOf rdf:resource="http://www.w3.org/ns/odrl/2/rightOperand"/>
    <skos:definition xml:lang="en">The maximum period of metered usage time.</skos:definition>
  </rdf:Property>
  <Action rdf:about="http://www.w3.org/ns/odrl/2/modify">
    <rdf:type rdf:resource="http://www.w3.org/2004/02/skos/core#Concept"/>
    <rdfs:comment xml:lang="en">This action will modify an asset which is typically updated from time to time without creating a new asset like a database. If the result from modifying the asset should be a new asset the actions derive or extract should be used. (Note that the notion of whether or not the change is significant enough to qualify as a new asset is subjective).</rdfs:comment>
    <rdfs:isDefinedBy rdf:resource="http://www.w3.org/ns/odrl/2/"/>
    <rdfs:label xml:lang="en">Modify</rdfs:label>
    <skos:broaderTransitive rdf:resource="http://www.w3.org/ns/odrl/2/use"/>
    <skos:definition xml:lang="en">The Assigner permits/prohibits the Assignees to update existing content of the Asset. A new asset is not created by this action.</skos:definition>
  </Action>
  <Action rdf:about="http://www.w3.org/ns/odrl/2/move">
    <rdf:type rdf:resource="http://www.w3.org/2004/02/skos/core#Concept"/>
    <rdfs:comment xml:lang="en">After the Asset has been moved, the original copy must be deleted.</rdfs:comment>
    <rdfs:isDefinedBy rdf:resource="http://www.w3.org/ns/odrl/2/"/>
    <rdfs:label xml:lang="en">Move</rdfs:label>
    <skos:broaderTransitive rdf:resource="http://www.w3.org/ns/odrl/2/use"/>
    <skos:definition xml:lang="en">The Assigner permits/prohibits the Assignees to move the Asset from one digital location to another including deleting the original copy.</skos:definition>
  </Action>
  <Operator rdf:about="http://www.w3.org/ns/odrl/2/neq">
    <rdf:type rdf:resource="http://www.w3.org/2002/07/owl#NamedIndividual"/>
    <rdfs:isDefinedBy rdf:resource="http://www.w3.org/ns/odrl/2/"/>
    <rdfs:label xml:lang="en">Not equal to</rdfs:label>
    <skos:definition xml:lang="en">Indicating that a given value is not equal to the right operand of the Constraint</skos:definition>
  </Operator>
  <Action rdf:about="http://www.w3.org/ns/odrl/2/nextPolicy">
    <rdf:type rdf:resource="http://www.w3.org/2004/02/skos/core#Concept"/>
    <rdfs:comment xml:lang="en">Useful for downstream policies.</rdfs:comment>
    <rdfs:isDefinedBy rdf:resource="http://www.w3.org/ns/odrl/2/"/>
    <rdfs:label xml:lang="en">Next policy</rdfs:label>
    <skos:definition xml:lang="en">The Assigner requires that the Assignees grants the specified Policy to a third party for their use of the Asset.</skos:definition>
  </Action>
  <Action rdf:about="http://www.w3.org/ns/odrl/2/obtainConsent">
    <rdf:type rdf:resource="http://www.w3.org/2004/02/skos/core#Concept"/>
    <rdfs:comment xml:lang="en">Used as a Duty to ensure that the Assigner or a Party is authorized to approve such actions on a case-by-case basis. May link to a Party with the role function “consentingParty”.</rdfs:comment>
    <rdfs:isDefinedBy rdf:resource="http://www.w3.org/ns/odrl/2/"/>
    <rdfs:label xml:lang="en">Obtain consent</rdfs:label>
    <skos:definition xml:lang="en">The Assigner requires that the Assignees obtains explicit consent from the Assigner or a consenting Party to perform the requested action in relation to the Asset.</skos:definition>
  </Action>
  <rdf:Property rdf:about="http://www.w3.org/ns/odrl/2/operator">
    <rdf:type rdf:resource="http://www.w3.org/2002/07/owl#ObjectProperty"/>
    <rdfs:domain rdf:resource="http://www.w3.org/ns/odrl/2/Constraint"/>
    <rdfs:isDefinedBy rdf:resource="http://www.w3.org/ns/odrl/2/"/>
    <rdfs:label xml:lang="en">operator</rdfs:label>
    <rdfs:range rdf:resource="http://www.w3.org/ns/odrl/2/Operator"/>
    <skos:definition xml:lang="en">The Boolean operator applied to a constraint and its operand.</skos:definition>
  </rdf:Property>
  <rdf:Property rdf:about="http://www.w3.org/ns/odrl/2/output">
    <rdf:type rdf:resource="http://www.w3.org/2002/07/owl#ObjectProperty"/>
    <rdfs:domain rdf:resource="http://www.w3.org/ns/odrl/2/Rule"/>
    <rdfs:isDefinedBy rdf:resource="http://www.w3.org/ns/odrl/2/"/>
    <rdfs:label xml:lang="en">output</rdfs:label>
    <rdfs:range rdf:resource="http://www.w3.org/ns/odrl/2/Asset"/>
    <rdfs:subPropertyOf rdf:resource="http://www.w3.org/ns/odrl/2/relation"/>
    <skos:definition xml:lang="en">The output property specifies the Asset which is created from the output of the Action.</skos:definition>
  </rdf:Property>
  <Action rdf:about="http://www.w3.org/ns/odrl/2/pay">
    <ont:deprecatedBy rdf:resource="http://www.w3.org/ns/odrl/2/compensate"/>
    <rdf:type rdf:resource="http://www.w3.org/2004/02/skos/core#Concept"/>
    <rdfs:isDefinedBy rdf:resource="http://www.w3.org/ns/odrl/2/"/>
    <rdfs:label xml:lang="en">Pay</rdfs:label>
    <skos:definition xml:lang="en">The act of paying a financial amount to a party for use of the asset.</skos:definition>
  </Action>
  <rdf:Property rdf:about="http://www.w3.org/ns/odrl/2/payAmount">
    <rdf:type rdf:resource="http://www.w3.org/2002/07/owl#DatatypeProperty"/>
    <rdfs:comment xml:lang="en">Maybe used for compensation duties. The dataType attribute may be used to indicate the type of the value (eg decimal) and the unit attribute to indicate the currency.</rdfs:comment>
    <rdfs:isDefinedBy rdf:resource="http://www.w3.org/ns/odrl/2/"/>
    <rdfs:label xml:lang="en">payment amount</rdfs:label>
    <rdfs:range rdf:resource="http://www.w3.org/2001/XMLSchema#decimal"/>
    <rdfs:subPropertyOf rdf:resource="http://www.w3.org/ns/odrl/2/rightOperand"/>
    <skos:definition xml:lang="en">The value of the financial payment</skos:definition>
  </rdf:Property>
  <rdf:Property rdf:about="http://www.w3.org/ns/odrl/2/payeeParty">
    <ont:deprecatedBy rdf:resource="http://www.w3.org/ns/odrl/2/compensatedParty"/>
    <rdf:type rdf:resource="http://www.w3.org/2002/07/owl#ObjectProperty"/>
    <rdfs:isDefinedBy rdf:resource="http://www.w3.org/ns/odrl/2/"/>
    <rdfs:label xml:lang="en">payee party</rdfs:label>
    <rdfs:subPropertyOf rdf:resource="http://www.w3.org/ns/odrl/2/function"/>
    <skos:definition xml:lang="en">The Party is the recipient of the payment.</skos:definition>
  </rdf:Property>
  <rdf:Property rdf:about="http://www.w3.org/ns/odrl/2/percentage">
    <rdf:type rdf:resource="http://www.w3.org/2002/07/owl#DatatypeProperty"/>
    <rdfs:comment xml:lang="en">A numeric value from 0 to 100. For example, extract a maximum of 50% of the asset</rdfs:comment>
    <rdfs:isDefinedBy rdf:resource="http://www.w3.org/ns/odrl/2/"/>
    <rdfs:label xml:lang="en">percentage</rdfs:label>
    <rdfs:range rdf:resource="http://www.w3.org/2001/XMLSchema#decimal"/>
    <rdfs:subPropertyOf rdf:resource="http://www.w3.org/ns/odrl/2/rightOperand"/>
    <skos:definition xml:lang="en">The amount (as a percentage) of the action applicable to the asset.</skos:definition>
  </rdf:Property>
  <ConflictTerm rdf:about="http://www.w3.org/ns/odrl/2/perm">
    <rdf:type rdf:resource="http://www.w3.org/2002/07/owl#NamedIndividual"/>
    <rdfs:comment xml:lang="en">Used to determine policy conflict outcomes.</rdfs:comment>
    <rdfs:isDefinedBy rdf:resource="http://www.w3.org/ns/odrl/2/"/>
    <rdfs:label xml:lang="en">Permissions</rdfs:label>
    <skos:definition xml:lang="en">Permissions take precedence over prohibitions.</skos:definition>
  </ConflictTerm>
  <rdf:Property rdf:about="http://www.w3.org/ns/odrl/2/permission">
    <rdf:type rdf:resource="http://www.w3.org/2002/07/owl#ObjectProperty"/>
    <rdfs:comment xml:lang="en">A permission can be specified either in terms of an Action alone, or an instance of Permission relating an Action and one or more other attributes.</rdfs:comment>
    <rdfs:domain rdf:resource="http://www.w3.org/ns/odrl/2/Policy"/>
    <rdfs:isDefinedBy rdf:resource="http://www.w3.org/ns/odrl/2/"/>
    <rdfs:label xml:lang="en">permission</rdfs:label>
    <rdfs:range>
      <owl:Class>
        <owl:unionOf>
          <rdf:Description>
            <rdf:first rdf:resource="http://www.w3.org/ns/odrl/2/Permission"/>
            <rdf:rest>
              <rdf:Description>
                <rdf:first rdf:resource="http://www.w3.org/ns/odrl/2/Action"/>
                <rdf:rest rdf:resource="http://www.w3.org/1999/02/22-rdf-syntax-ns#nil"/>
              </rdf:Description>
            </rdf:rest>
          </rdf:Description>
        </owl:unionOf>
      </owl:Class>
    </rdfs:range>
    <skos:definition xml:lang="en">Relates the description of an individual Permission to a Policy</skos:definition>
  </rdf:Property>
  <Action rdf:about="http://www.w3.org/ns/odrl/2/play">
    <rdf:type rdf:resource="http://www.w3.org/2004/02/skos/core#Concept"/>
    <rdfs:isDefinedBy rdf:resource="http://www.w3.org/ns/odrl/2/"/>
    <rdfs:label xml:lang="en">Play</rdfs:label>
    <skos:broaderTransitive rdf:resource="http://www.w3.org/ns/odrl/2/present"/>
    <skos:definition xml:lang="en">The Assigner permits/prohibits the Assignees to perform an audio Asset to an audience.</skos:definition>
  </Action>
  <owl:NamedIndividual rdf:about="http://www.w3.org/ns/odrl/2/policyUsage">
    <rdfs:comment xml:lang="en">This will enable constraints to be expressed such as “event lt o:policyUsage” indicating before the policy is exercised.</rdfs:comment>
    <rdfs:isDefinedBy rdf:resource="http://www.w3.org/ns/odrl/2/"/>
    <rdfs:label xml:lang="en">Policy usage time</rdfs:label>
    <skos:definition xml:lang="en">When used as an event in constraints, indicates that the event occurs at the time when the policy is executed.</skos:definition>
  </owl:NamedIndividual>
  <Action rdf:about="http://www.w3.org/ns/odrl/2/present">
    <rdf:type rdf:resource="http://www.w3.org/2004/02/skos/core#Concept"/>
    <rdfs:isDefinedBy rdf:resource="http://www.w3.org/ns/odrl/2/"/>
    <rdfs:label xml:lang="en">Present</rdfs:label>
    <skos:broaderTransitive rdf:resource="http://www.w3.org/ns/odrl/2/use"/>
    <skos:definition xml:lang="en">The Assigner permits/prohibits the Assignees to perform or exhibit an Asset to an audience.</skos:definition>
  </Action>
  <Action rdf:about="http://www.w3.org/ns/odrl/2/preview">
    <ont:deprecatedBy rdf:resource="http://www.w3.org/1999/02/22-rdf-syntax-ns#nil"/>
    <rdf:type rdf:resource="http://www.w3.org/2004/02/skos/core#Concept"/>
    <rdfs:isDefinedBy rdf:resource="http://www.w3.org/ns/odrl/2/"/>
    <rdfs:label xml:lang="en">Preview</rdfs:label>
    <skos:definition xml:lang="en">The act of providing a short preview of the asset.</skos:definition>
  </Action>
  <Action rdf:about="http://www.w3.org/ns/odrl/2/print">
    <rdf:type rdf:resource="http://www.w3.org/2004/02/skos/core#Concept"/>
    <rdfs:comment xml:lang="en">For example, creating a permanent, fixed (static), and directly perceivable representation of the Asset.</rdfs:comment>
    <rdfs:isDefinedBy rdf:resource="http://www.w3.org/ns/odrl/2/"/>
    <rdfs:label xml:lang="en">Print</rdfs:label>
    <skos:broaderTransitive rdf:resource="http://www.w3.org/ns/odrl/2/present"/>
    <skos:definition xml:lang="en">The Assigner permits/prohibits the Assignees to print an Asset onto paper or to create a hard copy.</skos:definition>
  </Action>
  <rdf:Property rdf:about="http://www.w3.org/ns/odrl/2/product">
    <rdf:type rdf:resource="http://www.w3.org/2002/07/owl#DatatypeProperty"/>
    <rdfs:comment xml:lang="en">For example, images may only be reproduced in the XYZ Magazine. This may be used to express [[plus]] semantics;</rdfs:comment>
    <rdfs:isDefinedBy rdf:resource="http://www.w3.org/ns/odrl/2/"/>
    <rdfs:label xml:lang="en">product</rdfs:label>
    <rdfs:range rdf:resource="http://www.w3.org/2001/XMLSchema#string"/>
    <rdfs:subPropertyOf rdf:resource="http://www.w3.org/ns/odrl/2/rightOperand"/>
    <skos:definition xml:lang="en">The specified Product or Service name.</skos:definition>
  </rdf:Property>
  <rdf:Property rdf:about="http://www.w3.org/ns/odrl/2/profile">
    <rdfs:comment xml:lang="en">ODRL Profiles may be defined by community groups and express additional semantics.</rdfs:comment>
    <rdfs:domain rdf:resource="http://www.w3.org/ns/odrl/2/Policy"/>
    <rdfs:isDefinedBy rdf:resource="http://www.w3.org/ns/odrl/2/"/>
    <rdfs:label xml:lang="en">profile</rdfs:label>
    <rdfs:range rdf:resource="http://www.w3.org/2000/01/rdf-schema#Resource"/>
    <skos:definition xml:lang="en">The identifier of an ODRL Profile that this Policy conforms to.</skos:definition>
  </rdf:Property>
  <ConflictTerm rdf:about="http://www.w3.org/ns/odrl/2/prohibit">
    <rdf:type rdf:resource="http://www.w3.org/2002/07/owl#NamedIndividual"/>
    <rdfs:comment xml:lang="en">Used to determine policy conflict outcomes.</rdfs:comment>
    <rdfs:isDefinedBy rdf:resource="http://www.w3.org/ns/odrl/2/"/>
    <rdfs:label xml:lang="en">Prohibit</rdfs:label>
    <skos:definition xml:lang="en">Prohibitions take precedence over permissions</skos:definition>
  </ConflictTerm>
  <rdf:Property rdf:about="http://www.w3.org/ns/odrl/2/prohibition">
    <rdf:type rdf:resource="http://www.w3.org/2002/07/owl#ObjectProperty"/>
    <rdfs:comment xml:lang="en">A prohibition can be specified either in terms of an Action alone, or an instance of Prohibition relating an Action and one or more other attributes.</rdfs:comment>
    <rdfs:domain rdf:resource="http://www.w3.org/ns/odrl/2/Policy"/>
    <rdfs:isDefinedBy rdf:resource="http://www.w3.org/ns/odrl/2/"/>
    <rdfs:label xml:lang="en">prohibition</rdfs:label>
    <rdfs:range>
      <owl:Class>
        <owl:unionOf>
          <rdf:Description>
            <rdf:first rdf:resource="http://www.w3.org/ns/odrl/2/Prohibition"/>
            <rdf:rest>
              <rdf:Description>
                <rdf:first rdf:resource="http://www.w3.org/ns/odrl/2/Action"/>
                <rdf:rest rdf:resource="http://www.w3.org/1999/02/22-rdf-syntax-ns#nil"/>
              </rdf:Description>
            </rdf:rest>
          </rdf:Description>
        </owl:unionOf>
      </owl:Class>
    </rdfs:range>
    <skos:definition xml:lang="en">Relates the description of an individual Prohibition to a Policy.</skos:definition>
  </rdf:Property>
  <rdf:Property rdf:about="http://www.w3.org/ns/odrl/2/proximity">
    <ont:deprecatedBy rdf:resource="http://www.openmobilealliance.com/oma-dd/proximity"/>
    <rdf:type rdf:resource="http://www.w3.org/2002/07/owl#DatatypeProperty"/>
    <rdfs:isDefinedBy rdf:resource="http://www.w3.org/ns/odrl/2/"/>
    <rdfs:label xml:lang="en">proximity</rdfs:label>
    <rdfs:subPropertyOf rdf:resource="http://www.w3.org/ns/odrl/2/rightOperand"/>
    <skos:definition xml:lang="en">An value indicating the closeness or nearness.</skos:definition>
  </rdf:Property>
  <rdf:Property rdf:about="http://www.w3.org/ns/odrl/2/purpose">
    <rdf:type rdf:resource="http://www.w3.org/2002/07/owl#ObjectProperty"/>
    <rdfs:comment xml:lang="en">For example, educational use. Purpose values from [[p3p]] may also be used.</rdfs:comment>
    <rdfs:isDefinedBy rdf:resource="http://www.w3.org/ns/odrl/2/"/>
    <rdfs:label xml:lang="en">purpose</rdfs:label>
    <rdfs:subPropertyOf rdf:resource="http://www.w3.org/ns/odrl/2/rightOperand"/>
    <skos:definition xml:lang="en">Specification of a defined purpose applicable to the asset usage.</skos:definition>
  </rdf:Property>
  <Action rdf:about="http://www.w3.org/ns/odrl/2/read">
    <rdf:type rdf:resource="http://www.w3.org/2004/02/skos/core#Concept"/>
    <rdfs:comment xml:lang="en">For example, the ability to read a record from a database (the Asset).</rdfs:comment>
    <rdfs:isDefinedBy rdf:resource="http://www.w3.org/ns/odrl/2/"/>
    <rdfs:label xml:lang="en">Read</rdfs:label>
    <skos:broaderTransitive rdf:resource="http://www.w3.org/ns/odrl/2/use"/>
    <skos:definition xml:lang="en">The Assigner permits/prohibits the Assignees to obtain data from the Asset.</skos:definition>
  </Action>
  <rdf:Property rdf:about="http://www.w3.org/ns/odrl/2/recipient">
    <rdf:type rdf:resource="http://www.w3.org/2002/07/owl#ObjectProperty"/>
    <rdfs:comment xml:lang="en">The right operand must identify one or more specific parties or categories of party</rdfs:comment>
    <rdfs:isDefinedBy rdf:resource="http://www.w3.org/ns/odrl/2/"/>
    <rdfs:label xml:lang="en">recipient</rdfs:label>
    <rdfs:subPropertyOf rdf:resource="http://www.w3.org/ns/odrl/2/rightOperand"/>
    <skos:definition xml:lang="en">The party that receives the result of the Action on the Asset.</skos:definition>
  </rdf:Property>
  <rdf:Property rdf:about="http://www.w3.org/ns/odrl/2/relation">
    <rdf:type rdf:resource="http://www.w3.org/2002/07/owl#ObjectProperty"/>
    <rdfs:comment xml:lang="en">Sub-properties of relation are used to define the nature of that link.</rdfs:comment>
    <rdfs:domain rdf:resource="http://www.w3.org/ns/odrl/2/Rule"/>
    <rdfs:isDefinedBy rdf:resource="http://www.w3.org/ns/odrl/2/"/>
    <rdfs:label xml:lang="en">relation</rdfs:label>
    <rdfs:range rdf:resource="http://www.w3.org/ns/odrl/2/Asset"/>
    <skos:definition xml:lang="en">Relation is an abstract property which creates an explicit link between an Action and an Asset.</skos:definition>
  </rdf:Property>
  <rdf:Property rdf:about="http://www.w3.org/ns/odrl/2/relativePosition">
    <rdf:type rdf:resource="http://www.w3.org/2002/07/owl#DatatypeProperty"/>
    <rdfs:comment xml:lang="en">For example, JPEG image must be positioned at the Top of the Page. This may be used to express [[plus]] semantics;</rdfs:comment>
    <rdfs:isDefinedBy rdf:resource="http://www.w3.org/ns/odrl/2/"/>
    <rdfs:label xml:lang="en">relative position</rdfs:label>
    <rdfs:subPropertyOf rdf:resource="http://www.w3.org/ns/odrl/2/rightOperand"/>
    <skos:definition xml:lang="en">A point defined with reference to another position.</skos:definition>
  </rdf:Property>
  <rdf:Property rdf:about="http://www.w3.org/ns/odrl/2/relativeSize">
    <rdf:type rdf:resource="http://www.w3.org/2002/07/owl#DatatypeProperty"/>
    <rdfs:comment xml:lang="en">For example, JPEG image resized to maximum of 200%. This may be used to express [[plus]] semantics;</rdfs:comment>
    <rdfs:isDefinedBy rdf:resource="http://www.w3.org/ns/odrl/2/"/>
    <rdfs:label xml:lang="en">relative size</rdfs:label>
    <rdfs:subPropertyOf rdf:resource="http://www.w3.org/ns/odrl/2/rightOperand"/>
    <skos:definition xml:lang="en">The relative dimension that the Asset may be resized.</skos:definition>
  </rdf:Property>
  <Action rdf:about="http://www.w3.org/ns/odrl/2/reproduce">
    <rdf:type rdf:resource="http://www.w3.org/2004/02/skos/core#Concept"/>
    <rdfs:isDefinedBy rdf:resource="http://www.w3.org/ns/odrl/2/"/>
    <rdfs:label xml:lang="en">Reproduce</rdfs:label>
    <skos:broaderTransitive rdf:resource="http://www.w3.org/ns/odrl/2/use"/>
    <skos:definition xml:lang="en">The Assigner permits/prohibits the Assignee(s) to make (an) exact reproduction(s) of the Asset.</skos:definition>
  </Action>
  <rdf:Property rdf:about="http://www.w3.org/ns/odrl/2/resolution">
    <rdfs:comment xml:lang="en">For example, may be printed at 1200dpi.</rdfs:comment>
    <rdfs:isDefinedBy rdf:resource="http://www.w3.org/ns/odrl/2/"/>
    <rdfs:label xml:lang="en">resolution</rdfs:label>
    <rdfs:subPropertyOf rdf:resource="http://www.w3.org/ns/odrl/2/rightOperand"/>
    <skos:definition xml:lang="en">The resolution at which the asset may be used.</skos:definition>
  </rdf:Property>
  <Action rdf:about="http://www.w3.org/ns/odrl/2/reviewPolicy">
    <rdf:type rdf:resource="http://www.w3.org/2004/02/skos/core#Concept"/>
    <rdfs:comment xml:lang="en">Used when human intervention is required to review the Policy. May link to an Asset which represents the full Policy information.</rdfs:comment>
    <rdfs:isDefinedBy rdf:resource="http://www.w3.org/ns/odrl/2/"/>
    <rdfs:label xml:lang="en">Review policy</rdfs:label>
    <skos:definition xml:lang="en">The Assigner requires that the Assignee(s) has(ve) a person review the Policy applicable to the Asset.</skos:definition>
  </Action>
  <rdf:Property rdf:about="http://www.w3.org/ns/odrl/2/rightOperand">
    <rdfs:comment xml:lang="en">Do not use the right-operand property directly within a Constraint. Instead, a Constraint instance must contain exactly one triple which makes use of one of the sub-properties of right-operand.</rdfs:comment>
    <rdfs:domain rdf:resource="http://www.w3.org/ns/odrl/2/Constraint"/>
    <rdfs:isDefinedBy rdf:resource="http://www.w3.org/ns/odrl/2/"/>
    <rdfs:label xml:lang="en">right-operand</rdfs:label>
    <skos:definition xml:lang="en">The operand applied to an instance of a constraint.</skos:definition>
  </rdf:Property>
  <Action rdf:about="http://www.w3.org/ns/odrl/2/secondaryUse">
    <ont:deprecatedBy rdf:resource="http://www.w3.org/1999/02/22-rdf-syntax-ns#nil"/>
    <rdf:type rdf:resource="http://www.w3.org/2004/02/skos/core#Concept"/>
    <rdfs:isDefinedBy rdf:resource="http://www.w3.org/ns/odrl/2/"/>
    <rdfs:label xml:lang="en">Secondary use</rdfs:label>
    <skos:definition xml:lang="en">The act of using the asset for a purpose other than the purpose it was intended for.</skos:definition>
  </Action>
  <Action rdf:about="http://www.w3.org/ns/odrl/2/sell">
    <rdf:type rdf:resource="http://www.w3.org/2004/02/skos/core#Concept"/>
    <rdfs:isDefinedBy rdf:resource="http://www.w3.org/ns/odrl/2/"/>
    <rdfs:label xml:lang="en">Sell</rdfs:label>
    <skos:broaderTransitive rdf:resource="http://www.w3.org/ns/odrl/2/transfer"/>
    <skos:definition xml:lang="en">The Assigner permits/prohibits the Assignees to transfer the ownership of the Asset to a third party with compensation and while deleting the original asset.</skos:definition>
  </Action>
  <Action rdf:about="http://www.w3.org/ns/odrl/2/share">
    <ont:deprecatedBy rdf:resource="http://creativecommons.org/ns#Distribution"/>
    <rdf:type rdf:resource="http://www.w3.org/2004/02/skos/core#Concept"/>
    <rdfs:isDefinedBy rdf:resource="http://www.w3.org/ns/odrl/2/"/>
    <rdfs:label xml:lang="en">Share</rdfs:label>
    <skos:definition xml:lang="en">The act of the non-commercial reproduction and distribution of the asset to third-parties.</skos:definition>
  </Action>
  <Action rdf:about="http://www.w3.org/ns/odrl/2/shareAlike">
    <ont:deprecatedBy rdf:resource="http://creativecommons.org/ns#ShareAlike"/>
    <rdf:type rdf:resource="http://www.w3.org/2004/02/skos/core#Concept"/>
    <rdfs:isDefinedBy rdf:resource="http://www.w3.org/ns/odrl/2/"/>
    <rdfs:label xml:lang="en">Share-alike</rdfs:label>
    <skos:definition xml:lang="en">The act of distributing any derivative asset under the same terms as the original asset.</skos:definition>
  </Action>
  <rdf:Property rdf:about="http://www.w3.org/ns/odrl/2/spatial">
    <rdfs:comment xml:lang="en">The code value and code source must be represented. For example, the [[iso3166]] Country Codes or the Getty Thesaurus of Geographic Names. A URI should be used to represent this value.</rdfs:comment>
    <rdfs:isDefinedBy rdf:resource="http://www.w3.org/ns/odrl/2/"/>
    <rdfs:label xml:lang="en">spatial</rdfs:label>
    <rdfs:subPropertyOf rdf:resource="http://www.w3.org/ns/odrl/2/rightOperand"/>
    <skos:definition xml:lang="en">A code representing a geospatial area.</skos:definition>
  </rdf:Property>
  <rdf:Property rdf:about="http://www.w3.org/ns/odrl/2/status">
    <rdfs:comment xml:lang="en">The range of the status property is identical to that of the operand property selected used in the constraint.</rdfs:comment>
    <rdfs:domain rdf:resource="http://www.w3.org/ns/odrl/2/Constraint"/>
    <rdfs:isDefinedBy rdf:resource="http://www.w3.org/ns/odrl/2/"/>
    <rdfs:label xml:lang="en">status</rdfs:label>
    <skos:definition xml:lang="en">The current value of the constraint.</skos:definition>
  </rdf:Property>
  <UndefinedTerm rdf:about="http://www.w3.org/ns/odrl/2/support">
    <rdf:type rdf:resource="http://www.w3.org/2002/07/owl#NamedIndividual"/>
    <rdfs:comment xml:lang="en">Used to support actions not known to the policy system.</rdfs:comment>
    <rdfs:isDefinedBy rdf:resource="http://www.w3.org/ns/odrl/2/"/>
    <rdfs:label xml:lang="en">Support</rdfs:label>
    <skos:definition xml:lang="en">The Action is to be supported as part of the policy – and the policy remains valid</skos:definition>
  </UndefinedTerm>
  <rdf:Property rdf:about="http://www.w3.org/ns/odrl/2/system">
    <ont:deprecatedBy rdf:resource="http://www.w3.org/ns/odrl/2/systemDevice"/>
    <rdfs:isDefinedBy rdf:resource="http://www.w3.org/ns/odrl/2/"/>
    <rdfs:label xml:lang="en">system</rdfs:label>
    <rdfs:subPropertyOf rdf:resource="http://www.w3.org/ns/odrl/2/rightOperand"/>
    <owl:equivalentProperty rdf:resource="http://www.w3.org/ns/odrl/2/device"/>
    <skos:definition xml:lang="en">An identifiable computing system.</skos:definition>
  </rdf:Property>
  <rdf:Property rdf:about="http://www.w3.org/ns/odrl/2/systemDevice">
    <rdf:type rdf:resource="http://www.w3.org/2002/07/owl#ObjectProperty"/>
    <rdfs:comment xml:lang="en">For example, identifiable via the CPU or unique hardware address.</rdfs:comment>
    <rdfs:isDefinedBy rdf:resource="http://www.w3.org/ns/odrl/2/"/>
    <rdfs:label xml:lang="en">system device</rdfs:label>
    <rdfs:subPropertyOf rdf:resource="http://www.w3.org/ns/odrl/2/rightOperand"/>
    <owl:equivalentProperty rdf:resource="http://www.w3.org/ns/odrl/2/device"/>
    <owl:equivalentProperty rdf:resource="http://www.w3.org/ns/odrl/2/system"/>
    <skos:definition xml:lang="en">An identifiable computing system.</skos:definition>
  </rdf:Property>
  <rdf:Property rdf:about="http://www.w3.org/ns/odrl/2/target">
    <rdf:type rdf:resource="http://www.w3.org/2002/07/owl#ObjectProperty"/>
    <rdfs:comment xml:lang="en">Or not performed by Prohibitions.</rdfs:comment>
    <rdfs:domain rdf:resource="http://www.w3.org/ns/odrl/2/Rule"/>
    <rdfs:isDefinedBy rdf:resource="http://www.w3.org/ns/odrl/2/"/>
    <rdfs:label xml:lang="en">target</rdfs:label>
    <rdfs:range rdf:resource="http://www.w3.org/ns/odrl/2/Asset"/>
    <rdfs:subPropertyOf rdf:resource="http://www.w3.org/ns/odrl/2/relation"/>
    <skos:definition xml:lang="en">The target property specifies the Asset upon which the Action is performed.</skos:definition>
  </rdf:Property>
  <Action rdf:about="http://www.w3.org/ns/odrl/2/textToSpeech">
    <rdf:type rdf:resource="http://www.w3.org/2004/02/skos/core#Concept"/>
    <rdfs:isDefinedBy rdf:resource="http://www.w3.org/ns/odrl/2/"/>
    <rdfs:label xml:lang="en">Text-to-speech</rdfs:label>
    <skos:broaderTransitive rdf:resource="http://www.w3.org/ns/odrl/2/use"/>
    <skos:definition xml:lang="en">The Assigner permits/prohibits the Assignees to have a text Asset read out loud to an audience.</skos:definition>
  </Action>
  <rdf:Property rdf:about="http://www.w3.org/ns/odrl/2/timeInterval">
    <rdf:type rdf:resource="http://www.w3.org/2002/07/owl#DatatypeProperty"/>
    <rdfs:comment xml:lang="en">For example, “P7D” indicates a 7 day period. Value must conform to [iso8601] as represented in [xmlschema11-2].</rdfs:comment>
    <rdfs:isDefinedBy rdf:resource="http://www.w3.org/ns/odrl/2/"/>
    <rdfs:label xml:lang="en">time interval</rdfs:label>
    <rdfs:range rdf:resource="http://www.w3.org/2001/XMLSchema#duration"/>
    <rdfs:subPropertyOf rdf:resource="http://www.w3.org/ns/odrl/2/rightOperand"/>
    <skos:definition xml:lang="en">Recurring period of time in which the usage may be exercised.</skos:definition>
  </rdf:Property>
  <rdf:Property rdf:about="http://www.w3.org/ns/odrl/2/timedCount">
    <ont:deprecatedBy rdf:resource="http://www.openmobilealliance.com/oma-dd/timed-count"/>
    <rdf:type rdf:resource="http://www.w3.org/2002/07/owl#DatatypeProperty"/>
    <rdfs:isDefinedBy rdf:resource="http://www.w3.org/ns/odrl/2/"/>
    <rdfs:label xml:lang="en">timed count</rdfs:label>
    <rdfs:range rdf:resource="http://www.w3.org/2000/01/rdf-schema#Literal"/>
    <rdfs:subPropertyOf rdf:resource="http://www.w3.org/ns/odrl/2/rightOperand"/>
    <skos:definition xml:lang="en">The number of seconds after which timed metering use of the asset begins.</skos:definition>
  </rdf:Property>
  <rdf:Property rdf:about="http://www.w3.org/ns/odrl/2/trackingParty">
    <rdf:type rdf:resource="http://www.w3.org/2002/07/owl#ObjectProperty"/>
    <rdfs:comment xml:lang="en">May be specified as part of the acceptTracking action.</rdfs:comment>
    <rdfs:isDefinedBy rdf:resource="http://www.w3.org/ns/odrl/2/"/>
    <rdfs:label xml:lang="en">tracking party</rdfs:label>
    <rdfs:subPropertyOf rdf:resource="http://www.w3.org/ns/odrl/2/function"/>
    <skos:definition xml:lang="en">The Party is the usage tracker.</skos:definition>
  </rdf:Property>
  <Action rdf:about="http://www.w3.org/ns/odrl/2/transfer">
    <rdf:type rdf:resource="http://www.w3.org/2004/02/skos/core#Concept"/>
    <rdfs:isDefinedBy rdf:resource="http://www.w3.org/ns/odrl/2/"/>
    <rdfs:label xml:lang="en">Transfer</rdfs:label>
    <skos:definition xml:lang="en">The Assigner transfers/does not transfer the ownership in perpetuity to the Assignees.</skos:definition>
  </Action>
  <Action rdf:about="http://www.w3.org/ns/odrl/2/transform">
    <rdf:type rdf:resource="http://www.w3.org/2004/02/skos/core#Concept"/>
    <rdfs:comment xml:lang="en">Typically used to convert the Asset into a different format for consumption on/transfer to a third party system.</rdfs:comment>
    <rdfs:isDefinedBy rdf:resource="http://www.w3.org/ns/odrl/2/"/>
    <rdfs:label xml:lang="en">Transform</rdfs:label>
    <skos:broaderTransitive rdf:resource="http://www.w3.org/ns/odrl/2/use"/>
    <skos:definition xml:lang="en">The Assigner permits/prohibits the Assignees to make a digital copy of the digital Asset in another digital format.</skos:definition>
  </Action>
  <Action rdf:about="http://www.w3.org/ns/odrl/2/translate">
    <rdf:type rdf:resource="http://www.w3.org/2004/02/skos/core#Concept"/>
    <rdfs:comment xml:lang="en">A new derivative Asset is created by that action.</rdfs:comment>
    <rdfs:isDefinedBy rdf:resource="http://www.w3.org/ns/odrl/2/"/>
    <rdfs:label xml:lang="en">Translate</rdfs:label>
    <skos:broaderTransitive rdf:resource="http://www.w3.org/ns/odrl/2/use"/>
    <skos:definition xml:lang="en">The Assigner permits/prohibits the Assignees to translate the original natural language of an Asset into another natural language.</skos:definition>
  </Action>
  <rdf:Property rdf:about="http://www.w3.org/ns/odrl/2/undefined">
    <rdf:type rdf:resource="http://www.w3.org/2002/07/owl#ObjectProperty"/>
    <rdfs:comment xml:lang="en">If no mechanism is specified, the default is invalid.</rdfs:comment>
    <rdfs:domain rdf:resource="http://www.w3.org/ns/odrl/2/Policy"/>
    <rdfs:isDefinedBy rdf:resource="http://www.w3.org/ns/odrl/2/"/>
    <rdfs:label xml:lang="en">undefined</rdfs:label>
    <rdfs:range rdf:resource="http://www.w3.org/ns/odrl/2/UndefinedTerm"/>
    <skos:definition xml:lang="en">Relates the mechanism used for handling undefined actions to a Policy.</skos:definition>
  </rdf:Property>
  <Action rdf:about="http://www.w3.org/ns/odrl/2/uninstall">
    <rdf:type rdf:resource="http://www.w3.org/2004/02/skos/core#Concept"/>
    <rdfs:comment xml:lang="en">The Asset is no longer accessible to the Assignees.</rdfs:comment>
    <rdfs:isDefinedBy rdf:resource="http://www.w3.org/ns/odrl/2/"/>
    <rdfs:label xml:lang="en">Uninstall</rdfs:label>
    <skos:definition xml:lang="en">The Assigner requires that the Assignees unload and delete the computer program Asset from a storage device and disable its readiness for operation.</skos:definition>
  </Action>
  <rdf:Property rdf:about="http://www.w3.org/ns/odrl/2/unit">
    <rdfs:domain rdf:resource="http://www.w3.org/ns/odrl/2/Constraint"/>
    <rdfs:isDefinedBy rdf:resource="http://www.w3.org/ns/odrl/2/"/>
    <rdfs:label xml:lang="en">unit</rdfs:label>
    <rdfs:range rdf:resource="http://www.w3.org/2000/01/rdf-schema#Resource"/>
    <skos:definition xml:lang="en">The unit of measurement used for the constraint value.</skos:definition>
  </rdf:Property>
  <Action rdf:about="http://www.w3.org/ns/odrl/2/use">
    <rdf:type rdf:resource="http://www.w3.org/2004/02/skos/core#Concept"/>
    <rdfs:comment xml:lang="en">Use is the most generic action for all non-third-party usage. More details may be defined in the applicable agreements or under applicable commercial laws. Refined types of actions can be expressed by the narrower actions.</rdfs:comment>
    <rdfs:isDefinedBy rdf:resource="http://www.w3.org/ns/odrl/2/"/>
    <rdfs:label xml:lang="en">Use</rdfs:label>
    <skos:definition xml:lang="en">The Assigner permits/prohibits the Assignee to use the Asset as agreed.</skos:definition>
  </Action>
  <rdf:Property rdf:about="http://www.w3.org/ns/odrl/2/version">
    <rdf:type rdf:resource="http://www.w3.org/2002/07/owl#ObjectProperty"/>
    <rdfs:comment xml:lang="en">For example, Single Paperback, or Multiple Issues. This may be used to express [[plus]] semantics.</rdfs:comment>
    <rdfs:isDefinedBy rdf:resource="http://www.w3.org/ns/odrl/2/"/>
    <rdfs:label xml:lang="en">version</rdfs:label>
    <rdfs:subPropertyOf rdf:resource="http://www.w3.org/ns/odrl/2/rightOperand"/>
    <skos:definition xml:lang="en">The scope of versions for the asset.</skos:definition>
  </rdf:Property>
  <rdf:Property rdf:about="http://www.w3.org/ns/odrl/2/virtualLocation">
    <rdf:type rdf:resource="http://www.w3.org/2002/07/owl#ObjectProperty"/>
    <rdfs:comment xml:lang="en">For example, an Internet domain or IP address range.</rdfs:comment>
    <rdfs:isDefinedBy rdf:resource="http://www.w3.org/ns/odrl/2/"/>
    <rdfs:label xml:lang="en">virtual location</rdfs:label>
    <rdfs:subPropertyOf rdf:resource="http://www.w3.org/ns/odrl/2/rightOperand"/>
    <skos:definition xml:lang="en">Specification of a digital locale.</skos:definition>
  </rdf:Property>
  <Action rdf:about="http://www.w3.org/ns/odrl/2/watermark">
    <rdf:type rdf:resource="http://www.w3.org/2004/02/skos/core#Concept"/>
    <rdfs:comment xml:lang="en">It is recommended to embed a link to the watermark.</rdfs:comment>
    <rdfs:isDefinedBy rdf:resource="http://www.w3.org/ns/odrl/2/"/>
    <rdfs:label xml:lang="en">Watermark</rdfs:label>
    <skos:definition xml:lang="en">The Assigner requires that the Assignees apply a watermark as provided by the Assigner to the Asset.</skos:definition>
  </Action>
  <Action rdf:about="http://www.w3.org/ns/odrl/2/write">
    <ont:deprecatedBy rdf:resource="http://www.w3.org/ns/odrl/2/modify"/>
    <rdf:type rdf:resource="http://www.w3.org/2004/02/skos/core#Concept"/>
    <rdfs:isDefinedBy rdf:resource="http://www.w3.org/ns/odrl/2/"/>
    <rdfs:label xml:lang="en">Write</rdfs:label>
    <skos:definition xml:lang="en">The act of writing to the asset.</skos:definition>
  </Action>
  <Action rdf:about="http://www.w3.org/ns/odrl/2/writeTo">
    <ont:deprecatedBy rdf:resource="http://www.w3.org/ns/odrl/2/modify"/>
    <rdf:type rdf:resource="http://www.w3.org/2004/02/skos/core#Concept"/>
    <rdfs:isDefinedBy rdf:resource="http://www.w3.org/ns/odrl/2/"/>
    <rdfs:label xml:lang="en">Write to</rdfs:label>
    <skos:broaderTransitive rdf:resource="http://www.w3.org/ns/odrl/2/use"/>
    <skos:definition xml:lang="en">The act of adding data to the Asset.</skos:definition>
  </Action>
</rdf:RDF>
