@base <http://www.w3.org/ns/odrl/2/> .
@prefix : <http://www.w3.org/ns/odrl/2/> .
@prefix odrl: <http://www.w3.org/ns/odrl/2/> .
@prefix rdf: <http://www.w3.org/1999/02/22-rdf-syntax-ns#> .
@prefix rdfs: <http://www.w3.org/2000/01/rdf-schema#> .
@prefix skos: <http://www.w3.org/2004/02/skos/core#> .
@prefix owl: <http://www.w3.org/2002/07/owl#> .
@prefix xsd: <http://www.w3.org/2001/XMLSchema#> .
@prefix dct: <http://purl.org/dc/terms/> .
@prefix dcmit: <http://purl.org/dc/dcmitype/> .
@prefix voaf: <http://purl.org/vocommons/voaf#> .
@prefix schema: <http://schema.org/> .
@prefix foaf: <http://xmlns.com/foaf/0.1/> .
@prefix vcard: <http://www.w3.org/2006/vcard/ns#> .

odrl:
	a owl:Ontology , voaf:Vocabulary ;
	rdfs:label "ODRL Version 2.2"@en ;
	owl:versionInfo "2.2" ;
	dct:creator "Mo McRoberts", "Renato Iannella", "Michael Steidl", "Stuart Myles", "Víctor Rodríguez-Doncel" ;
	dct:issued "2017-05-09"^^xsd:date ;
	dct:contributor "W3C Permissions & Obligations Expression Working Group" ;
	dct:description "The ODRL Vocabulary and Expression defines a set of concepts and terms (the vocabulary) and encoding mechanism (the expression) for permissions and obligations statements describing digital content usage based on the ODRL Information Model."@en ;
	rdfs:comment "This is the RDF ontology for ODRL Version 2.2 (working draft)."@en ;
	dct:license <https://www.w3.org/Consortium/Legal/2002/ipr-notice-20021231#Copyright/> .

<http://www.w3.org/ns/odrl/2/ODRL22.ttl>
	a dcmit:Text ;
	rdfs:label "ODRL 2.2 (Turtle Ontology Definition)"@en ;
	dct:subject odrl: ;
	dct:isVersionOf odrl: ;
	dct:format <http://purl.org/NET/mediatypes/text/turtle> .

<http://www.w3.org/ns/odrl/2/ODRL22.rdf>
	a dcmit:Text ;
	rdfs:label "ODRL 2.2 (RDF/XML Ontology Definition)"@en ;
	dct:subject odrl: ;
	dct:isVersionOf odrl: ;
	dct:format <http://purl.org/NET/mediatypes/application/rdf+xml> .

<http://www.w3.org/ns/odrl/2/ODRL22.xsd>
	a dcmit:Text ;
	rdfs:label "ODRL 2.2 (XML Schema Definition)"@en ;
	dct:subject odrl: ;
	dct:isVersionOf odrl: ;
	dct:format <http://purl.org/NET/mediatypes/application/xml> .

<http://www.w3.org/ns/odrl/2/ODRL22.jsonld>
	a dcmit:Text ;
	rdfs:label "ODRL 2.2 (JSON-LD Definition)"@en ;
	dct:subject odrl: ;
	dct:isVersionOf odrl: ;
	dct:format <http://purl.org/NET/mediatypes/application/ld+json> .


## SKOS Collections for Grouping related concepts

<http://www.w3.org/ns/odrl/2/#policyConcepts>
    a skos:Collection ;
    skos:prefLabel "Policy"@en ;
    skos:member :Policy ;
    skos:member :Rule ;
    skos:member :profile .


<http://www.w3.org/ns/odrl/2/#inheritanceConcepts>
    a skos:Collection ;
    skos:prefLabel "Policy Inheritance"@en ;
    skos:member :inheritAllowed ;
    skos:member :inheritFrom .

<http://www.w3.org/ns/odrl/2/#conflictConcepts>
    a skos:Collection ;
    skos:prefLabel "Policy Conflict Strategy"@en ;
    skos:member :ConflictTerm ;
    skos:member :conflict ;
    skos:member :perm ;
    skos:member :prohibit ;
    skos:member :invalid .


<http://www.w3.org/ns/odrl/2/#policySubClasses>
    a skos:Collection ;
    skos:prefLabel "Policy Subclasses"@en ;
    skos:member :Agreement ;
    skos:member :Assertion ;
    skos:member :Offer ;
    skos:member :Privacy ;
    skos:member :Request ;
    skos:member :Set ;
    skos:member :Ticket .

<http://www.w3.org/ns/odrl/2/#assetConcepts>
    a skos:Collection ;
    skos:prefLabel "Asset"@en ;
    skos:member :Asset ;
    skos:member :relation ;
    skos:member :AssetScope .

<http://www.w3.org/ns/odrl/2/#assetRelations>
    a skos:Collection ;
    skos:prefLabel "Asset Relations"@en ;
    skos:member :target ;
    skos:member :output .


<http://www.w3.org/ns/odrl/2/#partyConcepts>
    a skos:Collection ;
    skos:prefLabel "Party"@en ;
    skos:member :Party ;
    skos:member :function ;
    skos:member :PartyScope .

<http://www.w3.org/ns/odrl/2/#partyAssetConcepts>
    a skos:Collection ;
    skos:prefLabel "Party and Asset"@en ;
    skos:member :scope .


<http://www.w3.org/ns/odrl/2/#partyRoles>
    a skos:Collection ;
    skos:prefLabel "Party Functions"@en ;
    skos:member :assignee ;
    skos:member :assigner ;
    skos:member :attributedParty ;
    skos:member :attributingParty ;
    skos:member :compensatedParty ;
    skos:member :compensatingParty ;
    skos:member :consentingParty ;
    skos:member :consentedParty ;
    skos:member :contractingParty ;
    skos:member :contractedParty ;
    skos:member :informedParty ;
    skos:member :informingParty ;
    skos:member :trackingParty ;
    skos:member :trackedParty .


<http://www.w3.org/ns/odrl/2/#partyScopes>
    a skos:Collection ;
    skos:prefLabel "Party Scopes"@en ;
    skos:member :Group ;
    skos:member :Individual ;
    skos:member :All ;
    skos:member :AllConnections ;
    skos:member :All2ndConnections ;
    skos:member :AllGroups .

<http://www.w3.org/ns/odrl/2/#actionConcepts>
    a skos:Collection ;
    skos:prefLabel "Action"@en ;
    skos:member :Action ;
    skos:member :action .

<http://www.w3.org/ns/odrl/2/#permissions>
    a skos:Collection ;
    skos:prefLabel "Permission"@en ;
    skos:member :Permission ;
    skos:member :permission .

<http://www.w3.org/ns/odrl/2/#prohibitions>
    a skos:Collection ;
    skos:prefLabel "Prohibition"@en ;
    skos:member :Prohibition ;
    skos:member :prohibition .

<http://www.w3.org/ns/odrl/2/#actions>
    a skos:Collection ;
    skos:prefLabel "Actions for Permissions and Prohibitions"@en ;
    skos:member :use ;
    skos:member :grantUse ;
    skos:member :aggregate ;
    skos:member :annotate ;
    skos:member :anonymize ;
    skos:member :archive ;
    skos:member :concurrentUse ;
    skos:member :derive ;
    skos:member :digitize ;
    skos:member :display ;
    skos:member :distribute ;
    skos:member :execute ;
    skos:member :extract ;
    skos:member :give ;
    skos:member :index ;
    skos:member :install ;
    skos:member :modify ;
    skos:member :move ;
    skos:member :play ;
    skos:member :present ;
    skos:member :print ;
    skos:member :read ;
    skos:member :reproduce ;
    skos:member :sell ;
    skos:member :stream ;
    skos:member :textToSpeech ;
    skos:member :transfer ;
    skos:member :transform ;
    skos:member :translate .


<http://www.w3.org/ns/odrl/2/#duties>
    a skos:Collection ;
    skos:prefLabel "Duty"@en ;
    skos:member :Duty ;
    skos:member :duty ; .


<http://www.w3.org/ns/odrl/2/#dutyActions>
    a skos:Collection ;
    skos:prefLabel "Actions for Duties"@en ;
    skos:member :acceptTracking ;
    skos:member :attribute ;
    skos:member :compensate ;
    skos:member :delete ;
    skos:member :ensureExclusivity ;
    skos:member :include ;
    skos:member :inform ;
    skos:member :nextPolicy ;
    skos:member :obtainConsent ;
    skos:member :reviewPolicy ;
    skos:member :uninstall ;
    skos:member :watermark .

<http://www.w3.org/ns/odrl/2/#constraints>
    a skos:Collection ;
    skos:prefLabel "Constraint"@en ;
    skos:member :Constraint ;
    skos:member :constraint ;
    skos:member :Operator ;
    skos:member :operator ;
	skos:member :RightOperand ;
    skos:member :rightOperand ;
    skos:member :rightOperandReference ;
	skos:member :LeftOperand ;
	skos:member :leftOperand ;
    skos:member :unit ;
    skos:member :dataType ;
    skos:member :status .

<http://www.w3.org/ns/odrl/2/#constraintLeftOperand>
    a skos:Collection ;
    skos:prefLabel "Constraint Left Operands"@en ;
    skos:member :absolutePosition ;
    skos:member :absoluteSpatialPosition ;
    skos:member :absoluteTemporalPosition ;
    skos:member :absoluteSize ;
    skos:member :count ;
    skos:member :dateTime ;
    skos:member :delayPeriod ;
    skos:member :deliveryChannel ;
    skos:member :elapsedTime ;
    skos:member :event ;
    skos:member :fileFormat ;
    skos:member :industry ;
    skos:member :language ;
    skos:member :media ;
    skos:member :meteredTime ;
    skos:member :payAmount ;
    skos:member :percentage ;
    skos:member :product ;
    skos:member :purpose ;
    skos:member :recipient ;
    skos:member :relativePosition ;
    skos:member :relativeSpatialPosition ;
    skos:member :relativeTemporalPosition ;
    skos:member :relativeSize ;
    skos:member :resolution ;
    skos:member :spatial ;
    skos:member :spatialCoordinates ;
    skos:member :systemDevice ;
    skos:member :timeInterval ;
    skos:member :unitOfCount ;
    skos:member :version ;
    skos:member :virtualLocation .


<http://www.w3.org/ns/odrl/2/#constraintOperators>
    a skos:Collection ;
    skos:prefLabel "Constraint Operators"@en ;
    skos:member :eq ;
    skos:member :gt ;
    skos:member :gteq ;
    skos:member :lt ;
    skos:member :lteq ;
    skos:member :neq ;
    skos:member :isA ;
    skos:member :hasPart ;
    skos:member :isPartOf ;
    skos:member :isAllOf ;
    skos:member :isAnyOf ;
    skos:member :isNoneOf ;
    skos:member :or ;
    skos:member :xor ;
    skos:member :and ;
    skos:member :andSequence .

<http://www.w3.org/ns/odrl/2/#constraintRightOp>
    a skos:Collection ;
    skos:prefLabel "Constraint Right Operands"@en ;
    skos:member :policyUsage .


<http://www.w3.org/ns/odrl/2/#deprecatedTerms>
    a skos:Collection ;
    skos:prefLabel "Deprecated Terms"@en ;
    skos:member :device ;
    skos:member :system ;
    skos:member :proximity ;
    skos:member :append ;
    skos:member :appendTo ;
    skos:member :copy ;
    skos:member :export ;
    skos:member :lease ;
    skos:member :license ;
    skos:member :lend ;
    skos:member :pay ;
    skos:member :payeeParty ;
    skos:member :preview ;
    skos:member :secondaryUse ;
    skos:member :write ;
    skos:member :writeTo ;
    skos:member :adHocShare ;
    skos:member :extractChar ;
    skos:member :extractPage ;
    skos:member :extractWord ;
    skos:member :attachPolicy ;
    skos:member :attachSource ;
    skos:member :shareAlike ;
    skos:member :commercialize ;
    skos:member :share ;
    skos:member :timedCount ;
    skos:member :inheritRelation ;
    skos:member :UndefinedTerm ;
    skos:member :undefined ;
    skos:member :ignore ;
    skos:member :support .



## SKOS Concept Schemes

:actions
	a skos:ConceptScheme ;
	rdfs:isDefinedBy odrl: ;
	rdfs:label "ODRL Actions Vocabulary"@en ;
	skos:hasTopConcept :acceptTracking, :aggregate, :annotate,
		:anonymize, :archive,
		:attribute, :concurrentUse, :delete,
		:derive, :display, :distribute, :digitize, :ensureExclusivity, :execute,
		:extract, :give, :include, :index, :inform,
		:install, :modify, :move, :nextPolicy,
		:obtainConsent, :play, :present, :print, :read,
		:reproduce, :reviewPolicy, :sell,
		:textToSpeech, :transform, :transfer, :translate, :uninstall,
		:watermark, :use, :grantUse, :compensate .

## Assets

:Asset
	a rdfs:Class , owl:Class ;
	rdfs:isDefinedBy odrl: ;
	rdfs:label "Asset"@en ;
	skos:definition "An identifiable resource that is the subject of a Rule."@en ;
    skos:note "The Asset entity can be any form of identifiable resource, such as data/information, content/media, applications, or services. Furthermore, it can be used to represent other Asset entities that are needed to undertake the Policy expression, such as with the Duty entity. To describe more details about the Asset, it is recommened to use Dublin Core [[dcterms]] elements or other content metadata."@en .

## Parties

:Party
	a rdfs:Class , owl:Class ;
	rdfs:isDefinedBy odrl: ;
	rdfs:label "Party"@en ;
	skos:definition "An identifiable entity who may undertake a functional role in a Policy."@en ;
	rdfs:subClassOf [
		a owl:Class ;
		owl:unionOf ( schema:Person schema:Organization foaf:Person foaf:Organization vcard:Individual vcard:Organization ) ;
	];
	skos:note "The Party entity could be a person, group of people, organisation, or agent. An agent is a person or thing that takes an active role or produces a specified effect. To describe more details about the Party, it is recommened to use W3C vCard Ontology [[vcard-rdf]] or FOAF Vocabulary [[foaf]]."@en .

## Policies

:Policy
	a rdfs:Class , owl:Class ;
	rdfs:isDefinedBy odrl: ;
	rdfs:label "Policy"@en ;
	skos:definition "A Rule expressing what Action is allowed and/or disallowed over an Asset."@en ;
	skos:note "A Policy may contain multiple Rules."@en .

:ConflictTerm
	a rdfs:Class, owl:Class ;
	rdfs:isDefinedBy odrl: ;
    skos:definition "Used to establish strategies to resolve conflicts that arise from the merging of Policies or conflicts between Permissions and Prohibitions in the same Policy."@en ;
    skos:note "Instances of ConflictTerm describe strategies for resolving conflicts."@en ;
	rdfs:label "Conflict Stratey Preference"@en ;
    skos:scopeNote "Non-Normative"@en .

:perm
	a :ConflictTerm, owl:NamedIndividual ;
	rdfs:isDefinedBy odrl: ;
	rdfs:label "Prefer Permissions"@en ;
    skos:definition "Permissions take preference over prohibitions."@en ;
    skos:note "Used to determine policy conflict outcomes."@en ;
    skos:scopeNote "Non-Normative"@en .

:prohibit
	a :ConflictTerm, owl:NamedIndividual;
	rdfs:isDefinedBy odrl: ;
	rdfs:label "Prefer Prohibitions"@en ;
    skos:definition "Prohibitions take preference over permissions."@en ;
	skos:note "Used to determine policy conflict outcomes."@en ;
    skos:scopeNote "Non-Normative"@en .

:UndefinedTerm
	a rdfs:Class, owl:Class ;
	rdfs:isDefinedBy odrl: ;
	skos:definition "Is used to indicate how to support Actions that are not part of any vocabulary or profile in the policy expression system."@en ;
	skos:note "Instances of UndefinedTerm describe strategies for processing unsupported actions."@en ;
	rdfs:label "Undefined Term"@en ;
    owl:deprecated true .

:ignore
	a :UndefinedTerm, owl:NamedIndividual ;
	rdfs:isDefinedBy odrl: ;
	rdfs:label "Ignore Undefined Actions"@en ;
	skos:definition "The Action is to be ignored and is not part of the policy – and the policy remains valid."@en ;
	skos:note "Used to support actions not known to the policy system."@en ;
    owl:deprecated true .

:invalid
	a :ConflictTerm, owl:NamedIndividual ;
	rdfs:isDefinedBy odrl: ;
	rdfs:label "Invalidate Policy"@en ;
	skos:definition "The policy is invalid."@en ;
	skos:note "Used to indicate the policy is invalid for Conflict Strategy."@en ;
    skos:scopeNote "Non-Normative"@en .

:support
	a :UndefinedTerm, owl:NamedIndividual ;
	rdfs:isDefinedBy odrl: ;
	rdfs:label "Support Undefined Actions"@en ;
	skos:definition "The Action is to be supported as part of the policy – and the policy remains valid."@en ;
	skos:note "Used to support actions not known to the policy system."@en ;
    owl:deprecated true .

:conflict
	a rdf:Property , owl:ObjectProperty ;
	rdfs:isDefinedBy odrl: ;
	rdfs:label "Handle Policy Conflicts"@en ;
	skos:definition "The conflict-resolution strategy for a Policy."@en ;
	skos:note "If no strategy is specified, the default is invalid."@en ;
	rdfs:domain :Policy ;
	rdfs:range :ConflictTerm ;
    skos:scopeNote "Non-Normative"@en .

:undefined
	a rdf:Property , owl:ObjectProperty ;
	rdfs:isDefinedBy odrl: ;
	rdfs:label "Handle Undefined Term"@en ;
	skos:definition "Relates the strategy used for handling undefined actions to a Policy."@en ;
	skos:note "If no strategy is specified, the default is invalid."@en ;
	rdfs:range :UndefinedTerm ;
    owl:deprecated true .

:permission
	a rdf:Property , owl:ObjectProperty ;
	rdfs:isDefinedBy odrl: ;
	rdfs:label "Has Permission"@en ;
	skos:definition "Relates the description of an individual Permission to a Policy."@en ;
	skos:note "A permission can be specified either in terms of an Action alone, or an instance of Permission relating an Action and one or more other attributes."@en ;
	rdfs:domain :Policy ;
	rdfs:range [
		a owl:Class ;
		owl:unionOf ( :Permission :Action ) ;
	] .

:prohibition
	a rdf:Property , owl:ObjectProperty ;
	rdfs:isDefinedBy odrl: ;
	rdfs:label "Has Prohibition"@en ;
	skos:definition "Relates the description of an individual Prohibition to a Policy."@en ;
	skos:note "A prohibition can be specified either in terms of an Action alone, or an instance of Prohibition relating an Action and one or more other attributes."@en ;
	rdfs:domain :Policy ;
	rdfs:range [
		a owl:Class ;
		owl:unionOf ( :Prohibition  :Action ) ;
	] .

:inheritAllowed
	a rdf:Property , owl:DatatypeProperty ;
	rdfs:isDefinedBy odrl: ;
	rdfs:label "Inheritance Allowed"@en ;
	skos:definition "Indicates if the Policy entity can be inherited."@en ;
	skos:note "A boolean value."@en ;
	rdfs:domain :Policy ;
	rdfs:range xsd:boolean ;
    skos:scopeNote "Non-Normative"@en .

:inheritFrom
	a rdf:Property , owl:ObjectProperty ;
	rdfs:isDefinedBy odrl: ;
	rdfs:label "Inherits From"@en ;
	skos:definition "Relates a (child) policy to another (parent) policy from which terms are inherited."@en ;
	skos:note "The child policy will inherit from the parent policy"@en ;
	rdfs:domain :Policy ;
	rdfs:range :Policy ;
    skos:scopeNote "Non-Normative"@en .

:inheritRelation
	a rdf:Property , owl:ObjectProperty ;
	rdfs:isDefinedBy odrl: ;
	rdfs:label "Inherit Relation"@en ;
	skos:definition "Indentifies the type of inheritance."@en ;
	skos:note "For example, this may indicate the business scenario, such as subscription, or prior arrangements between the parties (that are not machine representable)."@en ;
#	rdfs:domain :Policy ;
#	rdfs:range rdfs:Resource ;
    owl:deprecated true .


:profile
	a rdf:Property ;
	rdfs:isDefinedBy odrl: ;
	rdfs:label "Profile"@en ;
	skos:definition "The identifier of an ODRL Profile that the Policy conforms to."@en ;
	skos:note "ODRL Profiles may be defined by community groups and express additional semantics."@en ;
	rdfs:domain :Policy .
#	rdfs:range rdfs:Resource .

## Permissions, prohibitions and duties

:Rule
	a rdfs:Class , owl:Class ;
	rdfs:isDefinedBy odrl: ;
	rdfs:label "Rule"@en ;
	skos:definition "A Permission, Prohibition or Duty that expresses an Action that may, must not, or must be performed (respectively)."@en ;
	skos:note "Rule is an abstract concept."@en .

:Permission
	a rdfs:Class , owl:Class ;
	rdfs:isDefinedBy odrl: ;
	rdfs:subClassOf :Rule ;
	owl:disjointWith :Prohibition, :Duty ;
	rdfs:label "Permission"@en ;
	skos:definition "An Action that may be performed over an Asset."@en ;
	skos:note "In other words, what the assigner (supplier) has granted to the assignee (consumer)."@en .

:Prohibition
	a rdfs:Class , owl:Class ;
	rdfs:isDefinedBy odrl: ;
	rdfs:subClassOf :Rule ;
	owl:disjointWith :Duty, :Permission ;
	rdfs:label "Prohibition"@en ;
	skos:definition "An Action that must not be performed over an Asset."@en ;
	skos:note "Prohibitions are issued by the supplier of the Asset – the Party with the function assigner."@en .

:Duty
	a rdfs:Class , owl:Class ;
	rdfs:isDefinedBy odrl: ;
	rdfs:subClassOf :Rule ;
	owl:disjointWith :Prohibition, :Permission ;
	rdfs:label "Duty"@en ;
    skos:definition "An Action that has been agreed to be performed as a requirement for the applicable Permission to become valid."@en .

:Action
	a rdfs:Class, owl:Class ;
	rdfs:isDefinedBy odrl: ;
	rdfs:subClassOf skos:Concept ;
	skos:definition "An operation that is applicable to an Asset."@en ;
	skos:note "Actions may be allowed by Permissions, disallowed by Prohibitions, or made mandatory by Duties."@en ;
	rdfs:subClassOf schema:Action ;
	rdfs:label "Action"@en .

:Constraint
	a rdfs:Class, owl:Class ;
	rdfs:isDefinedBy odrl: ;
	rdfs:subClassOf owl:Thing ;
	rdfs:label "Constraint"@en ;
	skos:definition "The context, such as limitations, restrictions, or interpretations, that must be applied to an Action."@en ;
	skos:note "Parent class of all Constraints."@en .

:relation
	a rdf:Property , owl:ObjectProperty ;
	rdfs:isDefinedBy odrl: ;
	rdfs:label "Relation"@en ;
	skos:definition "Relation is an abstract property which creates an explicit link between an Action and an Asset."@en ;
	skos:note "Sub-properties of relation are used to define the nature of that link."@en ;
	rdfs:domain :Rule ;
	rdfs:range :Asset .

:output
	a rdf:Property , owl:ObjectProperty ;
	rdfs:isDefinedBy odrl: ;
	rdfs:subPropertyOf :relation ;
	rdfs:label "Output"@en ;
	skos:definition "The output property specifies the Asset which is created from the output of the Action."@en ;
	rdfs:domain :Rule ;
	rdfs:range :Asset  ;
    skos:scopeNote "Non-Normative"@en .

:target
	a rdf:Property , owl:ObjectProperty ;
	rdfs:isDefinedBy odrl: ;
	rdfs:subPropertyOf :relation ;
	rdfs:label "Target"@en ;
	skos:definition "The target property indicates the Asset that is the primary subject to which the Rule action directly applies."@en ;
	rdfs:domain :Rule ;
	rdfs:range :Asset .

:function
	a rdf:Property , owl:ObjectProperty ;
	rdfs:isDefinedBy odrl: ;
	rdfs:label "Function"@en ;
	skos:definition "Function is an abstract property whose sub-properties define the functional roles which may be fulfilled by a party in relation to a Rule."@en ;
	rdfs:domain :Rule ;
	rdfs:range :Party .

:scope
	a rdf:Property , owl:ObjectProperty ;
	rdfs:isDefinedBy odrl: ;
	rdfs:label "Scope"@en ;
	skos:definition "The identifier of a scope that provides context to the extent of the entity."@en ;
	skos:note "Used to define scopes for Assets and Parties."@en ;
	rdfs:range [
		a owl:Class ;
		owl:unionOf ( :AssetScope :PartyScope ) ;
	] .

:action
	a rdf:Property , owl:ObjectProperty ;
	rdfs:isDefinedBy odrl: ;
	rdfs:label "Has Action"@en ;
	skos:definition "The operation relating to the Asset for which the Rule is being subjected."@en ;
	rdfs:domain :Rule ;
	rdfs:range :Action .

:constraint
	a rdf:Property , owl:ObjectProperty ;
	rdfs:isDefinedBy odrl: ;
	rdfs:label "Has Constraint"@en ;
	skos:definition "The constraint relating to the Rule."@en ;
	skos:note "One or more constraints which affect the validity of the Rule; e.g. if the Action play is only permitted for a certain period of time."@en ;
	rdfs:domain :Rule ;
	rdfs:range :Constraint .

:duty
	a rdf:Property , owl:ObjectProperty ;
	rdfs:isDefinedBy odrl: ;
	rdfs:label "Has Duty"@en ;
	skos:definition "The duty relating to the Permission."@en ;
	skos:note "A Duty indicates requirements which must be fulfilled in order to receive the permission."@en ;
	rdfs:domain :Permission ;
	rdfs:range [
		a owl:Class ;
		owl:unionOf ( :Duty :Action ) ;
	] .

:unit
	a rdf:Property ;
	rdfs:isDefinedBy odrl: ;
	rdfs:domain :Constraint ;
#	rdfs:range rdfs:Resource ;
	rdfs:label "Unit"@en ;
	skos:definition "The unit of measurement used for the constraint value."@en .

:dataType
	a rdf:Property ;
	rdfs:isDefinedBy odrl: ;
	rdfs:domain :Constraint ;
#	rdfs:range rdfs:Resource ;
	rdfs:label "Datatype"@en ;
	skos:definition "The datatype used for the constraint value."@en ;
    skos:note "In RDF encodings, use of the rdf:datatype MAY be used."@en .

:operator
	a rdf:Property , owl:ObjectProperty ;
	rdfs:isDefinedBy odrl: ;
	rdfs:label "Has Operator"@en ;
	skos:definition "The logical operator function applied to a constraint and its operands."@en ;
	rdfs:domain :Constraint ;
	rdfs:range :Operator .

:rightOperand
	a rdf:Property ;
	rdfs:isDefinedBy odrl: ;
	rdfs:label "Has Right Operand"@en ;
	skos:definition "The right operand in a constraint expression."@en ;
#	rdfs:range xsd:any ;
	rdfs:domain :Constraint .

:rightOperandReference
	a rdf:Property ;
	rdfs:isDefinedBy odrl: ;
	rdfs:label "Has Right Operand Reference"@en ;
	skos:definition "A reference to the operand applied to an instance of a constraint."@en ;
	skos:note "Represents an IRI that must be dereferenced to obtain the actual right operand value"@en ;
	rdfs:domain :Constraint ;
    skos:scopeNote "Non-Normative"@en .

:leftOperand
	a rdf:Property ;
	rdfs:isDefinedBy odrl: ;
	rdfs:label "Has Left Operand"@en ;
	skos:definition "The left operand in a constraint expression."@en ;
	rdfs:range :LeftOperand ;
	rdfs:domain :Constraint .

:status
	a rdf:Property ;
	rdfs:isDefinedBy odrl: ;
	rdfs:label "Status"@en ;
	skos:definition "the current value generated from the leftOperand action."@en ;
	rdfs:domain :Constraint ;
    skos:scopeNote "Non-Normative"@en .

## Operators

:Operator
	a rdfs:Class , owl:Class ;
	rdfs:isDefinedBy odrl: ;
	rdfs:subClassOf owl:Thing ;
	rdfs:label "Operator"@en ;
	skos:definition "Operators for constraint expressions."@en ;
	skos:note "Instances of the Operator class representing boolean operators and logical relationships."@en .

:eq
	a :Operator, owl:NamedIndividual ;
	rdfs:isDefinedBy odrl: ;
	rdfs:label "Equal to"@en ;
	skos:definition "Indicating that a given value equals the right operand of the Constraint."@en .

:gt
	a :Operator, owl:NamedIndividual ;
	rdfs:isDefinedBy odrl: ;
	skos:definition "Indicating that a given value is greater than the right operand of the Constraint."@en ;
	rdfs:label "Greater than"@en .

:gteq
	a :Operator, owl:NamedIndividual ;
	rdfs:isDefinedBy odrl: ;
	skos:definition "Indicating that a given value is greater than or equal to the right operand of the Constraint."@en ;
	rdfs:label "Greater than or equal to"@en .

:hasPart
	a :Operator, owl:NamedIndividual ;
	rdfs:isDefinedBy odrl: ;
	skos:definition "Indicating that a given value contains the right operand of the Constraint."@en ;
	rdfs:label "Has part"@en ;
    skos:scopeNote "Non-Normative"@en .

:isA
	a :Operator, owl:NamedIndividual ;
	rdfs:isDefinedBy odrl: ;
	skos:definition "Indicating that a given value is an instance of the right operand of the Constraint."@en ;
	rdfs:label "Is a"@en .

:isAllOf
	a :Operator, owl:NamedIndividual ;
	rdfs:isDefinedBy odrl: ;
	skos:definition "Indicating that a given value is all of the right operand of the Constraint."@en ;
	rdfs:label "Is all of"@en ;
    skos:scopeNote "Non-Normative"@en .

:isAnyOf
	a :Operator, owl:NamedIndividual ;
	rdfs:isDefinedBy odrl: ;
	skos:definition "Indicating that a given value is any of the right operand of the Constraint."@en ;
	rdfs:label "Is any of"@en ;
    skos:scopeNote "Non-Normative"@en .

:isNoneOf
	a :Operator, owl:NamedIndividual ;
	rdfs:isDefinedBy odrl: ;
	skos:definition "Indicating that a given value is none of the right operand of the Constraint."@en ;
	rdfs:label "Is none of"@en ;
    skos:scopeNote "Non-Normative"@en .

:isPartOf
	a :Operator, owl:NamedIndividual ;
	rdfs:isDefinedBy odrl: ;
	skos:definition "Indicating that a given value is contained by the right operand of the Constraint."@en ;
	rdfs:label "Is part of"@en ;
    skos:scopeNote "Non-Normative"@en .

:lt
	a :Operator, owl:NamedIndividual ;
	rdfs:isDefinedBy odrl: ;
	skos:definition "Indicating that a given value is less than the right operand of the Constraint."@en ;
	rdfs:label "Less than"@en .

:lteq
	a :Operator, owl:NamedIndividual ;
	rdfs:isDefinedBy odrl: ;
	skos:definition "Indicating that a given value is less than or equal to the right operand of the Constraint."@en ;
	rdfs:label "Less than or equal to"@en .

:neq
	a :Operator, owl:NamedIndividual ;
	rdfs:isDefinedBy odrl: ;
	skos:definition "Indicating that a given value is not equal to the right operand of the Constraint."@en ;
	rdfs:label "Not equal to"@en .

:or
	a :Operator, owl:NamedIndividual ;
	rdfs:isDefinedBy odrl: ;
	skos:definition "The relation is satisfied when any of the Constraints are satisfied."@en ;
	rdfs:label "Or"@en ;
	skos:note "This operator MUST only be used for Compound Constraints, and both left and right operands MUST be Atomic Constraints."@en ;
    skos:scopeNote "Non-Normative"@en .
	
:and
	a :Operator, owl:NamedIndividual ;
	rdfs:isDefinedBy odrl: ;
	skos:definition "The relation is satisfied when both of the Constraints are satisfied."@en ;
	skos:note "This operator MUST only be used for Compound Constraints, and both left and right operands MUST be Atomic Constraints."@en ;
	rdfs:label "And"@en .

:xor
	a :Operator, owl:NamedIndividual ;
	rdfs:isDefinedBy odrl: ;
	skos:definition "The relation is satisfied when only one of the Constaints is satisfied"@en ;
	rdfs:label "Exclusive Or"@en ;
	skos:note "This operator MUST only be used for Compound Constraints, and both left and right operands MUST be Atomic Constraints."@en ;
    skos:scopeNote "Non-Normative"@en .
	
:andSequence
	a :Operator, owl:NamedIndividual ;
	rdfs:isDefinedBy odrl: ;
	skos:definition "The relation is satisfied when the left operand Atomic Constraint  delivers a satisfied result before the right operand Atomic Constraint is evaluated. The right operand Atomic Constraint may build on the satisfaction of the left operand Atomic Constraint."@en ;
	rdfs:label "And Sequence"@en ;
	skos:note "This operator MUST only be used for Compound Constraints, and both left and right operands MUST be Atomic Constraints."@en ;
    skos:scopeNote "Non-Normative"@en .

## LeftOperand

:LeftOperand
	a rdfs:Class , owl:Class ;
	rdfs:isDefinedBy odrl: ;
	rdfs:subClassOf owl:Thing ;
	rdfs:label "Left Operand"@en ;
	skos:definition "Left operands for constraint expressions."@en ;
	skos:note "Instances of the LeftOperand class represent the left term in a Constraint."@en .

## Left Operands

:absolutePosition
	a :LeftOperand, owl:NamedIndividual ;
	rdfs:isDefinedBy odrl: ;
	rdfs:label "Absolute Asset Position"@en ;
	skos:definition "A point in space or time defined with absolute coordinates the positioning of the Asset has to comply with for excersing the Action."@en ;
	skos:note "Example: May be used with a natural language contract saying the the upper left corner of a picture may be constrainted to a specific position of the canvas rendiering it."@en .

:absoluteSpatialPosition
	a :LeftOperand, owl:NamedIndividual ;
	rdfs:isDefinedBy odrl: ;
	skos:broaderTransitive :absolutePosition;
	rdfs:label "Absolute Spatial Asset Position"@en ;
	skos:definition "The absolute spatial positions of four corners of a rectangle on a 2D-canvas or the eight corners of a cubiod in a 3D-space the Asset has to fit in after the Action."@en ;
	skos:note "Example: May be used with a natural language contract saying the the upper left corner of a picture may be constrainted to a specific position of the canvas rendiering it. Note: see also the Left Operand Relative Spatial Asset Position. "@en ;
  skos:scopeNote "Non-Normative"@en .

:absoluteTemporalPosition
	a :LeftOperand, owl:NamedIndividual ;
	rdfs:isDefinedBy odrl: ;
	skos:broaderTransitive :absolutePosition;
	rdfs:label "Absolute Temporal Asset Position"@en ;
	skos:definition "The absolute temporal positions in a media stream the Asset has to fit in after the Action."@en ;
	skos:note "Note: Use with Actions including the Asset in a larger media stream. The fragment part of a Media Fragment URI (https://www.w3.org/TR/media-frags/) may be used for the right operand. See the Left Operand realativeTemporalPosition. Example: The MP3 music file must be positioned between second 192 and 250 of the temporal length of a stream."@en ;
  skos:scopeNote "Non-Normative"@en .

:absoluteSize
	a :LeftOperand, owl:NamedIndividual ;
	rdfs:isDefinedBy odrl: ;
	rdfs:label "Absolute Asset Size"@en ;
	skos:definition "Measure(s) of one or two axes for 2D-objects or measure(s) of one to tree axes for 3D-objects of the Asset after the Action."@en ;
	skos:note "Example: The image can be resized in width to a maximum of 1000px."@en ;
    skos:scopeNote "Non-Normative"@en .

:count
	a :LeftOperand, owl:NamedIndividual ;
	rdfs:isDefinedBy odrl: ;
	rdfs:label "Count"@en ;
	skos:definition "Numeric count of exercising the Action."@en ;
	skos:note "Should be a positive integer"@en .

:dateTime
	a :LeftOperand, owl:NamedIndividual ;
	rdfs:isDefinedBy odrl: ;
	rdfs:label "Action Datetime"@en ;
	skos:definition "The date (and optional time and timezone) to be compared to the time when the Action is exercised."@en ;
	skos:note "Right operand value MUST be an xsd:date or xsd:dateTime as defined by [[xmlschema11-2]]. The use of Timezone information is strongly recommended."@en ;
	skos:note "The Action of the Rule may be exercised before (with operator lt/lteq) or after (with operator gt/gteq) the date(time) defined by the Right operand. Example: <code>dateTime gteq 2017-12-31T06:00Z</code> means the Action can only be exercised after (and including) 6:00AM on the 31st Decemeber 2017 UTC time."@en .

:delayPeriod
	a :LeftOperand, owl:NamedIndividual ;
	rdfs:isDefinedBy odrl: ;
	rdfs:label "Action Delay Period"@en ;
	skos:definition "The Action may be exercised after the end of this time period. The point in time triggering this period MAY be defined by another temporal Atomic Constraint expressed together in a Compound Constraint (utilsing the odrl:andSequence operator)."@en ;
	skos:note "Right operand value MUST be an xsd:duration as defined by [[xmlschema11-2]]. Only the eq operator SHOULD be used."@en ;
	skos:note "Example: <code>delayPeriod eq P60M</code> indicates a delay of 60 Minutes before exercising the action."@en ;
    skos:scopeNote "Non-Normative"@en .

:deliveryChannel
	a :LeftOperand, owl:NamedIndividual ;
	rdfs:isDefinedBy odrl: ;
	rdfs:label "Delivery Channel"@en ;
	skos:definition "The delivery channel used for exercising the Action."@en ;
	skos:note "Example: the asset may be distributed only on mobile networks."@en .

:device
	a :LeftOperand, owl:NamedIndividual ;
	rdfs:isDefinedBy odrl: ;
	rdfs:label "Device"@en ;
	skos:definition "An identified computing system for exercising the Action."@en ;
  owl:deprecated true ;
	owl:equivalentProperty :systemDevice .

:elapsedTime
	a :LeftOperand, owl:NamedIndividual ;
	rdfs:isDefinedBy odrl: ;
	rdfs:label "Elapsed Time"@en ;
	skos:definition "The Action may be exercised during this time period. The start of the period is trigged by exercising the Action for the first time."@en ;
	skos:note "Right operand value MUST be an xsd:duration as defined by [[xmlschema11-2]]. Only the eq operator SHOULD be used."@en ;
	skos:note "Example: <code>elpasedTime eq P60M</code> indicates a total elpased time of 60 Minutes can be used for exercising the action." ;
    skos:scopeNote "Non-Normative"@en .

:event
	a :LeftOperand, owl:NamedIndividual ;
	rdfs:isDefinedBy odrl: ;
	rdfs:label "Event Action"@en ;
	skos:definition "An identified event used for exercising the Action."@en ;
	skos:note "Events are temporal periods of time, and operators can be used to signal before, during or after the event. Example: Action may be taken during the “FIFA World Cup 2020” only."@en .

:fileFormat
	a :LeftOperand, owl:NamedIndividual ;
	rdfs:isDefinedBy odrl: ;
	rdfs:label "File Format"@en ;
	skos:definition "The file format of the Asset after exercising the Action."@en ;
	skos:note "Example: An asset may be transformed into JPEG format."@en ;
    skos:scopeNote "Non-Normative"@en .

:industry
	a :LeftOperand, owl:NamedIndividual ;
	rdfs:isDefinedBy odrl: ;
	rdfs:label "Industry Context"@en ;
	skos:definition "The defined industry sector in which the Action may be exercised."@en ;
	skos:note "Example: publishing or financial industry."@en .

:language
	a :LeftOperand, owl:NamedIndividual ;
	rdfs:isDefinedBy odrl: ;
	rdfs:label "Language"@en ;
	skos:definition "The main natural language of the Asset after exercising the Action."@en ;
	skos:note "Example: the asset can only be translated into Greek. Must use [[bcp47]] codes for language values."@en .
  
:media
	a :LeftOperand, owl:NamedIndividual ;
	rdfs:isDefinedBy odrl: ;
	rdfs:label "Media Context"@en ;
	skos:definition "Category of media setting the context for exercising the Action."@en ;
	skos:note "Example media types: electronic, print, advertising, marketing. Note: The used type should not be an IANA MediaType as they are focused on technical characteristics. "@en ;
    skos:scopeNote "Non-Normative"@en .

:meteredTime
	a :LeftOperand, owl:NamedIndividual ;
	rdfs:isDefinedBy odrl: ;
	rdfs:label "Metered Time"@en ;
	skos:definition "The Action may be exercised for an accumulated amount of this time period."@en ;
	skos:note "Right operand value MUST be an xsd:duration as defined by [[xmlschema11-2]]. Only the eq operator SHOULD be used."@en ;
	skos:note "Example: <code>meteredTime eq P60M</code> indicates that the action can be exercised for an accumulated period of 60 Minutes. This means that the action can be expercised for 5 minutes each day over 12 days." ;
    skos:scopeNote "Non-Normative"@en .

:payAmount
	a :LeftOperand, owl:NamedIndividual ;
	rdfs:isDefinedBy odrl: ;
	rdfs:label "Payment Amount"@en ;
	skos:definition "The amount of a payment related to the Action of a Duty."@en ;
	skos:note "The datatype of the right operand must be xsd:decimal. Note: Can be used for compensation duties. The data type property of the Right Operand may be used to indicate the type of the value (eg decimal) and the unit property to indicate the currency."@en .

:percentage
	a :LeftOperand, owl:NamedIndividual ;
	rdfs:isDefinedBy odrl: ;
	rdfs:label "Asset Percentage"@en ;
	skos:definition "The amount of an Asset - as a percentage - used for exercising the Action."@en ;
	skos:note "The datatype of the right operand must be xsd:decimal from 0 to 100. Example: Extract less than or equal to of 50% of the asset."@en ;
    skos:scopeNote "Non-Normative"@en .

:product
	a :LeftOperand, owl:NamedIndividual ;
	rdfs:isDefinedBy odrl: ;
	rdfs:label "Product Context"@en ;
	skos:definition "Product or service used for exercising the Action."@en ;
	skos:note "Example: The Asset image may only be reproduced in the XYZ Magazine."@en ;
  skos:scopeNote "Non-Normative"@en .

:purpose
	a :LeftOperand, owl:NamedIndividual ;
	rdfs:isDefinedBy odrl: ;
	rdfs:label "Purpose"@en ;
	skos:definition "Purpose for exercising the Action."@en ;
	skos:note "Example: Educational use."@en .

:recipient
	a :LeftOperand, owl:NamedIndividual ;
	rdfs:isDefinedBy odrl: ;
	rdfs:label "Recipient"@en ;
	skos:definition "The party receiving the result of an exercised Action."@en ;
	skos:note "Note: The Right Operand must identify one or more specific parties or category/ies of the party."@en .

:relativePosition
	a :LeftOperand, owl:NamedIndividual ;
	rdfs:isDefinedBy odrl: ;
	rdfs:label "Relative Asset Position"@en ;
	skos:definition "A point in space or time defined with coordinates relative to full measures the positioning of the Asset has to comply with for excersing the Action."@en ;
	skos:note "Example: May be used with a natural language contract saying the the upper left corner of a picture may be constrainted to a specific position of the canvas rendiering it."@en ;
  skos:scopeNote "Non-Normative"@en .

:relativeSpatialPosition
	a :LeftOperand, owl:NamedIndividual ;
	rdfs:isDefinedBy odrl: ;
	skos:broaderTransitive :relativePosition;
	rdfs:label "Relative Spatial Asset Position"@en ;
	skos:definition "The relative spatial positions - expressed as percentages of full values - of four corners of a rectangle on a 2D-canvas or the eight corners of a cubiod in a 3D-space the Asset has to fit in after the Action."@en ;
	skos:note "Note: See the Left Operand absoluteSpatialAssetPosition."@en ;
  skos:scopeNote "Non-Normative"@en .

:relativeTemporalPosition
	a :LeftOperand, owl:NamedIndividual ;
	rdfs:isDefinedBy odrl: ;
	skos:broaderTransitive :relativePosition;
	rdfs:label "Relative Temporal Asset Position"@en ;
	skos:definition "A point in space or time defined with coordinates relative to full measures the positioning of the Asset has to comply with for excersing the Action."@en ;
	skos:note "Example: The MP3 music file must be positioned between the positions at 33% and 48% of the temporal length of a stream. Note: See the Left Operand absoluteTemporalAssetPosition. "@en ;
  skos:scopeNote "Non-Normative"@en .

:relativeSize
	a :LeftOperand, owl:NamedIndividual ;
	rdfs:isDefinedBy odrl: ;
	rdfs:label "Relative Asset Size"@en ;
	skos:definition "Measure(s) of one or two axes for 2D-objects or measure(s) of one to tree axes for 3D-objects - expressed as percentages of full values - of the Asset after the Action."@en ;
	skos:note "Example: The image can be resized in width to a maximum of 200%. Note: See the Left Operand absoluteSize. "@en ;
  skos:scopeNote "Non-Normative"@en .

:resolution
	a :LeftOperand, owl:NamedIndividual ;
	rdfs:isDefinedBy odrl: ;
	rdfs:label "Rendition Resolution"@en ;
	skos:definition "Resolution of the rendition of the Asset after exercising the Action."@en ;
	skos:note "Example: the image may be printed at 1200dpi."@en ;
    skos:scopeNote "Non-Normative"@en .

:spatial
	a :LeftOperand, owl:NamedIndividual ;
	rdfs:isDefinedBy odrl: ;
	rdfs:label "Geospatial Named Area"@en ;
	skos:definition "A named and identified geospatial area with defined borders for exercising the Action."@en ;
	skos:note "A code value for the area and source of the code must be presented in the Right Operand. For example, the [[iso3166]] Country Codes or the Getty Thesaurus of Geographic Names. An IRI should be used to represent this value."@en ;
    skos:scopeNote "Non-Normative"@en .

:spatialCoordinates
	a :LeftOperand, owl:NamedIndividual ;
	rdfs:isDefinedBy odrl: ;
	skos:broaderTransitive :spatial;
	rdfs:label "Geospatial Coordinates"@en ;
	skos:definition "A set of coordinates setting the borders of a geospatial area for exercising the Action."@en ;
	skos:note "The coordinates MUST include longitude and lattitue, they MAY include altitude and the geodatic datum. If the latter are ommitted the default values are the altitude of earth's surface at this location and the WGS 84 datum."@en ;
    skos:scopeNote "Non-Normative"@en .

:system
	a :LeftOperand, owl:NamedIndividual ;
	rdfs:isDefinedBy odrl: ;
	rdfs:label "System"@en ;
	skos:definition "An identified computing system for exercising the Action."@en ;
    owl:deprecated true ;
	owl:equivalentProperty :systemDevice .

:systemDevice
	a :LeftOperand, owl:NamedIndividual ;
	rdfs:isDefinedBy odrl: ;
	owl:equivalentProperty :system, :device ;
	rdfs:label "System Device"@en ;
	skos:definition "An identified computing system for exercising the Action."@en ;
	skos:note "Example: The system device can be identified by a unique code created from the used hardware."@en ;
  skos:scopeNote "Non-Normative"@en .

:timeInterval
	a :LeftOperand, owl:NamedIndividual ;
	rdfs:isDefinedBy odrl: ;
	rdfs:label "Recurring Time Interval"@en ;
	skos:definition "The Action may be exercised within a recurring period of time after which the Action can or cannot be exercised again until the time period has elapsed."@en ;
	skos:note "Right operand value MUST be an xsd:duration as defined by [[xmlschema11-2]]. Only the eq operator SHOULD be used."@en ;
	skos:note "Example: <code>timeInterval eq P7D</code> indicates that the action can be exercised once every 7 day period." ;
    skos:scopeNote "Non-Normative"@en .

:unitOfCount
	a :LeftOperand, owl:NamedIndividual ;
	rdfs:isDefinedBy odrl: ;
	rdfs:label "Unit Of Count"@en ;
	skos:definition "The unit of measure used for counting."@en ;
	skos:note "Typically used with Duties to indicate the unit entity to be counted."@en ;
    skos:scopeNote "Non-Normative"@en .

:version
	a :LeftOperand, owl:NamedIndividual ;
	rdfs:isDefinedBy odrl: ;
	rdfs:label "Version"@en ;
	skos:definition "The range of versions of the Asset which can or cannot be used for exercising the Action."@en ;
	skos:note "Example: Single Paperback or Multiple Issues or version 2.0 or higher."@en ;
    skos:scopeNote "Non-Normative"@en .

:virtualLocation
	a :LeftOperand, owl:NamedIndividual ;
	rdfs:isDefinedBy odrl: ;
	rdfs:label "Virtual IT Communication Location"@en ;
	skos:definition "An identified location of the IT communication space where the Action can or cannot be exercised."@en ;
	skos:note "Example: an Internet domain or IP address range."@en ;
  skos:scopeNote "Non-Normative"@en .


## RightOperand

:RightOperand
	a rdfs:Class , owl:Class ;
	rdfs:isDefinedBy odrl: ;
	rdfs:subClassOf owl:Thing ;
	rdfs:label "Right Operand"@en ;
	skos:definition "Right operands for constraint expressions."@en ;
	skos:note "Instances of the RightOperand class represent the right term in a Constraint."@en .

:policyUsage
	a :RightOperand, owl:NamedIndividual ;
	rdfs:isDefinedBy odrl: ;
	rdfs:label "Policy Usage Time"@en ;
	skos:definition "Indicates the time when the policy is exercised."@en ;
	skos:note "This can be used to express constraints related to the time the policy is exercised. For example,  <code>event lt policyUsage</code> expresses a constraint on the Action to occur before the policy is exercised. Other operators may be used to indicate during (eg) or after (gt, gte) policy usage."@en ;
    skos:scopeNote "Non-Normative"@en .

## Actions

:use
	a :Action, skos:Concept ;
	rdfs:isDefinedBy odrl: ;
	rdfs:label "Use"@en ;
	skos:definition "The Assigner permits/prohibits the Assignee to use the Asset as agreed."@en ;
	skos:note "Use is the most generic action for all non-third-party usage. More details may be defined in the applicable agreements or under applicable commercial laws. Refined types of actions can be expressed by the narrower actions."@en .

:grantUse
	a :Action, skos:Concept ;
	rdfs:isDefinedBy odrl: ;
	rdfs:label "Grant Use"@en ;
	skos:definition "The Assigner permits/prohibits the Assignee to grant the use the Asset to third parties."@en ;
	skos:note "This action enables the Assignee to create policies for the use of the Asset for third parties. nextPolicy is recommended to be agreed with the third party. Use of temporal constraints is recommended."@en ;
	skos:broaderTransitive odrl:use ;
    skos:scopeNote "Non-Normative"@en .

:compensate
	a :Action, skos:Concept ;
	rdfs:isDefinedBy odrl: ;
	rdfs:label "Compensate"@en ;
	skos:definition "The Assigner requires that the Assignees compensates the Assigner (or other specified compensation Party) by some amount of value, if defined, for use of the Asset."@en ;
	skos:note "The compensation may use different types of things with a value: (i) the thing is expressed by the value (term) of the Constraint name; (b) the value is expressed by operator, rightOperand, dataType and unit"@en .

:acceptTracking
	a :Action, skos:Concept ;
	rdfs:isDefinedBy odrl: ;
	rdfs:label "Accept Tracking"@en ;
	skos:definition "The Assigner requires that the Assignees accepts that the use of the Asset may be tracked."@en ;
	skos:note "The collected information may be tracked by the Assigner, or may link to a Party with the role “trackingParty” function."@en ;
    skos:scopeNote "Non-Normative"@en .


:aggregate
	a :Action, skos:Concept ;
	skos:broaderTransitive odrl:use ;
	rdfs:isDefinedBy odrl: ;
	rdfs:label "Aggregate"@en ;
	skos:definition "The Assigner permits/prohibits the Assignees to use the Asset or parts of it as part of a composite collection."@en ;
    skos:scopeNote "Non-Normative"@en .

:annotate
	a :Action, skos:Concept ;
	skos:broaderTransitive odrl:use ;
	rdfs:isDefinedBy odrl: ;
	rdfs:label "Annotate"@en ;
	skos:definition "The Assigner permits/prohibits the Assignees to add explanatory notations/commentaries to the Asset without modifying the Asset in any other way."@en ;
    skos:scopeNote "Non-Normative"@en .

:anonymize
	a :Action, skos:Concept ;
	skos:broaderTransitive odrl:use ;
	rdfs:isDefinedBy odrl: ;
	rdfs:label "Anonymize"@en ;
	skos:definition "The Assigner permits/prohibits the Assignees to anonymize all or parts of the Asset."@en ;
	skos:note "For example, to remove identifying particulars for statistical or for other comparable purposes, or to use the asset without stating the author/source."@en ;
    skos:scopeNote "Non-Normative"@en .

:append
	a :Action, skos:Concept ;
	rdfs:isDefinedBy odrl: ;
	rdfs:label "Append"@en ;
	skos:definition "The act of adding to the end of an asset."@en ;
    owl:deprecated true ;
	owl:equivalentProperty :modify .

:appendTo
	a :Action, skos:Concept ;
	rdfs:isDefinedBy odrl: ;
	rdfs:label "Append To"@en ;
	skos:broaderTransitive odrl:writeTo ;
	skos:definition "The act of appending data to the Asset without modifying the Asset in any other way."@en ;
    owl:deprecated true ;
	owl:equivalentProperty :modify .

:archive
	a :Action, skos:Concept ;
	rdfs:isDefinedBy odrl: ;
	rdfs:label "Archive"@en ;
	skos:definition "The Assigner permits/prohibits the Assignees to store the Asset (in a non-transient form)."@en ;
	skos:note "Constraints may be used for temporal conditions."@en ;
	skos:broaderTransitive :use ;
    skos:scopeNote "Non-Normative"@en .

:attribute
	a :Action, skos:Concept ;
	rdfs:isDefinedBy odrl: ;
	rdfs:label "Attribute"@en ;
	skos:definition "The Assigner requires that the Assignees attributes the Asset to the Assigner or an attributed Party."@en ;
	skos:note "May link to an Asset with the attribution information. May link to a Party with the  role “attributedParty” function."@en .

:concurrentUse
	a :Action, skos:Concept ;
	rdfs:isDefinedBy odrl: ;
	rdfs:label "Concurrent Use"@en ;
	skos:definition "The Assigner permits/prohibits the Assignees to create multiple copies of the Asset that are being concurrently used."@en ;
	skos:broaderTransitive :use ;
    skos:scopeNote "Non-Normative"@en .

:copy
	a :Action, skos:Concept ;
	rdfs:isDefinedBy odrl: ;
	owl:sameAs :reproduce ;
	rdfs:label "Copy"@en ;
	skos:definition "The act of making an exact reproduction of the asset."@en ;
    owl:deprecated true ;
	owl:equivalentProperty :reproduce .

:delete
	a :Action, skos:Concept ;
	rdfs:isDefinedBy odrl: ;
	rdfs:label "Delete"@en ;
	skos:definition "The Assigner requires that the Assignees permanently removes all copies of the Asset."@en ;
	skos:note "Use a constraint to define under which conditions the Asset should be deleted."@en ;
    skos:scopeNote "Non-Normative"@en .

:derive
	a :Action, skos:Concept ;
	rdfs:isDefinedBy odrl: ;
	rdfs:label "Derive"@en ;
	skos:definition "The Assigner permits/prohibits the Assignees to create a new derivative Asset from this Asset and to edit or modify the derivative."@en ;
	skos:note "A new asset is created and may have significant overlaps with the original Asset. (Note that the notion of whether or not the change is significant enough to qualify as a new asset is subjective). To the derived Asset a next policy may be applied."@en ;
	skos:broaderTransitive :use ;
    skos:scopeNote "Non-Normative"@en .

:digitize
	a :Action, skos:Concept ;
	rdfs:isDefinedBy odrl: ;
	rdfs:label "Digitize"@en ;
	skos:broaderTransitive :use ;
	skos:definition "The Assigner permits/prohibits the Assignees to produce a digital copy of (or otherwise digitize) the Asset from its analogue form."@en ;
    skos:scopeNote "Non-Normative"@en .

:display
	a :Action, skos:Concept ;
	rdfs:isDefinedBy odrl: ;
	rdfs:label "Display"@en ;
	skos:definition "The Assigner permits/prohibits the Assignees to display the visual media Asset."@en ;
	skos:note "For example, displaying an image on a screen. If the action is to be performed to a wider audience than just the Assignees, then the Recipient constraint is recommened to be used."@en ;
	skos:broaderTransitive :present .

:distribute
	a :Action, skos:Concept ;
	rdfs:isDefinedBy odrl: ;
	rdfs:label "Distribute"@en ;
	skos:definition "The Assigner permits/prohibits the Assignees to distribute the Asset."@en ;
	skos:broaderTransitive :use .

:ensureExclusivity
	a :Action, skos:Concept ;
	rdfs:isDefinedBy odrl: ;
	rdfs:label "Ensure Exclusivity"@en ;
	skos:definition "The Assignee requires that the Assigners ensure that the permission on the Asset is exclusive to the Assignee."@en ;
    skos:scopeNote "Non-Normative"@en .

:execute
	a :Action, skos:Concept ;
	rdfs:isDefinedBy odrl: ;
	rdfs:label "Execute"@en ;
	skos:definition "The Assigner permits/prohibits the Assignees to run the computer program Asset."@en ;
	skos:note "For example, machine executable code or Java such as a game or application."@en ;
	skos:broaderTransitive :use ;
    skos:scopeNote "Non-Normative"@en .

:export
	a :Action, skos:Concept ;
	rdfs:isDefinedBy odrl: ;
	rdfs:label "Export"@en ;
	skos:definition "The act of transforming the asset into a new form."@en ;
    owl:deprecated true ;
	owl:equivalentProperty :transform .


:extract
	a :Action, skos:Concept ;
	rdfs:isDefinedBy odrl: ;
	rdfs:label "Extract"@en ;
	skos:definition "The Assigner permits/prohibits the Assignees to extract parts of the Asset and to use it as a new Asset."@en ;
	skos:note "A new asset is created and may have very little in common with the original Asset. (Note that the notion of whether or not the change is significant enough to qualify as a new asset is subjective). To the extracted Asset a next policy may be applied."@en ;
	skos:broaderTransitive :reproduce ;
    skos:scopeNote "Non-Normative"@en .

:give
	a :Action, skos:Concept ;
	rdfs:isDefinedBy odrl: ;
	rdfs:label "Give"@en ;
	skos:definition "The Assigner permits/prohibits the Assignees to transfer the ownership of the Asset to a third party without compensation and while deleting the original asset."@en ;
	skos:broaderTransitive :transfer ;
    skos:scopeNote "Non-Normative"@en .

:include
	a :Action, skos:Concept ;
	rdfs:isDefinedBy odrl: ;
	rdfs:label "Include"@en ;
	skos:definition "The Assigner requires that the Assignees include other related assets in the Asset."@en ;
	skos:note "For example: bio picture must be included in the attribution. Use of the Asset relation attribute is required."@en ;
    skos:scopeNote "Non-Normative"@en .

:index
	a :Action, skos:Concept ;
	rdfs:isDefinedBy odrl: ;
	rdfs:label "Index"@en ;
	skos:definition "The Assigner permits/prohibits the Assignees to record the Asset in an index."@en ;
	skos:note "For example, to include a link to the Asset in a search engine database."@en ;
	skos:broaderTransitive :use ;
    skos:scopeNote "Non-Normative"@en .

:inform
	a :Action, skos:Concept ;
	rdfs:isDefinedBy odrl: ;
	rdfs:label "Inform"@en ;
	skos:definition "The Assigner requires that the Assignees inform the Assigner or an informed Party that an action has been performed on or in relation to the Asset."@en ;
	skos:note "May link to a Party with the role “informedParty” function."@en ;
    skos:scopeNote "Non-Normative"@en .

:install
	a :Action, skos:Concept ;
	rdfs:isDefinedBy odrl: ;
	rdfs:label "Install"@en ;
	skos:definition "The Assigner permits/prohibits the Assignees to load the computer program Asset onto a storage device which allows operating or running the Asset."@en ;
	skos:broaderTransitive :use ;
    skos:scopeNote "Non-Normative"@en .

:lease
	a :Action, skos:Concept ;
	rdfs:isDefinedBy odrl: ;
	rdfs:label "Lease"@en ;
	skos:definition "The act of making available the asset to a third-party for a fixed period of time with exchange of value."@en ;
    owl:deprecated true .


:license
	a :Action, skos:Concept ;
	rdfs:isDefinedBy odrl: ;
	rdfs:label "License"@en ;
	skos:definition "The act of granting the right to use the asset to a third-party."@en ;
    owl:deprecated true ;
	owl:equivalentProperty :grantUse .


:lend
	a :Action, skos:Concept ;
	rdfs:isDefinedBy odrl: ;
	rdfs:label "Lend"@en ;
	skos:definition "The act of making available the asset to a third-party for a fixed period of time without exchange of value."@en ;
    owl:deprecated true .


:modify
	a :Action, skos:Concept ;
	rdfs:isDefinedBy odrl: ;
	rdfs:label "Modify"@en ;
	skos:definition "The Assigner permits/prohibits the Assignees to update existing content of the Asset. A new asset is not created by this action."@en ;
	skos:note "This action will modify an asset which is typically updated from time to time without creating a new asset like a database. If the result from modifying the asset should be a new asset the actions derive or extract should be used. (Note that the notion of whether or not the change is significant enough to qualify as a new asset is subjective)."@en ;
	skos:broaderTransitive :use ;
    skos:scopeNote "Non-Normative"@en .

:move
	a :Action, skos:Concept ;
	rdfs:isDefinedBy odrl: ;
	rdfs:label "Move"@en ;
	skos:definition "The Assigner permits/prohibits the Assignees to move the Asset from one digital location to another including deleting the original copy."@en ;
	skos:note "After the Asset has been moved, the original copy must be deleted."@en ;
	skos:broaderTransitive :use ;
    skos:scopeNote "Non-Normative"@en .

:nextPolicy
	a :Action, skos:Concept ;
	rdfs:isDefinedBy odrl: ;
	rdfs:label "Next Policy"@en ;
	skos:definition "The Assigner requires that the Assignees grants the specified Policy to a third party for their use of the Asset."@en ;
	skos:note "Useful for downstream policies."@en .

:obtainConsent
	a :Action, skos:Concept ;
	rdfs:isDefinedBy odrl: ;
	rdfs:label "Obtain Consent"@en ;
	skos:definition "The Assigner requires that the Assignees obtains explicit consent from the Assigner or a consenting Party to perform the requested action in relation to the Asset."@en ;
	skos:note "Used as a Duty to ensure that the Assigner or a Party is authorized to approve such actions on a case-by-case basis. May link to a Party with the role “consentingParty” function."@en ;
    skos:scopeNote "Non-Normative"@en .

:pay
	a :Action, skos:Concept ;
	rdfs:isDefinedBy odrl: ;
	rdfs:label "Pay"@en ;
	skos:definition "The act of paying a financial amount to a party for use of the asset."@en ;
    owl:deprecated true ;
	owl:equivalentProperty :compensate .

:play
	a :Action, skos:Concept ;
	rdfs:isDefinedBy odrl: ;
	rdfs:label "Play"@en ;
	skos:definition "The Assigner permits/prohibits the Assignees to perform an audio Asset."@en ;
	skos:broaderTransitive :present ;
    skos:note "If the action is to be performed to a wider audience than just the Assignees, then the Recipient constraint is recommened to be used.";
    skos:scopeNote "Non-Normative"@en .

:present
	a :Action, skos:Concept ;
	rdfs:isDefinedBy odrl: ;
	rdfs:label "Present"@en ;
	skos:definition "The Assigner permits/prohibits the Assignees to perform or exhibit an Asset."@en ;
	skos:broaderTransitive :use ;
   skos:note "If the action is to be performed to a wider audience than just the Assignees, then the Recipient constraint is recommened to be used.";
    skos:scopeNote "Non-Normative"@en .

:preview
	a :Action, skos:Concept ;
	rdfs:isDefinedBy odrl: ;
	rdfs:label "Preview"@en ;
	skos:definition "The act of providing a short preview of the asset."@en ;
    skos:note "Use a time constraint with the appropriate action."@en ;
    owl:deprecated true .


:print
	a :Action, skos:Concept ;
	rdfs:isDefinedBy odrl: ;
	rdfs:label "Print"@en ;
	skos:definition "The Assigner permits/prohibits the Assignees to print an Asset onto paper or to create a hard copy."@en ;
	skos:note "For example, creating a permanent, fixed (static), and directly perceivable representation of the Asset."@en ;
	skos:broaderTransitive :present ;
    skos:scopeNote "Non-Normative"@en .

:read
	a :Action, skos:Concept ;
	rdfs:isDefinedBy odrl: ;
	rdfs:label "Read"@en ;
	skos:definition "The Assigner permits/prohibits the Assignees to obtain data from the Asset."@en ;
	skos:note "For example, the ability to read a record from a database (the Asset)."@en ;
	skos:broaderTransitive :use ;
    skos:scopeNote "Non-Normative"@en .

:reproduce
	a :Action, skos:Concept ;
	rdfs:isDefinedBy odrl: ;
	rdfs:label "Reproduce"@en ;
	skos:definition "The Assigner permits/prohibits the Assignee(s) to make (an) exact reproduction(s) of the Asset."@en ;
	skos:broaderTransitive :use ;
    skos:scopeNote "Non-Normative"@en .

:reviewPolicy
	a :Action, skos:Concept ;
	rdfs:isDefinedBy odrl: ;
	rdfs:label "Review Policy"@en ;
	skos:definition "The Assigner requires that the Assignee(s) has(ve) a person review the Policy applicable to the Asset."@en ;
	skos:note "Used when human intervention is required to review the Policy. May link to an Asset which represents the full Policy information."@en ;
    skos:scopeNote "Non-Normative"@en .

:secondaryUse
	a :Action, skos:Concept ;
	rdfs:isDefinedBy odrl: ;
	rdfs:label "Secondary Use"@en ;
	skos:definition "The act of using the asset for a purpose other than the purpose it was intended for."@en ;
    owl:deprecated true .

:sell
	a :Action, skos:Concept ;
	rdfs:isDefinedBy odrl: ;
	rdfs:label "Sell"@en ;
	skos:definition "The Assigner permits/prohibits the Assignees to transfer the ownership of the Asset to a third party with compensation and while deleting the original asset."@en ;
	skos:broaderTransitive :transfer ;
    skos:scopeNote "Non-Normative"@en .

:stream
	a :Action, skos:Concept ;
	rdfs:isDefinedBy odrl: ;
	rdfs:label "Stream"@en ;
	skos:definition "The Assigner permits/prohibits the Assignees to deliver the Asset in real-time."@en ;
	skos:broaderTransitive :use ;
    skos:note "The Asset maybe utilised in real-time as it is being delivered. If the action is to be performed to a wider audience than just the Assignees, then the Recipient constraint is recommened to be used.";
    skos:scopeNote "Non-Normative"@en .

:textToSpeech
	a :Action, skos:Concept ;
	rdfs:isDefinedBy odrl: ;
	rdfs:label "Text-to-speech"@en ;
	skos:definition "The Assigner permits/prohibits the Assignees to have a text Asset read out loud."@en ;
	skos:broaderTransitive :use ;
    skos:note "If the action is to be performed to a wider audience than just the Assignees, then the Recipient constraint is recommened to be used.";
    skos:scopeNote "Non-Normative"@en .

:transfer
	a :Action, skos:Concept ;
	rdfs:isDefinedBy odrl: ;
	rdfs:label "Transfer"@en ;
	skos:definition "The Assigner transfers/does not transfer the ownership in perpetuity to the Assignees."@en ;
    skos:scopeNote "Non-Normative"@en .

:transform
	a :Action, skos:Concept ;
	rdfs:isDefinedBy odrl: ;
	rdfs:label "Transform"@en ;
	skos:definition "The Assigner permits/prohibits the Assignees to make a digital copy of the digital Asset in another digital format."@en ;
	skos:note "Typically used to convert the Asset into a different format for consumption on/transfer to a third party system."@en ;
	skos:broaderTransitive :use ;
    skos:scopeNote "Non-Normative"@en .

:translate
	a :Action, skos:Concept ;
	rdfs:isDefinedBy odrl: ;
	rdfs:label "Translate"@en ;
	skos:definition "The Assigner permits/prohibits the Assignees to translate the original natural language of an Asset into another natural language."@en ;
	skos:note "A new derivative Asset is created by that action."@en ;
	skos:broaderTransitive :use .

:uninstall
	a :Action, skos:Concept ;
	rdfs:isDefinedBy odrl: ;
	rdfs:label "Uninstall"@en ;
	skos:definition "The Assigner requires that the Assignees unload and delete the computer program Asset from a storage device and disable its readiness for operation."@en ;
	skos:note "The Asset is no longer accessible to the Assignees."@en ;
    skos:scopeNote "Non-Normative"@en .

:watermark
	a :Action, skos:Concept ;
	rdfs:isDefinedBy odrl: ;
	rdfs:label "Watermark"@en ;
	skos:definition "The Assigner requires that the Assignees apply a watermark as provided by the Assigner to the Asset."@en ;
	skos:note "It is recommended to embed a link to the watermark."@en ;
    skos:scopeNote "Non-Normative"@en .

:write
	a :Action, skos:Concept ;
	rdfs:isDefinedBy odrl: ;
	rdfs:label "Write"@en ;
	skos:definition "The act of writing to the asset."@en ;
    owl:deprecated true ;
	owl:equivalentProperty :modify .


:writeTo
	a :Action, skos:Concept ;
	rdfs:isDefinedBy odrl: ;
	rdfs:label "Write to"@en ;
	skos:broaderTransitive odrl:use ;
	skos:definition "The act of adding data to the Asset."@en ;
    owl:deprecated true ;
	owl:equivalentProperty :modify .


## Functions

:assignee
	a rdf:Property , owl:ObjectProperty ;
	rdfs:isDefinedBy odrl: ;
	rdfs:subPropertyOf :function ;
	rdfs:label "Assignee"@en ;
	skos:definition "The Party is the recipient of the policy statement."@en ;
	rdfs:domain :Rule ;
	rdfs:range :Party .

:assigner
	a rdf:Property , owl:ObjectProperty ;
	rdfs:isDefinedBy odrl: ;
	rdfs:subPropertyOf :function ;
	rdfs:label "Assigner"@en ;
	skos:definition "The Party is the issuer of the policy statement."@en ;
	rdfs:domain :Rule ;
	rdfs:range :Party .

:attributedParty
	a rdf:Property , owl:ObjectProperty ;
	rdfs:isDefinedBy odrl: ;
	rdfs:subPropertyOf :function ;
	rdfs:label "Attributed Party"@en ;
	skos:definition "The Party to be attributed."@en ;
	skos:note "Maybe specified as part of the attribute action."@en .

:attributingParty
	a rdf:Property , owl:ObjectProperty ;
	rdfs:isDefinedBy odrl: ;
	rdfs:subPropertyOf :function ;
	rdfs:label "Attributing Party"@en ;
	skos:definition "The Party who undertakes the attribution."@en ;
	skos:note "Maybe specified as part of the attribute action."@en ;
    skos:scopeNote "Non-Normative"@en .

:consentingParty
	a rdf:Property , owl:ObjectProperty ;
	rdfs:isDefinedBy odrl: ;
	rdfs:subPropertyOf :function ;
	rdfs:label "Consenting Party"@en ;
	skos:definition "The Party to obtain consent from."@en ;
	skos:note "Maybe specified as part of the obtainConsent action."@en .

:consentedParty
	a rdf:Property , owl:ObjectProperty ;
	rdfs:isDefinedBy odrl: ;
	rdfs:subPropertyOf :function ;
	rdfs:label "Consented Party"@en ;
	skos:definition "The Party who obtains the consent."@en ;
	skos:note "Maybe specified as part of the obtainConsent action."@en ;
    skos:scopeNote "Non-Normative"@en .

:informedParty
	a rdf:Property , owl:ObjectProperty ;
	rdfs:isDefinedBy odrl: ;
	rdfs:subPropertyOf :function ;
	rdfs:label "Informed Party"@en ;
	skos:definition "The Party to be informed of all uses."@en ;
	skos:note "Maybe specified as part of the inform action."@en ;
    skos:scopeNote "Non-Normative"@en .

:informingParty
	a rdf:Property , owl:ObjectProperty ;
	rdfs:isDefinedBy odrl: ;
	rdfs:subPropertyOf :function ;
	rdfs:label "Informing Party"@en ;
	skos:definition "The Party who provides the inform use data."@en ;
	skos:note "Maybe specified as part of the inform action."@en ;
    skos:scopeNote "Non-Normative"@en .

:payeeParty
	a rdf:Property , owl:ObjectProperty ;
	rdfs:isDefinedBy odrl: ;
	rdfs:label "Payee Party"@en ;
	skos:definition "The Party is the recipient of the payment."@en ;
    owl:deprecated true ;
	owl:equivalentProperty :compensatedParty .


:compensatedParty
	a rdf:Property , owl:ObjectProperty ;
	rdfs:isDefinedBy odrl: ;
	rdfs:subPropertyOf :function ;
	rdfs:label "Compensated Party"@en ;
	skos:definition "The Party is the recipient of the compensation."@en ;
	skos:note "Maybe specified as part of the compensate duty action."@en ;
    skos:scopeNote "Non-Normative"@en .

:compensatingParty
	a rdf:Property , owl:ObjectProperty ;
	rdfs:isDefinedBy odrl: ;
	rdfs:subPropertyOf :function ;
	rdfs:label "Compensating Party"@en ;
	skos:definition "The Party that is the provider of the compensation."@en ;
	skos:note "Maybe specified as part of the compensate duty action."@en ;
    skos:scopeNote "Non-Normative"@en .

:trackingParty
	a rdf:Property , owl:ObjectProperty ;
	rdfs:isDefinedBy odrl: ;
	rdfs:subPropertyOf :function ;
	rdfs:label "Tracking Party"@en ;
	skos:definition "The Party who is tracking usage."@en ;
	skos:note "May be specified as part of the acceptTracking action."@en .

:trackedParty
	a rdf:Property , owl:ObjectProperty ;
	rdfs:isDefinedBy odrl: ;
	rdfs:subPropertyOf :function ;
	rdfs:label "Tracked Party"@en ;
	skos:definition "The Party whose usage is being tracked."@en ;
	skos:note "May be specified as part of the acceptTracking action."@en ;
    skos:scopeNote "Non-Normative"@en .

:contractingParty
	a rdf:Property , owl:ObjectProperty ;
	rdfs:isDefinedBy odrl: ;
	rdfs:subPropertyOf :function ;
	rdfs:label "Contracting Party"@en ;
	skos:definition "The Party who is offering the contract."@en ;
    skos:scopeNote "Non-Normative"@en .

:contractedParty
	a rdf:Property , owl:ObjectProperty ;
	rdfs:isDefinedBy odrl: ;
	rdfs:subPropertyOf :function ;
	rdfs:label "Contracted Party"@en ;
	skos:definition "The Party who is being contracted."@en ;
    skos:scopeNote "Non-Normative"@en .

## Policies

:Agreement
	a rdfs:Class , owl:Class ;
	rdfs:isDefinedBy odrl: ;
	rdfs:subClassOf :Policy ;
	owl:disjointWith :Offer, :Privacy, :Request, :Set, :Ticket, :Assertion ;
	rdfs:label "Agreement"@en ;
	skos:definition "A Policy that grants the assignee a Rule over an Asset from an assigner."@en ;
	skos:note "An Agreement Policy MUST contain a target Asset, a Party  with Assigner function, a Party with Assignee fuction, and at least one of a Permission or Prohibition rule. The Agreement Policy will grant the terms of the Policy from the Assigner to the Assignee."@en .

:Assertion
	a rdfs:Class , owl:Class ;
	rdfs:isDefinedBy odrl: ;
	rdfs:subClassOf :Policy ;
	owl:disjointWith :Offer, :Privacy, :Request, :Set, :Ticket ;
	rdfs:label "Assertion"@en ;
	skos:definition "A Policy that asserts a Rule over an Asset from parties."@en ;
	skos:note "For example, a party (an assignee or assigner) can claim what terms they have over an Asset. An Assertion Policy does not grant such permissions/prohibitions but only asserts the parties claims. An Assetion Policy  MUST contain a target Asset, a Party with any functional role, and at least one of a Permission or Prohibition rule."@en .

:Offer
	a rdfs:Class , owl:Class ;
	rdfs:isDefinedBy odrl: ;
	rdfs:subClassOf :Policy ;
	owl:disjointWith :Agreement, :Privacy, :Request, :Set, :Ticket, :Assertion ;
	rdfs:label "Offer"@en ;
	skos:definition "A Policy that proposes a Rule over an Asset from an assigner."@en ;
	skos:note "A Offer Policy  MUST contain a target Asset, a Party with Assigner function, and at least one of a Permission or Prohibition rule. The Offer Policy  MAY contain a Party  with Assignee function, but MUST not grant any privileges to that Party."@en .

:Privacy
	a rdfs:Class , owl:Class ;
	rdfs:isDefinedBy odrl: ;
	rdfs:subClassOf :Policy ;
	owl:disjointWith :Agreement, :Offer, :Request, :Set, :Ticket, :Assertion ;
	rdfs:label "Privacy"@en ;
	skos:definition "A Policy that expresses a Rule over an Asset containing personal information."@en ;
	skos:note "A Privacy Policy  MUST contain a target Asset, a Party with Assigner  is, a Party with Assignee function, and at least one of a Permission or Prohibition rule that MUST include a Duty. The target Asset SHOULD contain or relate to personal information about the Assignee. The Duty MUST describe  obligations on the Assigner about managing the Asset. The Assignee is being granted the terms of the Privacy policy from the Assigner."@en ;
   skos:scopeNote "Non-Normative"@en .

:Request
	a rdfs:Class , owl:Class ;
	rdfs:isDefinedBy odrl: ;
	rdfs:subClassOf :Policy ;
	owl:disjointWith :Agreement, :Offer, :Privacy, :Set, :Ticket, :Assertion ;
	rdfs:label "Request"@en ;
	skos:definition "A Policy that proposes a Rule over an Asset from an assignee."@en ;
	skos:note "A Request Policy  MUST contain a target Asset, a Party with Assignee function, and at least one of a Permission or Prohibition rule. The Request MAY also contain the Party with Assigner function if this is known. No privileges are granted to any Party."@en ;
    skos:scopeNote "Non-Normative"@en .

:Set
	a rdfs:Class , owl:Class ;
	rdfs:isDefinedBy odrl: ;
	rdfs:subClassOf :Policy ;
	owl:disjointWith :Agreement, :Offer, :Privacy, :Request, :Ticket, :Assertion ;
	rdfs:label "Set"@en ;
	skos:definition "A Policy that expresses a Rule over an Asset."@en ;
	skos:note "A Set Policy MUST contain a target Asset, and at least one Rule. A Set Policy is the default Policy subclass. The Set is aimed at scenarios where there is an open criteria for the semantics of the policy expressions and typically refined by other systems/profiles that process the information at a later time. No privileges are granted to any Party (if defined)."@en .

:Ticket
	a rdfs:Class , owl:Class ;
	rdfs:isDefinedBy odrl: ;
	rdfs:subClassOf :Policy ;
	owl:disjointWith :Agreement, :Offer, :Privacy, :Request, :Set, :Assertion ;
	rdfs:label "Ticket"@en ;
	skos:definition "A Policy that grants the holder a Rule over an Asset from an assigner."@en ;
	skos:note "A Ticket Policy MUST contain a target Asset and at least one of a Permission or Prohibition rule.  The Ticket MAY contain the Party with Assigner function and MUST NOT contain an Assignee. The Ticket Policy will grant the terms of the Policy to the holder of that Ticket. The holder of the Ticket MAY remain unknown or MAY have to be identified at some later stage."@en ;
    skos:scopeNote "Non-Normative"@en .

## Scopes

:AssetScope
	a rdfs:Class , owl:Class ;
	rdfs:isDefinedBy odrl: ;
	rdfs:subClassOf owl:Thing ;
	rdfs:label "Asset Scope"@en ;
	skos:definition "Scopes for Asset Scope expressions."@en ;
	skos:note "Instances of the AssetScope class represent the terms for the scope property of Assets."@en .

:PartyScope
	a rdfs:Class , owl:Class ;
	rdfs:isDefinedBy odrl: ;
	rdfs:subClassOf owl:Thing ;
	rdfs:label "Party Scope"@en ;
	skos:definition "Scopes for Party Scope expressions."@en ;
	skos:note "Instances of the PartyScope class represent the terms for the scope property of Parties."@en .

:All
	a :PartyScope, owl:NamedIndividual ;
	rdfs:isDefinedBy odrl: ;
	rdfs:label "All"@en ;
	skos:definition "Specifies that the scope of the relationship is all of the collective individuals within a context."@en ;
	skos:note "For example, may be used to indicate all the users of a specific social network the party is a member of. Note that “group” scope is also assumed."@en ;
    skos:scopeNote "Non-Normative"@en .

:All2ndConnections
	a :PartyScope, owl:NamedIndividual ;
	rdfs:isDefinedBy odrl: ;
	rdfs:label "All Second-level Connections"@en ;
	skos:definition "Specifies that the scope of the relationship is all of the second-level connections to the Party."@en ;
	skos:note "For example, may be used to indicate all “friends of friends” of the Party. Note that “group” scope is also assumed."@en ;
    skos:scopeNote "Non-Normative"@en .

:AllConnections
	a :PartyScope, owl:NamedIndividual ;
	rdfs:isDefinedBy odrl: ;
	rdfs:label "All First-Level Connections"@en ;
	skos:definition "Specifies that the scope of the relationship is all of the first-level connections of the Party."@en ;
	skos:note "For example, may be used to indicate all “friends” of the Party. Note that “group” scope is also assumed."@en ;
    skos:scopeNote "Non-Normative"@en .

:AllGroups
	a :PartyScope, owl:NamedIndividual ;
	rdfs:isDefinedBy odrl: ;
	rdfs:label "All Group Connections"@en ;
	skos:definition "Specifies that the scope of the relationship is all of the group connections of the Party."@en ;
	skos:note "For example, may be used to indicate all groups that the Party is a member of. Note that “group” scope is also assumed."@en ;
    skos:scopeNote "Non-Normative"@en .

:Group
	a :PartyScope, owl:NamedIndividual ;
	rdfs:isDefinedBy odrl: ;
	rdfs:label "Group"@en ;
	skos:definition "Specifies that the scope of the relationship is the defined group with multiple individual members."@en ;
    skos:scopeNote "Non-Normative"@en .

:Individual
	a :PartyScope, owl:NamedIndividual ;
	rdfs:isDefinedBy odrl: ;
	rdfs:label "Individual"@en ;
	skos:definition "Specifies that the scope of the relationship is the single Party individual."@en .

## Deprecated terms

:adHocShare
	a :Action, skos:Concept ;
	rdfs:isDefinedBy odrl: ;
	rdfs:label "Ad-hoc sharing"@en ;
	skos:definition "The act of sharing the asset to parties in close proximity to the owner."@en ;
    skos:note "This original term and URI from the OMA specification should be used: http://www.openmobilealliance.com/oma-dd/adhoc-share ."@en ;
    owl:deprecated true .

:extractChar
	a :Action, skos:Concept ;
	skos:broader :extract ;
	rdfs:isDefinedBy odrl: ;
	rdfs:label "Extract character"@en ;
	skos:definition "The act of extracting (replicating) unchanged characters from the asset."@en ;
 skos:note "This original term and URI from the ONIX specification should be used: http://www.editeur.org/onix-pl/extract-char ."@en ;
  owl:deprecated true .

:extractPage
	a :Action, skos:Concept ;
	skos:broader :extract ;
	rdfs:isDefinedBy odrl: ;
	rdfs:label "Extract page"@en ;
	skos:definition "The act of extracting (replicating) unchanged pages from the asset."@en ;
 skos:note "This original term and URI from the ONIX specification should be used: http://www.editeur.org/onix-pl/extract-page ."@en ;
    owl:deprecated true .


:extractWord
	a :Action, skos:Concept ;
	skos:broader :extract ;
	rdfs:isDefinedBy odrl: ;
	rdfs:label "Extract word"@en ;
	skos:definition "The act of extracting (replicating) unchanged words from the asset."@en ;
 skos:note "This original term and URI from the ONIX specification should be used: http://www.editeur.org/onix-pl/extract-word ."@en ;
    owl:deprecated true .

:attachPolicy
	a :Action, skos:Concept ;
	rdfs:isDefinedBy odrl: ;
	rdfs:label "Attach policy"@en ;
	skos:definition "The act of keeping the policy notice with the asset."@en ;
    owl:deprecated true ;
	owl:equivalentProperty <http://creativecommons.org/ns#Notice> .

:attachSource
	a :Action, skos:Concept ;
	rdfs:isDefinedBy odrl: ;
	rdfs:label "Attach source"@en ;
	skos:definition "The act of attaching the source of the asset and its derivatives."@en ;
    owl:deprecated true ;
	owl:equivalentProperty <http://creativecommons.org/ns#SourceCode> .

:shareAlike
	a :Action, skos:Concept ;
	rdfs:isDefinedBy odrl: ;
	rdfs:label "Share-alike"@en ;
	skos:definition "The act of distributing any derivative asset under the same terms as the original asset."@en ;
    owl:deprecated true ;
	owl:equivalentProperty <http://creativecommons.org/ns#ShareAlike> .

:commercialize
	a :Action, skos:Concept ;
	rdfs:isDefinedBy odrl: ;
	rdfs:label "Commercialize"@en ;
	skos:definition "The act of using the asset in a business environment."@en ;
    owl:deprecated true ;
	owl:equivalentProperty <http://creativecommons.org/ns#CommercialUse> .

:share
	a :Action, skos:Concept ;
	rdfs:isDefinedBy odrl: ;
	rdfs:label "Share"@en ;
	skos:definition "The act of the non-commercial reproduction and distribution of the asset to third-parties."@en ;
    owl:deprecated true ;
	owl:equivalentProperty <http://creativecommons.org/ns#Distribution> .


:proximity
	a rdf:Property , owl:DatatypeProperty ;
##	rdfs:subPropertyOf :rightOperand ;
	rdfs:isDefinedBy odrl: ;
	rdfs:label "proximity"@en ;
	skos:definition "An value indicating the closeness or nearness."@en ;
    skos:note "This original term and URI from the OMA specification should be used: http://www.openmobilealliance.com/oma-dd/proximity ."@en ;
    owl:deprecated true .

:timedCount
	a rdf:Property , owl:DatatypeProperty ;
##	rdfs:subPropertyOf :rightOperand ;
	rdfs:isDefinedBy odrl: ;
	rdfs:label "Timed Count"@en ;
	skos:definition "The number of seconds after which timed metering use of the asset begins."@en ;
	rdfs:range rdfs:Literal ;
    skos:note "This original term and URI from the OMA specification should be used: http://www.openmobilealliance.com/oma-dd/timed-count ."@en ;
    owl:deprecated true .

## Declaration of annotation properties to keep the ontology within OWL DL
	skos:broader rdf:type owl:AnnotationProperty .
	skos:member rdf:type owl:AnnotationProperty .
	skos:note rdf:type owl:AnnotationProperty .
	skos:scopeNote rdf:type owl:AnnotationProperty .
	skos:prefLabel rdf:type owl:AnnotationProperty .
	skos:definition rdf:type owl:AnnotationProperty .
	skos:broaderTransitive rdf:type owl:AnnotationProperty .
	skos:hasTopConcept rdf:type owl:AnnotationProperty .
	dct:contributor rdf:type owl:AnnotationProperty .
	dct:license rdf:type owl:AnnotationProperty .
	dct:issued rdf:type owl:AnnotationProperty .
	dct:subject rdf:type owl:AnnotationProperty .
	dct:creator rdf:type owl:AnnotationProperty .
	dct:description rdf:type owl:AnnotationProperty .
	dct:isVersionOf rdf:type owl:AnnotationProperty .
	dct:format rdf:type owl:AnnotationProperty .
	dcmit:Text a owl:Class .	
	skos:Collection a owl:Class .	
	skos:Concept a owl:Class .	
	skos:ConceptScheme a owl:Class .	
	voaf:Vocabulary a owl:Class .

	